propagating to 768

proof/correctness768/avx2/MLKEM_avx2_equivs.ec
@@ -1,12 +1,12 @@
 require import AllCore List Int IntDiv CoreMap Real Number.
 
 from Jasmin require import JModel.
-from JazzEC require import Array1152 Array1088 Array960 Array768 Array400 Array384 Array256 Array128 Array64 Array32 Array16 Array4 Array8.
-from JazzEC require import WArray512 WArray32 WArray16.
+from JazzEC require import Array1536 Array1568 Array1408 Array1410 Array1024 Array400 Array384 Array256 Array160 Array128 Array64 Array32 Array16 Array4 Array8 Array2.
+from JazzEC require import WArray512 WArray384 WArray32 WArray16 WArray1410 WArray160.
 
 require import AVX2_Ops W16extra.
-from JazzEC require import Jkem768.
-from JazzEC require import Jkem768_avx2.
+from JazzEC require import Jkem1024.
+from JazzEC require import Jkem1024_avx2.
 require import MLKEM_PolyVec_avx2_prevec.
 require import MLKEM_Poly_avx2_prevec.
 require import NTT_avx2.
@@ -23,7 +23,7 @@ require import MLKEM_PolyVec_avx2_vec.
 require import MLKEM_InnerPKE.
 require import MLKEMFCLib.
 
-import GFq Rq Symmetric Symmetric768 Serialization Serialization768 Sampling VecMat VecMat768 InnerPKE768 MLKEM768 Correctness768 Fq SignedReductions.
+import GFq Rq Symmetric Symmetric1024 Serialization Serialization1024 Sampling VecMat VecMat1024 InnerPKE1024 MLKEM1024 Correctness1024 Fq SignedReductions.
 
 import Zq.
 import ZModP.
@@ -37,83 +37,1594 @@ import MLKEM_PolyvecAVX.
 import MLKEM_PolyAVXVec.
 import MLKEM_PolyVecAVXVec.
 
-lemma polyvec_decompress_equiv :
-    equiv [Jkem768_avx2.M.__i_polyvec_decompress ~  Jkem768.M.__polyvec_decompress  :
-             rp{1} = ap{2}
-              ==>
-             ={res} /\
-             lift_array768 res{1} = lift_array768 res{2} /\
-             pos_bound768_cxq res{1} 0 768 1 /\
-             pos_bound768_cxq res{2} 0 768 1 ].
-admitted.
+require import Bindings.
 
-equiv compressequivvec_1 mem : 
- Jkem768_avx2.M.__polyvec_compress_1 ~  Jkem768.M.__i_polyvec_compress :
-     pos_bound768_cxq a{1} 0 768 2 /\
-     pos_bound768_cxq a{2} 0 768 2 /\
-    lift_array768 a{1} = lift_array768 a{2} /\ 
-    ={Glob.mem} /\ Glob.mem{1} = mem 
+
+import KMatrix Vector.
+
+from JazzEC require import WArray1568 WArray2048.
+require import Bindings BitEncoding.
+import BitChunking BS2Int.
+
+(********** BEGIN BDEP PROOF OF CSUBQ **************)
+
+lemma polyvec_csubq_avx2_ll :
+   islossless Jkem1024_avx2.M.__polyvec_csubq.
+by proc;inline *;do 5!(unroll for ^while);auto.
+qed.
+
+lemma poly_csubq_avx2_ll :
+   islossless Jkem1024_avx2.M._poly_csubq.
+by proc;inline *;unroll for ^while;auto.
+qed.
+
+op csubq_circuit(a : W16.t) : W16.t = 
+   if (a \ult W16.of_int 3329) then  a
+   else (W16_sub a (W16.of_int 3329)).
+
+lemma poly_csubq_avx2_corr_h (_aw : W16.t Array256.t):
+    hoare[ Jkem1024_avx2.M._poly_csubq  :
+             rp = _aw /\
+             pos_bound256_cxq rp 0 256 2 ==> 
+             lift_array256 res = lift_array256 _aw /\
+             pos_bound256_cxq res 0 256 1]. 
+proof.
+proc; inline *.
+proc change 1: (sliceget16_16_256 jqx16 0); 1: by auto.
+proc change ^while.1: (sliceget256_16_256 rp (i*256));1: by auto => /#.
+proc change ^while.9: (sliceset256_16_256 rp (i*256) r);1: by auto => /#.
+
+unroll for ^while.
+cfold ^i<-.
+wp -1. 
+bdep 16 16 [_aw] [rp] [rp] csubq_circuit pcond_reduced. 
+
+(* BDEP pre conseq *)
++ move => &hr />; rewrite flatten1 /= pre_lane_commute_in_aligned 1:/# //=.
+  rewrite allP /pos_bound1024_cxq /= => Hb. 
+  rewrite /pcond_reduced /= /tolist /= => x.
+  rewrite  mkseqP => He;elim He => /= i [ib?]; rewrite ultE /=.
+  have := Hb i; rewrite ib /= qE /=.
+  rewrite /to_sint /smod /=.
+  smt(W16.to_uint_cmp).
+
+(* BDEP post conseq *)
+
+(* We start with some boilerplate *)
+move => &hr [#]/= ->; rewrite /pos_bound256_cxq => Hb rr; rewrite /= !flatten1.
+rewrite !flattenK;1..4:smt(mapP W16.size_w2bits).
+rewrite -2!(map_comp) /(\o) /= -(map_comp W16.bits2w) /(\o).
+have -> := (eq_map (fun (x : W16.t) => W16.bits2w (w2bits x)) idfun);1: by move => ?/=/#.
+rewrite map_id.
+rewrite /lift_array256 /pos_bound256_cxq /= => H.
+rewrite -(Array256.to_listK witness rr) -H qE; split.
+
+rewrite tP => i ib.
+rewrite !mapiE 1,2:/# /= get_of_list 1:/# (nth_map witness); 1:smt(Array256.size_to_list).
+rewrite (Array256.get_to_list _aw i).
+rewrite /csubq_circuit ultE /W16_sub /=.
+move : (Hb i ib);rewrite /bpos16 qE /= /to_sint /smod /=.
+case (to_uint _aw.[i] < 3329) => *//;1:
+have ->/= : !32768 <= to_uint _aw.[i] by smt(W16.to_uint_cmp).
+rewrite to_uintB /=;1: by rewrite uleE => /#.
+have ->/= : !32768 <= to_uint _aw.[i] - 3329;  by smt(W16.to_uint_cmp).
+
+move => i ib.
+rewrite Array256.get_of_list 1:/# (nth_map witness); 1:smt(Array256.size_to_list).
+rewrite (nth_map witness) /=;1:smt(size_iota).
+rewrite nth_iota 1:/#.
+rewrite /csubq_circuit ultE /W16_sub /=.
+move : (Hb i ib);rewrite /bpos16 qE /= /to_sint /smod /=.
+case (to_uint _aw.[i] < 3329) => *//;1:
+have ->/= : !32768 <= to_uint _aw.[i] by smt(W16.to_uint_cmp).
+by smt(W16.to_uint_cmp).
+rewrite to_uintB /=;1: by rewrite uleE => /#.
+have ->/= : !32768 <= to_uint _aw.[i] - 3329;  by smt(W16.to_uint_cmp).
+qed.
+
+lemma poly_csubq_avx2_corr (_aw : W16.t Array256.t):
+    phoare[ Jkem1024_avx2.M._poly_csubq  :
+             rp = _aw /\
+             pos_bound256_cxq rp 0 256 2 ==> 
+             lift_array256 res = lift_array256 _aw /\
+             pos_bound256_cxq res 0 256 1] = 1%r
+  by conseq poly_csubq_avx2_ll (poly_csubq_avx2_corr_h _aw).
+
+
+lemma polyvec_csubq_avx2_corr_h (_aw : W16.t Array1024.t):
+    hoare[ Jkem1024_avx2.M.__polyvec_csubq  :
+             r = _aw /\
+             pos_bound1024_cxq r 0 1024 2 ==> 
+             lift_array1024 res = lift_array1024 _aw /\
+             pos_bound1024_cxq res 0 1024 1]. 
+proof.
+proc; inline *.
+proc change ^while.1: (init_256_16 (fun i0 => r.[256*i+i0]));1: by auto.
+proc change ^while.2: (sliceget16_16_256 jqx16 0); 1: by auto.
+proc change ^while.^while.1: (sliceget256_16_256 rp (i0*256));1: by auto => /#.
+proc change ^while.^while.9: (sliceset256_16_256 rp (i0*256) r0);1: by auto => /#.
+proc change ^while.6: (init_1024_16 (fun (i_0 : int) => if 256 * i <= i_0 < 256 * i + 256 then aux.[i_0 - 256 * i] else r.[i_0]));1: by auto. 
+
+do 5!(unroll for ^while).
+cfold ^i0<-.
+wp -2. 
+bdep 16 16 [_aw] [r] [r] csubq_circuit pcond_reduced. 
+
+(* BDEP pre conseq *)
++ move => &hr />; rewrite flatten1 /= pre_lane_commute_in_aligned 1:/# //=.
+  rewrite allP /pos_bound1024_cxq /= => Hb. 
+  rewrite /pcond_reduced /= /tolist /= => x.
+  rewrite  mkseqP => He;elim He => /= i [ib?]; rewrite ultE /=.
+  have := Hb i; rewrite ib /= qE /=.
+  rewrite /to_sint /smod /=.
+  smt(W16.to_uint_cmp).
+
+(* BDEP post conseq *)
+
+(* We start with some boilerplate *)
+move => &hr [#]/= ->; rewrite /pos_bound1024_cxq => Hb rr; rewrite /= !flatten1.
+rewrite !flattenK;1..4:smt(mapP W16.size_w2bits).
+rewrite -2!(map_comp) /(\o) /= -(map_comp W16.bits2w) /(\o).
+have -> := (eq_map (fun (x : W16.t) => W16.bits2w (w2bits x)) idfun);1: by move => ?/=/#.
+rewrite map_id.
+rewrite /lift_array1024 /pos_bound1024_cxq /= => H.
+rewrite -(Array1024.to_listK witness rr) -H qE; split.
+
+rewrite tP => i ib.
+rewrite !mapiE 1,2:/# /= get_of_list 1:/# (nth_map witness); 1:smt(Array1024.size_to_list).
+rewrite (Array1024.get_to_list _aw i).
+rewrite /csubq_circuit ultE /W16_sub /=.
+move : (Hb i ib);rewrite /bpos16 qE /= /to_sint /smod /=.
+case (to_uint _aw.[i] < 3329) => *//;1:
+have ->/= : !32768 <= to_uint _aw.[i] by smt(W16.to_uint_cmp).
+rewrite to_uintB /=;1: by rewrite uleE => /#.
+have ->/= : !32768 <= to_uint _aw.[i] - 3329;  by smt(W16.to_uint_cmp).
+
+move => i ib.
+rewrite Array1024.get_of_list 1:/# (nth_map witness); 1:smt(Array1024.size_to_list).
+rewrite (nth_map witness) /=;1:smt(size_iota).
+rewrite nth_iota 1:/#.
+rewrite /csubq_circuit ultE /W16_sub /=.
+move : (Hb i ib);rewrite /bpos16 qE /= /to_sint /smod /=.
+case (to_uint _aw.[i] < 3329) => *//;1:
+have ->/= : !32768 <= to_uint _aw.[i] by smt(W16.to_uint_cmp).
+by smt(W16.to_uint_cmp).
+rewrite to_uintB /=;1: by rewrite uleE => /#.
+have ->/= : !32768 <= to_uint _aw.[i] - 3329;  by smt(W16.to_uint_cmp).
+qed.
+
+lemma polyvec_csubq_avx2_corr (_aw : W16.t Array1024.t):
+    phoare[ Jkem1024_avx2.M.__polyvec_csubq  :
+             r = _aw /\
+             pos_bound1024_cxq r 0 1024 2 ==> 
+             lift_array1024 res = lift_array1024 _aw /\
+             pos_bound1024_cxq res 0 1024 1] = 1%r
+  by conseq polyvec_csubq_avx2_ll (polyvec_csubq_avx2_corr_h _aw).
+
+
+
+(********** END BDEP PROOF OF CSUBQ **************)
+
+
+lemma polyvec_decompress_ll :
+   islossless Jkem1024_avx2.M.__i_polyvec_decompress.
+by proc;inline *;unroll for ^while; do 4!(cfold ^inc<-; unroll for ^while);auto.
+qed.
+(********** BEGIN BDEP PROOF OF DECOMPRESS **************)
+
+op decompress11_circuit(c : W11.t) : W16.t = 
+  truncateu16 (srl_32 (((zeroextu11_32 c) * W32.of_int 3329) + W32.of_int 1024) (W32.of_int 11)).
+
+op pcond_true11(_: W11.t) = true.
+
+lemma init_id (rp0 : W8.t Array1568.t):
+  (Array1408.init ("_.[_]" (Array1408.init ("_.[_]" rp0)))) =
+    Array1408.init  ("_.[_]" rp0).
+rewrite tP => *.
+by rewrite initiE 1:/# /=.
+qed.
+
+lemma polyvec_decompress_corr_h (_aw : W8.t Array1408.t):
+    hoare[ Jkem1024_avx2.M.__i_polyvec_decompress :
+             Array1408.init (fun i => rp.[i]) = _aw ==> pos_bound1024_cxq res 0 1024 1 /\ lift_polyvec res = decompress_polyvec 11 (decode11_vec _aw)].
+proc; inline *.
+proc change 1: (sliceget16_16_256 jqx16 0); 1: by auto.
+proc change 2: (sliceget32_8_256 pvd_shufbidx_s 0); 1: by auto.
+proc change 3: (sliceget8_32_256 pvd_srlvdidx_s 0); 1: by auto.
+proc change 4: (sliceget4_64_256 pvd_srlvqidx_s 0); 1: by auto.
+proc change 5: (sliceget16_16_256 pvd_shift_s 0); 1: by auto.
+proc change ^while.^while.1 : (sliceget1568_8_256 rp ((352*k + 22*i)*8)); 1: by auto => /> /#.
+proc change ^while.^while.10 : (sliceset1024_16_256 r ((16 * k + i)*256) f); 1: by auto => /> /#.
+unroll for ^while.
+cfold ^inc<-.
+do 4!(unroll for ^while).
+cfold ^i<-.
+wp -3.
+bdep 11 16 [_aw[Array1408.t:0]] [rp[Array1408.t:0]] [r] decompress11_circuit pcond_true11. 
+
+(* BDEP pre conseq *)
++ move => &hr />; rewrite /pcond_true11 /=;split. 
+  + rewrite allP /#. 
+  have {2}<- := init_id rp{hr}; smt().
+
+(* BDEP post conseq *)
+
+(* We start with some boilerplate *)
+move => &hr [#]/= <- rr; rewrite /= !flatten1.
+rewrite init_id.
+move => H1; have H2 := post_lane_commute_out_aligned (to_list (Array1408.init ("_.[_]" rp{hr}))) (to_list rr) W8.w2bits W8.bits2w W11.w2bits W11.bits2w W16.w2bits W16.bits2w  decompress11_circuit 8 11 16 _ _ _ _ _ _ _ _ _ _ _ _ H1;1..12:
+smt(Array1408.size_to_list Array1024.size_to_list W16.bits2wK BVA_Top_Bindings_W11_t.oflistP).
+
+have H3 : 
+   map decompress11_circuit (map W11.bits2w (chunk 11 (flatten (map W8.w2bits (to_list (Array1408.init ("_.[_]" rp{hr}))))))) =
+   map (W16.of_int \o asint) (to_list (decompress_polyvec 11 (decode11_vec (Array1408.init ("_.[_]" rp{hr})))).[0] ++ 
+                              to_list (decompress_polyvec 11 (decode11_vec (Array1408.init ("_.[_]" rp{hr})))).[1] ++ 
+                              to_list (decompress_polyvec 11 (decode11_vec (Array1408.init ("_.[_]" rp{hr})))).[2] ++ 
+                              to_list (decompress_polyvec 11 (decode11_vec (Array1408.init ("_.[_]" rp{hr})))).[3])%Vector.
++ rewrite /decode11_vec /decompress_polyvec !map_cat !setvE !offunvE 1..4:/# /= !offunvK /vclamp /kvec /= /subarray256 /=.
+  apply (eq_from_nth witness).
+  + rewrite !size_map !size_cat !size_map !size_iota /max /=.
+     rewrite (EclibExtra.size_flatten' 8);1:smt(mapP W8.size_w2bits). 
+     by rewrite size_map size_to_list /=.
+  move => i.
+  rewrite !size_map size_iota.
+  rewrite (EclibExtra.size_flatten' 8);1:smt(mapP W8.size_w2bits). 
+   rewrite size_map size_to_list /max  /= => ib.
+  rewrite !nth_cat !size_map !size_cat !size_map !size_iota /max /=. 
+  case (i <256).
+  + move => ?;rewrite ifT 1:/# ifT 1:/#.
+    rewrite (nth_map witness).
+    + rewrite size_map size_chunk 1:/# (EclibExtra.size_flatten' 8);1:smt(mapP W8.size_w2bits). 
+      rewrite size_map size_to_list /= /#.
+    rewrite (nth_map []).
+    + rewrite  size_chunk 1:/# (EclibExtra.size_flatten' 8);1:smt(mapP W8.size_w2bits). 
+      rewrite size_map size_to_list /= /#.
+    rewrite (nth_map witness _ ((W16.of_int \o asint))) /=.
+    + rewrite size_to_list /= /#.
+   rewrite /(\o) /= mapiE 1:/# /= initiE 1:/# /=.  
+  rewrite /(\o) /decompress11_circuit -decompress_alt_decompress /decompress_alt //=.
+  rewrite get_of_list 1:/# /= qE /=.
+  have Hs := size_nth_chunk [] (flatten (map W8.w2bits (to_list(Array1408.init ("_.[_]" rp{hr}))))) i 11 _ _ => //.
+  + rewrite (EclibExtra.size_flatten' 8);1:smt(mapP W8.size_w2bits). 
+    by rewrite size_map size_to_list /#.
+  rewrite to_uint_eq to_uint_truncateu16 /= /srl_32 /= of_uintK /=;congr;congr.
+  have ? : 2^11 = 2048 by auto.
+  rewrite to_uint_shr //= /zeroextu11_32 to_uintD_small /=;1: by rewrite of_uintK /=; smt(modz_small W11.to_uint_cmp). 
+  rewrite of_uintK /= modz_small /=;1:by smt( W11.to_uint_cmp). 
+  rewrite /to_uint bits2wK 1:/# incoeffK qE /= /decode (nth_map [] _ bs2int) /=.
+  + rewrite size_chunk 1:/# size_BytesToBits size_to_list /= /#.
+  by smt(BS2Int.bs2int_ge0 BS2Int.bs2int_le2Xs modz_small W11.to_uint_cmp). 
+
+  case (i <512).
+  + move => ??;rewrite ifT 1:/#.
+    rewrite (nth_map witness).
+    + rewrite size_map size_chunk 1:/# (EclibExtra.size_flatten' 8);1:smt(mapP W8.size_w2bits). 
+      rewrite size_map size_to_list /= /#.
+    rewrite (nth_map []).
+    + rewrite  size_chunk 1:/# (EclibExtra.size_flatten' 8);1:smt(mapP W8.size_w2bits). 
+      rewrite size_map size_to_list /= /#.
+    rewrite (nth_map witness _ ((W16.of_int \o asint))) /=.
+    + rewrite size_to_list /= /#.
+   rewrite /(\o) /= mapiE 1:/# /= initiE 1:/# /=.  
+  rewrite /(\o) /decompress11_circuit -decompress_alt_decompress /decompress_alt //=.
+  rewrite get_of_list 1:/# /= qE /=.
+  have Hs := size_nth_chunk [] (flatten (map W8.w2bits (to_list (Array1408.init ("_.[_]" rp{hr}))))) i 11 _ _ => //.
+  + rewrite (EclibExtra.size_flatten' 8);1:smt(mapP W8.size_w2bits). 
+    by rewrite size_map size_to_list /#.
+  rewrite to_uint_eq to_uint_truncateu16 /= /srl_32 /= of_uintK /=;congr;congr.
+  have ? : 2^11 = 2048 by auto.
+  rewrite to_uint_shr //= /zeroextu11_32 to_uintD_small /=;1: by rewrite of_uintK /=; smt(modz_small W11.to_uint_cmp). 
+  rewrite of_uintK /= modz_small;1:by smt( W11.to_uint_cmp). 
+  rewrite /to_uint bits2wK 1:/# incoeffK qE /= /decode (nth_map [] _ bs2int) /=.
+  + rewrite size_chunk 1:/# size_BytesToBits size_to_list /= /#.
+  by smt(BS2Int.bs2int_ge0 BS2Int.bs2int_le2Xs modz_small W11.to_uint_cmp). 
+
+  case (i <768).
+  + move => ???.
+    rewrite (nth_map witness).
+    + rewrite size_map size_chunk 1:/# (EclibExtra.size_flatten' 8);1:smt(mapP W8.size_w2bits). 
+      rewrite size_map size_to_list /= /#.
+    rewrite (nth_map []).
+    + rewrite  size_chunk 1:/# (EclibExtra.size_flatten' 8);1:smt(mapP W8.size_w2bits). 
+      rewrite size_map size_to_list /= /#.
+    rewrite (nth_map witness _ ((W16.of_int \o asint))) /=.
+    + rewrite size_to_list /= /#.
+   rewrite /(\o) /= mapiE 1:/# /= initiE 1:/# /=.  
+  rewrite /(\o) /decompress11_circuit -decompress_alt_decompress /decompress_alt //=.
+  rewrite get_of_list 1:/# /= qE /=.
+  have Hs := size_nth_chunk [] (flatten (map W8.w2bits (to_list (Array1408.init ("_.[_]" rp{hr}))))) i 11 _ _ => //.
+  + rewrite (EclibExtra.size_flatten' 8);1:smt(mapP W8.size_w2bits). 
+    by rewrite size_map size_to_list /#.
+  rewrite to_uint_eq to_uint_truncateu16 /= /srl_32 /= of_uintK /=;congr;congr.
+  have ? : 2^11 = 2048 by auto.
+  rewrite to_uint_shr //= /zeroextu11_32 to_uintD_small /=;1: by rewrite of_uintK /=; smt(modz_small W11.to_uint_cmp). 
+  rewrite of_uintK /= modz_small;1:by smt( W11.to_uint_cmp). 
+  rewrite /to_uint bits2wK 1:/# incoeffK qE /= /decode (nth_map [] _ bs2int) /=.
+  + rewrite size_chunk 1:/# size_BytesToBits size_to_list /= /#.
+  by smt(BS2Int.bs2int_ge0 BS2Int.bs2int_le2Xs modz_small W11.to_uint_cmp). 
+
+  + move => ???.
+    rewrite (nth_map witness).
+    + rewrite size_map size_chunk 1:/# (EclibExtra.size_flatten' 8);1:smt(mapP W8.size_w2bits). 
+      rewrite size_map size_to_list /= /#.
+    rewrite (nth_map []).
+    + rewrite  size_chunk 1:/# (EclibExtra.size_flatten' 8);1:smt(mapP W8.size_w2bits). 
+      rewrite size_map size_to_list /= /#.
+    rewrite (nth_map witness _ ((W16.of_int \o asint))) /=.
+    + rewrite size_to_list /= /#.
+   rewrite /(\o) /= mapiE 1:/# /= initiE 1:/# /=.  
+  rewrite /(\o) /decompress11_circuit -decompress_alt_decompress /decompress_alt //=.
+  rewrite get_of_list 1:/# /= qE /=.
+  have Hs := size_nth_chunk [] (flatten (map W8.w2bits (to_list (Array1408.init ("_.[_]" rp{hr}))))) i 11 _ _ => //.
+  + rewrite (EclibExtra.size_flatten' 8);1:smt(mapP W8.size_w2bits). 
+    by rewrite size_map size_to_list /#.
+  rewrite to_uint_eq to_uint_truncateu16 /= /srl_32 /= of_uintK /=;congr;congr.
+  have ? : 2^11 = 2048 by auto.
+  rewrite to_uint_shr //= /zeroextu11_32 to_uintD_small /=;1: by rewrite of_uintK /=; smt(modz_small W11.to_uint_cmp). 
+  rewrite of_uintK /= modz_small;1:by smt( W11.to_uint_cmp). 
+  rewrite /to_uint bits2wK 1:/# incoeffK qE /= /decode (nth_map [] _ bs2int) /=.
+  + rewrite size_chunk 1:/# size_BytesToBits size_to_list /= /#.
+  by smt(BS2Int.bs2int_ge0 BS2Int.bs2int_le2Xs modz_small W11.to_uint_cmp). 
+
+
+split; last first.
++ rewrite eq_vectorP => i @/kvec ib.
+  rewrite /lift_polyvec /decompress_polyvec !setvE !offunvE 1..2:/# /= !offunvK /vclamp /kvec /= ib /=. 
+  case (3 = i) => Hi.
+  + rewrite tP => k kb. 
+    rewrite -Hi !mapiE 1,2:/# !initiE 1,2:/# /= /= -get_to_list H2 H3.
+  rewrite (nth_map witness);1: by smt(Array256.size_to_list size_cat).
+  rewrite (nth_cat witness).
+  + rewrite !size_cat !size_to_list /= ifF 1:/# /decompress_polyvec.
+    rewrite !setvE !offunvE 1:/# /=.
+    rewrite initiE 1:/# /= mapiE 1:/# initiE 1:/# /=.
+    rewrite get_of_list 1:/# /=.
+  pose c := (decompress 11 (nth 0 (decode 11 (to_list (Array1408.init ("_.[_]" rp{hr})))) (768 + k))).
+  rewrite of_sintK /= /smod /= ifF;1:smt(@Zq).
+  rewrite modz_small; smt(@Zq).  
+
+  case (2 = i) => Hi2.
+  + rewrite tP => k kb. 
+    rewrite -Hi2 !mapiE 1,2:/# !initiE 1,2:/# /= /= -get_to_list H2 H3.
+  rewrite (nth_map witness);1: by smt(Array256.size_to_list size_cat).
+  rewrite (nth_cat witness).
+  + rewrite !size_cat !size_to_list /= ifT 1:/# /decompress_polyvec.
+    rewrite !setvE !offunvE 1..3:/# /=  !offunvK /vclamp /= !ifT 1..6:/#.
+  rewrite (nth_cat witness).
+  + rewrite !size_cat !size_to_list /= ifF 1:/# /decompress_polyvec.
+    rewrite  mapiE 1:/# initiE 1:/# /= initiE 1:/# /=.
+    rewrite of_sintK /= /smod /= ifF;1:smt(@Zq).
+  pose c := decompress 11 (nth 0 (decode 11 (to_list (Array1408.init ("_.[_]" rp{hr})))) (512 + k)).
+  rewrite modz_small; smt(@Zq).  
+
+  case (1 = i) => Hi1.
+  + rewrite tP => k kb. 
+    rewrite -Hi1 !mapiE 1,2:/# !initiE 1,2:/# /= /= -get_to_list H2 H3.
+  rewrite (nth_map witness);1: by smt(Array256.size_to_list size_cat).
+  rewrite (nth_cat witness).
+  + rewrite !size_cat !size_to_list /= ifT 1:/# /decompress_polyvec.
+    rewrite !setvE !offunvE 1..3:/# /= !offunvK /vclamp /= !ifT 1..6:/#.
+  rewrite (nth_cat witness).
+  + rewrite !size_cat !size_to_list /= ifT 1:/# /decompress_polyvec.
+  rewrite (nth_cat witness).
+  + rewrite !size_to_list /= ifF 1:/# /decompress_polyvec.
+    rewrite  mapiE 1:/# initiE 1:/# /= initiE 1:/# /=.
+    rewrite of_sintK /= /smod /= ifF;1:smt(@Zq).
+    pose c := (decompress 11 (nth 0 (decode 11 (to_list (Array1408.init ("_.[_]" rp{hr})))) (256 + k))).
+  rewrite modz_small; smt(@Zq).  
+
+  have Hi3 :(0 = i) by smt().
+  + rewrite tP => k kb.
+    rewrite -Hi3 /= !mapiE 1,2:/# /= initiE 1:/# /= -( Array1024.get_to_list rr) H2 H3.
+  rewrite (nth_map witness);1: by smt(Array256.size_to_list size_cat).
+  rewrite (nth_cat witness).
+  + rewrite !size_cat !size_to_list /= ifT 1:/# /decompress_polyvec.
+    rewrite !setvE !offunvE 1..3:/# /= !offunvK /vclamp /= !ifT 1..6:/#.
+  rewrite (nth_cat witness).
+  + rewrite !size_cat !size_to_list /= ifT 1:/# /decompress_polyvec.
+  rewrite (nth_cat witness).
+  + rewrite !size_to_list /= ifT 1:/# /decompress_polyvec.
+    rewrite  mapiE 1:/# initiE 1:/# /= initiE 1:/# /=.
+    rewrite of_sintK /= /smod /= ifF;1:smt(@Zq).
+    pose c := (decompress 11 (nth 0 (decode 11 (to_list (Array1408.init ("_.[_]" rp{hr})))) (k))).
+  rewrite modz_small; smt(@Zq).  
+
+
+rewrite /pos_bound1024_cxq qE /= => k kb. 
+rewrite -get_to_list  H2 H3 /decompress_poly.
+rewrite (nth_map witness);1: by smt(size_cat Array256.size_to_list).
+rewrite (nth_cat witness) !size_cat !size_to_list /=. 
+rewrite (nth_cat witness) !size_cat !size_to_list /=. 
+rewrite (nth_cat witness)  !size_to_list /=. 
+rewrite /decompress_polyvec !setvE /= !offunvE 1..4:/# /= !offunvK /= /vclamp /kvec/=.
+case (k < 256).
++ move => *; rewrite ifT 1:/# .
+  rewrite mapiE 1:/# initiE 1:/# /=.
+  rewrite of_sintK /= /smod /= ifF;1:smt(@Zq).
+  rewrite modz_small; smt(@Zq).  
+case (k < 512).
++ move => *.
+  rewrite mapiE 1:/# initiE 1:/# /=.
+  rewrite of_sintK /= /smod /= ifF;1:smt(@Zq).
+  rewrite modz_small; smt(@Zq).  
+case (k < 768).
++ move => *.
+  rewrite mapiE 1:/# initiE 1:/# /=.
+  rewrite of_sintK /= /smod /= ifF;1:smt(@Zq).
+  rewrite modz_small; smt(@Zq).  
++ move => *.
+  rewrite mapiE 1:/# initiE 1:/# /=.
+  rewrite of_sintK /= /smod /= ifF;1:smt(@Zq).
+  rewrite modz_small; smt(@Zq).  
+
+qed.
+
+
+lemma polyvec_decompress_corr (_aw : W8.t Array1408.t):
+    phoare[ Jkem1024_avx2.M.__i_polyvec_decompress :
+             Array1408.init (fun i => rp.[i]) = _aw ==> pos_bound1024_cxq res 0 1024 1 /\ lift_polyvec res = decompress_polyvec 11 (decode11_vec _aw)] = 1%r
+ by conseq polyvec_decompress_ll (polyvec_decompress_corr_h _aw).
+
+lemma polyvec_decompress_equiv  :
+    equiv [Jkem1024_avx2.M.__i_polyvec_decompress ~  Jkem1024.M.__i_polyvec_decompress  :
+             Array1408.init(fun i => arg{1}.`2.[i]) =arg{2}.`2
+              ==>
+             lift_array1024 res{1} = lift_array1024 res{2} /\
+             pos_bound1024_cxq res{1} 0 1024 1 /\
+             pos_bound1024_cxq res{2} 0 1024 1 ].
+proc*. 
+ecall {2} (MLKEM_PolyVec.polyvec_decompress_corr ap{2}) => /=.
+ecall {1} (polyvec_decompress_corr (Array1408.init (fun (i : int) => rp{1}.[i]))).
++ auto => /> &1 r1 ? <- rr ?; rewrite /lift_array1024 /lift_polyvec /lift_array256 /subarray256 !eq_vectorP /kvec tP =>H i ib.
+  rewrite !mapiE 1,2:/# /=.
+  case (0<= i < 256) => Hi0.
+  + have  := (H 0 _);1:by auto.
+    rewrite !offunvE /= /kvec //= tP => Hi.
+    by have := (Hi i Hi0); rewrite !mapiE 1,2:/# /= initiE 1:/# /= initiE 1:/# /= /#.
+  case (256<= i < 512) => Hi1.
+  + have  := (H 1 _);1:by auto.
+    rewrite !offunvE /= /kvec //= tP => Hi.
+    have := (Hi (i - 256) _); 1:smt(). 
+    by rewrite !mapiE 1,2:/# /= initiE 1:/# /= initiE 1:/# /= /#.
+  case (512<= i < 768) => Hi2.
+  + have  := (H 2 _);1:by auto.
+    rewrite !offunvE /= /kvec //= tP => Hi.
+    have := (Hi (i - 512) _); 1:smt(). 
+    by rewrite !mapiE 1,2:/# /= initiE 1:/# /= initiE 1:/# /= /#.
+  have Hi3 :  (768<= i < 1024)  by smt().
+    have  := (H 3 _);1:by auto.
+    rewrite !offunvE /= /kvec //= tP => Hi.
+    have := (Hi (i - 768) _); 1:smt(). 
+    by rewrite !mapiE 1,2:/# /= initiE 1:/# /= initiE 1:/# /= /#.
+qed.
+
+(***********************)
+
+
+(********** BEGIN BDEP PROOF OF COMPRESS  **************)
+
+op compress11_circuit(a : W16.t) : W11.t = 
+   if (a \ult W16.of_int 3329) then  
+   truncate64_11 (srl_64 ((sll_64 (zeroextu64 a) (W64.of_int 11) + W64.of_int 1664) * W64.of_int 645084) (W64.of_int 31))
+   else 
+   truncate64_11 (srl_64 ((sll_64 (zeroextu64 (W16_sub a (W16.of_int 3329))) (W64.of_int 11) + W64.of_int 1664) * W64.of_int 645084) (W64.of_int 31)).
+
+abbrev keepodd11 = (W32.of_int 134152192).
+abbrev keepeven11 = (W32.of_int 2047).
+
+op VPMADDWD_alt(f0 m : W256.t) : W256.t =
+    if m <> (VPBROADCAST_4u64 (W64.of_int 576460756732608513)) then
+       VPMADDWD_256 f0 m
+    else 
+    let f2 = VPBROADCAST_8u32 keepodd11 in
+    let f1 = VPAND_256 f0 f2  in
+    let f2 = VPBROADCAST_8u32 keepeven11 in
+    let f0 = VPAND_256 f0 f2  in
+    let f1 = VPSRL_8u32 f1  (W128.of_int 5) in
+        VPOR_256 f0 f1.
+
+
+lemma keepeven_bits b: 
+  0 <= b < 32 =>
+   keepeven11.[b] <=> 0<=b<11.
+move => bb.
+have  : all (fun b => keepeven11.[b] <=> 0 <= b < 11) (iota_ 0 32); last by rewrite allP => H; move : (H b _); smt(mem_iota allP). 
+by rewrite /of_int  /int2bs /mkseq -iotaredE /=.
+qed.
+
+lemma keepodd_bits b: 
+  0 <= b < 32 =>
+   keepodd11.[b] <=> 16<=b<27.
+move => bb.
+have  : all (fun b => keepodd11.[b] <=> 16 <= b < 27) (iota_ 0 32); last by rewrite allP => H; move : (H b _); smt(mem_iota allP). 
+by rewrite /of_int  /int2bs /mkseq -iotaredE /=.
+qed.
+
+lemma lowbits_keep (f : W256.t) (i : int) (b : int) :
+  0 <= i < 16 => i %% 2 = 0 => 
+  0 <= b < 11 =>
+    (f \bits16 i).[b] = ((f \bits32 i%/2)  `&` keepeven11).[b].
+proof. 
+move => bi Hi Hb. 
+have H := W16u16.get_bits16 f (16*i + b) _;1:smt().
+have H0 := W8u32.get_bits32 f (16*i + b) _;1:smt().
+rewrite andE map2iE 1:/# /=.
+by smt(keepeven_bits).
+qed.
+
+lemma lowbits_drop (f : W256.t) (i : int) (b : int) :
+  0 <= i < 16 => i %% 2 = 0 => 
+  11 <= b < 16 =>
+  !((f \bits32 i%/2)  `&` keepeven11).[b].
+proof. 
+move => bi Hi Hb. 
+rewrite andE map2iE 1:/# /=.
+by smt(keepeven_bits).
+qed.
+
+lemma highbits_keep (f : W256.t) (i : int) (b : int) :
+  0 <= i < 16 => i %% 2 = 1 => 0 <= b < 11 =>
+    (f \bits16 i).[b] = ((f \bits32 i%/2)  `&` keepodd11).[b + 16].
+proof. 
+move => bi Hi Hb. 
+have H := W16u16.get_bits16 f (16*i + b) _;1:smt().
+have H0 := W8u32.get_bits32 f (16*i + b) _;1:smt().
+rewrite andE map2iE 1:/# /=.
+by smt(keepodd_bits).
+qed.
+
+lemma highbits_drop (f : W256.t) (i : int) (b : int) :
+  0 <= i < 16 => i %% 2 = 1 =>11 <= b < 15 =>
+    !((f \bits32 i%/2)  `&` keepodd11).[b + 16].
+proof. 
+move => bi Hi Hb. 
+rewrite andE map2iE 1:/# /=.
+by smt(keepodd_bits).
+qed.
+
+
+lemma lowbits_ofint_keep (f0 f1 : W16.t) b :
+  0 <= b < 11 =>
+  0<= to_sint f0 < 2048 =>
+  0<= to_sint f1 < 2048 =>
+  (W32.of_int (to_sint f0 + to_sint f1 * 2048)).[b] = f0.[b].
+move => ?.
+rewrite /to_sint /smod /= => ??.
+have  : all (fun b => (W32.of_int
+   ((if 32768 <= to_uint f0 then to_uint f0 - 65536 else to_uint f0) +
+    (if 32768 <= to_uint f1 then to_uint f1 - 65536 else to_uint f1) * 2048)).[b] =
+f0.[b]) (iota_ 0 11); last by rewrite allP => H; move : (H b _); smt(mem_iota allP). 
+ rewrite  /of_int /int2bs /mkseq -iotaredE /=;do split; rewrite get_to_uint /= /#.
+qed.
+
+lemma highbits_ofint_keep (f0 f1 : W16.t) b :
+  0<= to_sint f0 < 2048 =>
+  0<= to_sint f1 < 2048 =>
+  11 <= b < 22 =>
+  (W32.of_int (to_sint f0 + to_sint f1 * 2048)).[b] = f1.[b-11].
+move => ?.
+rewrite /to_sint /smod /= => ??.
+have  : all (fun b => (W32.of_int
+   ((if 32768 <= to_uint f0 then to_uint f0 - 65536 else to_uint f0) +
+    (if 32768 <= to_uint f1 then to_uint f1 - 65536 else to_uint f1) * 2048)).[b] =
+f1.[b - 11]) (iota_ 11 22); last by rewrite allP => H; move : (H b _); smt(mem_iota allP). 
+ rewrite  /of_int /int2bs /mkseq -iotaredE /=;do split; rewrite get_to_uint /=; smt(pow2_16 pow2_32). 
+qed.
+
+
+lemma highbits_ofint_drop (f0 f1 : W16.t) b :
+  0<= to_sint f0 < 2048 =>
+  0<= to_sint f1 < 2048 =>
+  22 <= b < 32 =>
+  !(W32.of_int (to_sint f0 + to_sint f1 * 2048)).[b].
+move => ?.
+rewrite /to_sint /smod /= => ??.
+have  : all (fun b => ! (W32.of_int
+     ((if 32768 <= to_uint f0 then to_uint f0 - 65536 else to_uint f0) +
+      (if 32768 <= to_uint f1 then to_uint f1 - 65536 else to_uint f1) * 2048)).[b]) (iota_ 22 32); last by rewrite allP => H; move : (H b _); smt(mem_iota allP). 
+ rewrite  /of_int /int2bs /mkseq -iotaredE /=;do split; smt(pow2_16 pow2_32). 
+qed.
+
+
+lemma unand (f : W256.t) (i : int) (b : int) :
+  0 <= i < 8 => 0<=b<32 =>
+   (W32.init (fun (j : int) => (f \bits32 i).[j + 5] /\ keepodd11.[j + 5])).[b] = ((f \bits32 i) `&` keepodd11).[b + 5].
+proof.
+move => ??.
+by rewrite initiE 1:/# /=.
+qed.
+
+lemma vpmaddwd_alt_corr (f0 shift2 : W256.t) :
+   (forall i, 0 <= i < 16 => 0<= to_sint (f0 \bits16 i) < 2^11) =>
+   VPMADDWD_256 f0 shift2 = VPMADDWD_alt f0 shift2.
++ move => /= H;rewrite /VPMADDWD_256 /VPMADDWD_alt /=. 
+  case (shift2 = VPBROADCAST_4u64 pvc_shift2_s);2: by auto. 
+  move => -> /=; rewrite /VPBROADCAST_4u64 /= -!(iotaredE) /=. 
+  pose f00 := (f0 \bits16 0).
+  pose f01 := (f0 \bits16 1).
+  pose f02 := (f0 \bits16 2).
+  pose f03 := (f0 \bits16 3).
+  pose f04 := (f0 \bits16 4).
+  pose f05 := (f0 \bits16 5).
+  pose f06 := (f0 \bits16 6).
+  pose f07 := (f0 \bits16 7).
+  pose f08 := (f0 \bits16 8).
+  pose f09 := (f0 \bits16 9).
+  pose f010 := (f0 \bits16 10).
+  pose f011 := (f0 \bits16 11).
+  pose f012 := (f0 \bits16 12).
+  pose f013 := (f0 \bits16 13).
+  pose f014 := (f0 \bits16 14).
+  pose f015 := (f0 \bits16 15).
+  rewrite  /(\bits16) /= !W16.init_bits2w -!iotaredE /= /W64.of_int /= /int2bs /mkseq -!iotaredE /=; do 16!(rewrite /(to_sint (W16.bits2w _)) /smod /= /(W16.to_uint (W16.bits2w (_::_)))). 
+  rewrite  !bits2wK //= !JUtils.bs2int_cons /b2i /= !bs2int_nil /=.
+  rewrite !hadd_cons2 hadd_nil /=.
+  rewrite /VPBROADCAST_8u32 -!iotaredE /= /VPSRL_8u32 /= /(`>>>`) /= -(unpack32K f0) andb8u32E !orb8u32E;congr;rewrite /unpack32 init_of_list -iotaredE /= orE.
+  congr;apply (eq_from_nth witness) => //= => i ib. 
+  apply W32.wordP => b bb. 
+  have /= H3 := highbits_keep f0 (i*2+1) (b-11) _ _;1,2: smt().
+  have /= H4 := highbits_drop f0 (i*2+1) (b-11) _ _;1,2: smt().
+  have /= H5 := lowbits_keep f0  (i*2) b _ _;1,2: smt().
+  have /= H6 := lowbits_drop f0 (i*2) b _ _;1,2: smt(). 
+  case (i = 0) => *.
+  + rewrite map2iE 1:/# unand 1,2:/#.
+    have /= H0 := highbits_ofint_drop f00 f01 b _ _;1,2:smt().
+    have /= H1 := highbits_ofint_keep f00 f01 b _ _;1,2:smt().
+    have /= H2 := lowbits_ofint_keep f00 f01 b.
+    smt(keepodd_bits keepeven_bits W32.get_out).
+  case (i - 1 = 0) => *.
+  + rewrite map2iE 1:/# unand 1,2:/#.
+    have /= H0 := highbits_ofint_drop f02 f03 b _ _;1,2:smt().
+    have /= H1 := highbits_ofint_keep f02 f03 b _ _;1,2:smt().
+    have /= H2 := lowbits_ofint_keep f02 f03 b.
+    smt(keepodd_bits keepeven_bits W32.get_out).
+  case (i - 2 = 0) => *.
+  + rewrite map2iE 1:/# unand 1,2:/#.
+    have /= H0 := highbits_ofint_drop f04 f05 b _ _;1,2:smt().
+    have /= H1 := highbits_ofint_keep f04 f05 b _ _;1,2:smt().
+    have /= H2 := lowbits_ofint_keep f04 f05 b.
+    smt(keepodd_bits keepeven_bits W32.get_out).
+  case (i - 3 = 0) => *.
+  + rewrite map2iE 1:/# unand 1,2:/#.
+    have /= H0 := highbits_ofint_drop f06 f07 b _ _;1,2:smt().
+    have /= H1 := highbits_ofint_keep f06 f07 b _ _;1,2:smt().
+    have /= H2 := lowbits_ofint_keep f06 f07 b.
+    smt(keepodd_bits keepeven_bits W32.get_out).
+  case (i - 4 = 0) => *.
+  + rewrite map2iE 1:/# unand 1,2:/#.
+    have /= H0 := highbits_ofint_drop f08 f09 b _ _;1,2:smt().
+    have /= H1 := highbits_ofint_keep f08 f09 b _ _;1,2:smt().
+    have /= H2 := lowbits_ofint_keep f08 f09 b.
+    smt(keepodd_bits keepeven_bits W32.get_out).
+  case (i - 5 = 0) => *.
+  + rewrite map2iE 1:/# unand 1,2:/#.
+    have /= H0 := highbits_ofint_drop f010 f011 b _ _;1,2:smt().
+    have /= H1 := highbits_ofint_keep f010 f011 b _ _;1,2:smt().
+    have /= H2 := lowbits_ofint_keep f010 f011 b.
+    smt(keepodd_bits keepeven_bits W32.get_out).
+  case (i - 6 = 0) => *.
+  + rewrite map2iE 1:/# unand 1,2:/#.
+    have /= H0 := highbits_ofint_drop f012 f013 b _ _;1,2:smt().
+    have /= H1 := highbits_ofint_keep f012 f013 b _ _;1,2:smt().
+    have /= H2 := lowbits_ofint_keep f012 f013 b.
+    smt(keepodd_bits keepeven_bits W32.get_out).
+  case (i - 7 = 0) => *.
+  + rewrite map2iE 1:/# unand 1,2:/#.
+    have /= H0 := highbits_ofint_drop f014 f015 b _ _;1,2:smt().
+    have /= H1 := highbits_ofint_keep f014 f015 b _ _;1,2:smt().
+    have /= H2 := lowbits_ofint_keep f014 f015 b.
+    smt(keepodd_bits keepeven_bits W32.get_out).
+by smt().
+qed.
+
+
+module AuxCompress11 = {
+ proc __i_polyvec_compress(rp : W8.t Array1410.t, a : W16.t Array1024.t) : W8.t Array1410.t = {
+    var inc : int;
+    var v : W256.t;
+    var v8 : W256.t;
+    var off : W256.t;
+    var shift1 : W256.t;
+    var mask : W256.t;
+    var shift2 : W256.t;
+    var sllvdidx : W256.t;
+    var srlvqidx : W256.t;
+    var shufbidx : W256.t;
+    var i : int;
+    var f0 : W256.t;
+    var f1 : W256.t;
+    var f2 : W256.t;
+    var t0 : W128.t;
+    var t1 : W128.t;
+    
+    a <@ M.__polyvec_csubq(a);
+    v <- get256 (WArray32.init16 (fun (i_0 : int) => jvx16.[i_0])) 0;
+    v8 <- VPSLL_16u16 v (W128.of_int 3);
+    off <- VPBROADCAST_16u16 pvc_off_s;
+    shift1 <- VPBROADCAST_16u16 pvc_shift1_s;
+    mask <- VPBROADCAST_16u16 pvc_mask_s;
+    shift2 <- VPBROADCAST_4u64 pvc_shift2_s;
+    sllvdidx <- VPBROADCAST_4u64 pvc_sllvdidx_s;
+    srlvqidx <- get256 (WArray32.init64 (fun (i_0 : int) => pvc_srlvqidx.[i_0])) 0;
+    shufbidx <- get256 (WArray32.init8 (fun (i_0 : int) => pvc_shufbidx_s.[i_0])) 0;
+    inc <- 4 * 256 %/ 16;
+    i <- 0;
+    while (i < inc){
+      f0 <- get256 (WArray2048.init16 (fun (i_0 : int) => a.[i_0])) i;
+      f1 <- VPMULL_16u16 f0 v8;
+      f2 <- VPADD_16u16 f0 off;
+      f0 <- VPSLL_16u16 f0 (W128.of_int 3);
+      f0 <- VPMULH_16u16 f0 v;
+      f2 <- VPSUB_16u16 f1 f2;
+      f1 <- invw f1 `&` f2;
+      f1 <- VPSRL_16u16 f1 (W128.of_int 15);
+      f0 <- VPSUB_16u16 f0 f1;
+      f0 <- VPMULHRS_16u16 f0 shift1;
+      f0 <- f0 `&` mask;
+      f2 <- VPBROADCAST_8u32 keepodd11;
+      f1 <- VPAND_256 f0 f2;
+      f2 <- VPBROADCAST_8u32 keepeven11;
+      f0 <- VPAND_256 f0 f2;
+      f1 <- VPSRL_8u32 f1  (W128.of_int 5);
+      f0 <- VPOR_256 f0 f1;
+      f0 <- VPSLLV_8u32 f0 sllvdidx;
+      f1 <- VPSRLDQ_256 f0 (W8.of_int 8);
+      f0 <- VPSRLV_4u64 f0 srlvqidx;
+      f1 <- VPSLL_4u64 f1 (W128.of_int 34);
+      f0 <- f0 `|` f1;
+      f0 <- VPSHUFB_256 f0 shufbidx;
+      t0 <- truncateu128 f0;
+      t1 <- VEXTRACTI128 f0 W8.one;
+      t0 <- BLENDV_16u8 t0 t1 (truncateu128 shufbidx);
+      rp <- Array1410.init (get8 (set128_direct (WArray1410.init8 (fun (i_0 : int) => rp.[i_0])) (22 * i) t0));
+      rp <-
+        Array1410.init
+          (get8 (set64_direct (WArray1410.init8 (fun (i_0 : int) => rp.[i_0])) (22 * i + 16) (truncateu64 t1)));
+      i <- i + 1;
+    }
+    
+    return rp;
+  }
+}.
+
+lemma auxcompress11_ll : islossless AuxCompress11.__i_polyvec_compress.
+proc. cfold 11. unroll for ^while; wp => /=. 
+inline *;unroll for ^while; do 4!(unroll for ^while);auto.
+qed.
+
+lemma auxcompress11_corr_h (_aw : W16.t Array1024.t):
+    hoare[ AuxCompress11.__i_polyvec_compress  :
+             a = _aw /\
+             pos_bound1024_cxq a 0 1024 2 ==> 
+      Array1408.init (fun i => res.[i])  = encode11_vec (compress_polyvec 11 (lift_polyvec _aw))].
+proof.
+proc; inline *.
+proc change ^while.1: (init_256_16 (fun i => r.[256*i0+i]));1: by auto.
+proc change ^while.2: (sliceget16_16_256 jqx16 0); 1: by auto.
+proc change ^while.^while.1: (sliceget256_16_256 rp0 (i1*256));1: by auto => /#.
+proc change ^while.^while.9: (sliceset256_16_256 rp0 (i1*256) r0);1: by auto => /#.
+proc change ^while.6: (init_1024_16 (fun (i_0 : int) => if 256 * i0 <= i_0 < 256 * i0 + 256 then aux.[i_0 - 256 * i0] else r.[i_0]));1: by auto. 
+proc change 5: (sliceget16_16_256 jvx16 0); 1: by auto.
+proc change ^while{2}.1: (sliceget1024_16_256 a (i*256));1: by auto => /#.
+proc change 12: (sliceget4_64_256 pvc_srlvqidx 0); 1: by auto.
+proc change 13: (sliceget32_8_256 pvc_shufbidx_s 0); 1: by auto.
+proc change ^while{2}.27 : (sliceset1410_8_128 rp  (22*i*8) t0);1: by auto => /#.
+proc change ^while{2}.28 : (sliceset1410_8_64 rp  ((22*i+16)*8) (truncateu64 t1)).
++ move => *;rewrite /sliceset1410_8_64 tP => *.
+  rewrite initiE /= 1:/# ifT 1:/# initiE 1:/#.
+  do congr;smt().
+unroll for ^while.
+do 4!(unroll for ^while).
+cfold ^inc<-.
+unroll for ^while.
+cfold ^i0<-. 
+cfold ^i1<-. 
+wp -4. 
+bdep 16 11 [_aw] [a] [rp[Array1408.t:0]] compress11_circuit pcond_reduced. 
+
+
+
+(* BDEP pre conseq *)
++ move => &hr />; rewrite flatten1 /= pre_lane_commute_in_aligned 1:/# //=.
+  rewrite allP /pos_bound1024_cxq /= => Hb. 
+  rewrite /pcond_reduced /= /tolist /= => x.
+  rewrite  mkseqP => He;elim He => /= i [ib?]; rewrite ultE /=.
+  have := Hb i; rewrite ib /= qE /=.
+  rewrite /to_sint /smod /=.
+  smt(W16.to_uint_cmp).
+
+(* BDEP post conseq *)
+
+(* We start with some boilerplate *)
+move => &hr [#]/= <- H0  rr; rewrite /= !flatten1.
+move => H1.
+
+apply (inj_eq Array1408.to_list Array1408.to_list_inj).
+apply (flatten_map_eq _ _ W8.w2bits 8 _ W8.w2bits_inj W8.size_w2bits);1:smt().
+have -> := post_lane_commute_in_aligned (to_list a{hr}) (to_list (Array1408.init ("_.[_]" rr))) W16.w2bits W16.bits2w W8.w2bits W8.bits2w W11.w2bits W11.bits2w  compress11_circuit 16 11 8 _ _ _ _ _ _ _ _ _ _ _ _ H1;1..12:
+    smt(Array1408.size_to_list Array1024.size_to_list W16.bits2wK BVA_Top_Bindings_W11_t.oflistP).
+
+rewrite output_pack_1408_8. 
++ rewrite (EclibExtra.size_flatten' 11);1: smt(mapP BS2Int.size_int2bs).
+  by rewrite size_map size_to_list /=.
+
+congr.
+rewrite /compress11_circuit /compress_polyvec /fromarray256  -map_comp -map_comp -map_comp /(\o) /=.  
+apply (eq_from_nth witness); 1: by rewrite !size_map //.
+rewrite size_map size_iota /max /= => i ib; rewrite !(nth_map witness) //=;1,2:smt(size_iota).
+rewrite nth_iota 1:/# mapiE 1:/# initiE 1:/# /= /lift_polyvec /=.
+case (0<=i<256).
++ move => ? /=.
+  rewrite  !getvE offunvE 1:/# /= -(BVA_Top_Bindings_W11_t.oflistP (int2bs 11 (compress 11 (lift_array256 (subarray256 a{hr} 0)).[i]))); 1: by rewrite BS2Int.size_int2bs /#.
+congr; rewrite -BVA_Top_Bindings_W11_t.ofintP /lift_array256 /subarray256 !mapiE 1:/# /= initiE 1:/# /=. 
+
+rewrite /truncate64_11 to_uint_eq.
+(* This is now the equivalence betwen specs. It's made slightly more verbose
+   because the impl circuit is only proved correct wrt compress for values
+   in the q range. *)
+rewrite ultE /=. 
+case (to_uint a{hr}.[i] < 3329) => /= *.
++ rewrite -Fq.compress_impl_large //=; 1: by rewrite /bpos16 qE /= /to_sint /smod /=;smt(W16.to_uint_cmp).     
+  rewrite /srl_64 /sll_64 /(`<<`) /(`>>`) !of_uintK /= /#. 
+have := H0;rewrite /pos_bound1024_cxq qE /= => H00.
+
+have ? : 0 <= to_sint ((W16_sub a{hr}.[i] (W16.of_int 3329))) < 3329.
++  rewrite /bpos16 to_sintB_small /=;1: by rewrite  /(to_sint (W16.of_int 3329)) /smod /= /smod /=;smt(size_map size_iota). 
+   by rewrite  /(to_sint (W16.of_int 3329)) /smod /=; smt(size_map size_iota W16.to_uint_cmp).
+
+have ? : to_sint ((W16_sub a{hr}.[i] (W16.of_int 3329))) = to_sint a{hr}.[i] -  3329.
++  rewrite to_sintB_small /=;1: by rewrite  /(to_sint (W16.of_int 3329)) /= /smod /=;smt(size_map size_iota). 
+   by rewrite  /(to_sint (W16.of_int 3329)) /= /smod /=; smt(size_map size_iota W16.to_uint_cmp).
+
+have -> : (incoeff (to_sint a{hr}.[i])) = (incoeff (to_sint (W16_sub a{hr}.[i] (W16.of_int 3329)))) by  rewrite -eq_incoeff;  smt().  
+
+rewrite -Fq.compress_impl_large //=;1:by smt().
+by rewrite /srl_64 /sll_64 /(`<<`) /(`>>`) !of_uintK /= /#. 
+
+case (256<=i<512).
++ move => ?? /=.
+  rewrite  !getvE offunvE 1:/# /= -(BVA_Top_Bindings_W11_t.oflistP (int2bs 11 (compress 11 (lift_array256 (subarray256 a{hr} 1)).[i-256]))); 1: by rewrite BS2Int.size_int2bs /#.
+congr; rewrite -BVA_Top_Bindings_W11_t.ofintP /lift_array256 /subarray256 !mapiE 1:/# /= initiE 1:/# /=. 
+
+rewrite /truncate64_11 to_uint_eq.
+(* This is now the equivalence betwen specs. It's made slightly more verbose
+   because the impl circuit is only proved correct wrt compress for values
+   in the q range. *)
+rewrite ultE /=. 
+case (to_uint a{hr}.[i] < 3329) => /= *.
++ rewrite -Fq.compress_impl_large //=; 1: by rewrite /bpos16 qE /= /to_sint /smod /=;smt(W16.to_uint_cmp).     
+  rewrite /srl_64 /sll_64 /(`<<`) /(`>>`) !of_uintK /= /#. 
+have := H0;rewrite /pos_bound1024_cxq qE /= => H00.
+
+have ? : 0 <= to_sint ((W16_sub a{hr}.[i] (W16.of_int 3329))) < 3329.
++  rewrite /bpos16 to_sintB_small /=;1: by rewrite  /(to_sint (W16.of_int 3329)) /= /smod /=;smt(size_map size_iota). 
+   by rewrite  /(to_sint (W16.of_int 3329))   /= /smod /=; smt(size_map size_iota W16.to_uint_cmp).
+
+have ? : to_sint ((W16_sub a{hr}.[i] (W16.of_int 3329))) = to_sint a{hr}.[i] -  3329.
++  rewrite to_sintB_small /=;1: by rewrite  /(to_sint (W16.of_int 3329))  /= /smod /=;smt(size_map size_iota). 
+   by rewrite  /(to_sint (W16.of_int 3329))  /= /smod /=; smt(size_map size_iota W16.to_uint_cmp).
+
+have -> : (incoeff (to_sint a{hr}.[i])) = (incoeff (to_sint (W16_sub a{hr}.[i] (W16.of_int 3329)))) by  rewrite -eq_incoeff;  smt().  
+
+rewrite -Fq.compress_impl_large //=;1:by smt().
+by rewrite /srl_64 /sll_64 /(`<<`) /(`>>`) !of_uintK /= /#. 
+
+case (512<=i<768).
++ move => ??? /=.
+  rewrite  !getvE offunvE 1:/# /= -(BVA_Top_Bindings_W11_t.oflistP (int2bs 11 (compress 11 (lift_array256 (subarray256 a{hr} 2)).[i-512]))); 1: by rewrite BS2Int.size_int2bs /#.
+congr; rewrite -BVA_Top_Bindings_W11_t.ofintP /lift_array256 /subarray256 !mapiE 1:/# /= initiE 1:/# /=. 
+
+rewrite /truncate64_11 to_uint_eq.
+(* This is now the equivalence betwen specs. It's made slightly more verbose
+   because the impl circuit is only proved correct wrt compress for values
+   in the q range. *)
+rewrite ultE /=. 
+case (to_uint a{hr}.[i] < 3329) => /= *.
++ rewrite -Fq.compress_impl_large //=; 1: by rewrite /bpos16 qE /= /to_sint /smod /=;smt(W16.to_uint_cmp).     
+  rewrite /srl_64 /sll_64 /(`<<`) /(`>>`) !of_uintK /= /#. 
+have := H0;rewrite /pos_bound1024_cxq qE /= => H00.
+
+have ? : 0 <= to_sint ((W16_sub a{hr}.[i] (W16.of_int 3329))) < 3329.
++  rewrite /bpos16 to_sintB_small /=;1: by rewrite  /(to_sint (W16.of_int 3329)) /= /smod /=;smt(size_map size_iota). 
+   by rewrite  /(to_sint (W16.of_int 3329)) /= /smod /=; smt(size_map size_iota W16.to_uint_cmp).
+
+have ? : to_sint ((W16_sub a{hr}.[i] (W16.of_int 3329))) = to_sint a{hr}.[i] -  3329.
++  rewrite to_sintB_small /=;1: by rewrite  /(to_sint (W16.of_int 3329)) /= /smod /=;smt(size_map size_iota). 
+   by rewrite  /(to_sint (W16.of_int 3329))  /= /smod /=; smt(size_map size_iota W16.to_uint_cmp).
+
+have -> : (incoeff (to_sint a{hr}.[i])) = (incoeff (to_sint (W16_sub a{hr}.[i] (W16.of_int 3329)))) by  rewrite -eq_incoeff;  smt().  
+
+rewrite -Fq.compress_impl_large //=;1:by smt().
+by rewrite /srl_64 /sll_64 /(`<<`) /(`>>`) !of_uintK /= /#. 
+
+ move => ??? /=.
+  rewrite  !getvE offunvE 1:/# /= -(BVA_Top_Bindings_W11_t.oflistP (int2bs 11 (compress 11 (lift_array256 (subarray256 a{hr} 3)).[i-768]))); 1: by rewrite BS2Int.size_int2bs /#.
+congr; rewrite -BVA_Top_Bindings_W11_t.ofintP /lift_array256 /subarray256 !mapiE 1:/# /= initiE 1:/# /=. 
+
+rewrite /truncate64_10 to_uint_eq.
+(* This is now the equivalence betwen specs. It's made slightly more verbose
+   because the impl circuit is only proved correct wrt compress for values
+   in the q range. *)
+rewrite ultE /=. 
+case (to_uint a{hr}.[i] < 3329) => /= *.
++ rewrite -Fq.compress_impl_large //=; 1: by rewrite /bpos16 qE /= /to_sint /smod /=;smt(W16.to_uint_cmp).     
+  rewrite /srl_64 /sll_64 /(`<<`) /(`>>`) !of_uintK /= /#. 
+have := H0;rewrite /pos_bound1024_cxq qE /= => H00.
+
+have ? : 0 <= to_sint ((W16_sub a{hr}.[i] (W16.of_int 3329))) < 3329.
++  rewrite /bpos16 to_sintB_small /=;1: by rewrite  /(to_sint (W16.of_int 3329)) /= /smod /=;smt(size_map size_iota). 
+   by rewrite  /(to_sint (W16.of_int 3329))  /= /smod /=; smt(size_map size_iota W16.to_uint_cmp).
+
+have ? : to_sint ((W16_sub a{hr}.[i] (W16.of_int 3329))) = to_sint a{hr}.[i] -  3329.
++  rewrite to_sintB_small /=;1: by rewrite  /(to_sint (W16.of_int 3329)) /= /smod /=;smt(size_map size_iota). 
+   by rewrite  /(to_sint (W16.of_int 3329))  /= /smod /=; smt(size_map size_iota W16.to_uint_cmp).
+
+have -> : (incoeff (to_sint a{hr}.[i])) = (incoeff (to_sint (W16_sub a{hr}.[i] (W16.of_int 3329)))) by  rewrite -eq_incoeff;  smt().  
+
+rewrite -Fq.compress_impl_large //=;1:by smt().
+by rewrite /srl_64 /sll_64 /(`<<`) /(`>>`) !of_uintK /= /#. 
+
+qed.
+
+(********** END BDEP PROOF OF COMPRESS **************)
+
+lemma auxcompress11_corr (_aw : W16.t Array1024.t):
+    phoare[ AuxCompress11.__i_polyvec_compress  :
+             a = _aw /\
+             pos_bound1024_cxq a 0 1024 2 ==> 
+      Array1408.init (fun i => res.[i])  = encode11_vec (compress_polyvec 11 (lift_polyvec _aw))] = 1%r 
+  by conseq auxcompress11_ll (auxcompress11_corr_h _aw).
+
+
+lemma polyvec_compress_avx2_ll : islossless Jkem1024_avx2.M.__i_polyvec_compress.
+proc. cfold 11. unroll for ^while; wp => /=. 
+inline *;unroll for ^while; do 4!(unroll for ^while);auto.
+qed.
+
+lemma polyvec_compress_avx2_corr (_aw : W16.t Array1024.t):
+    phoare[ Jkem1024_avx2.M.__i_polyvec_compress  :
+             a = _aw /\
+             pos_bound1024_cxq a 0 1024 2 ==> 
+      Array1408.init (fun i => res.[i])  = encode11_vec (compress_polyvec 11 (lift_polyvec _aw))] = 1%r.
+bypr => &m [->?].
+have <- : Pr[ AuxCompress11.__i_polyvec_compress(rp{m}, _aw) @ &m :
+   Array1408.init (fun (i : int) => res.[i]) = encode11_vec (compress_polyvec 11 (lift_polyvec _aw))] = 1%r
+   by byphoare (auxcompress11_corr _aw)  =>/=;1:smt().
+byequiv (: ={arg} /\ a{1} = _aw /\
+             pos_bound1024_cxq a{1} 0 1024 2 ==> ={res}) => //.
+proc. 
+seq 1 1 : (={rp,a} /\ pos_bound1024_cxq a{1} 0 1024 1).
++ ecall {1} (polyvec_csubq_avx2_corr a{1}). 
+  ecall {2} (polyvec_csubq_avx2_corr a{2}). 
+  auto => />; rewrite /pos_bound1024_cxq /lift_array1024 /= qE /= => ? rr1.
+  rewrite !tP;move =>  Hrr11 Hrr12 rr2.
+  rewrite !tP;move =>  Hrr21 Hrr22.
+  move => i ib. 
+  have := Hrr11 i ib; rewrite !mapiE 1,2:/# /=. 
+  have := Hrr12 i ib.  
+  have := Hrr21 i ib; rewrite !mapiE 1,2:/# /=. 
+  have := Hrr22 i ib.  
+  rewrite /to_sint /smod /=. 
+  move => Hrr11i Hrr12i Hrr21i Hrr22i.
+  have Hn1 : !(32768 <= to_uint rr2.[i]) by smt(W16.to_uint_cmp pow2_16).
+  have Hn2 : !(32768 <= to_uint rr1.[i]) by smt(W16.to_uint_cmp pow2_16).
+  have Hn3 : !(32768 <= to_uint _aw.[i]) by smt(W16.to_uint_cmp pow2_16).
+  move : Hrr11i Hrr12i Hrr21i Hrr22i; rewrite Hn1 Hn2 Hn3 /=.
+  move => Hrr11i Hrr12i Hrr21i Hrr22i.
+  move : Hrr12i; rewrite -Hrr22i -eq_incoeff.  
+  by rewrite !modz_small ?qE /= 1,2:/# to_uint_eq /#.
+
+cfold {1} ^inc<-. 
+cfold {2} ^inc<-. 
+sp 9 9.
+wp;while (#pre /\ ={i} /\ 0 <= i{1} <=64); last by auto.
+wp -1 -1; conseq (: _ ==> ={rp}); 1: by auto => /#.
+sim;conseq />.
+seq 10 10 : (#pre /\ ={f0}); 1: by conseq />;sim.
+auto => /> &1;rewrite vpmaddwd_alt_corr; last by rewrite /VPMADDWD_alt /=.
+move => i ib /=; rewrite /VPBROADCAST_16u16 /=.
+rewrite Montgomery16.bits16_W16u16 ib /= get_of_list 1:/# /= (nth_map witness) /=;1:smt(size_iota).
+have -> : 2047 = 2^11 -1 by auto.
+rewrite and_mod 1:/# /= /smod /= /#.
+qed.
+
+equiv compressequivvec  : 
+ Jkem1024_avx2.M.__i_polyvec_compress ~  Jkem1024.M.__i_polyvec_compress :
+     pos_bound1024_cxq a{1} 0 1024 2 /\
+     pos_bound1024_cxq a{2} 0 1024 2 /\
+    lift_array1024 a{1} = lift_array1024 a{2} 
     ==> 
-    ={Glob.mem,res} /\  Glob.mem{1} = mem.
-admitted.
+    res{2} = Array1408.init (fun i => res{1}.[i]).
+proc*.
+print MLKEM_PolyVec.
+ecall {2} (i_polyvec_compress_corr a{2}) => /=.
+ecall {1} (polyvec_compress_avx2_corr a{1}).
++ auto => /> &1 &2 ??? rr;rewrite !tP => H k kb. 
+   rewrite initiE 1:/# /= H 1:/# /encode11_vec get_of_list 1:/#;do 4!(congr). 
+   rewrite eq_vectorP => i ib.
+   rewrite tP => j jb.
+   smt(liftarrayvector).
+qed.
 
-lemma poly_decompress_equiv mem _p : 
-    equiv [Jkem768_avx2.M._poly_decompress ~  Jkem768.M._poly_decompress  :
-             valid_ptr _p 128 /\
-             Glob.mem{1} = mem /\ to_uint ap{1} = _p /\
-             ={Glob.mem,ap}
+(***************)
+
+(********** BEGIN BDEP PROOF OF DECOMPRESS **************)
+
+op decompress5_circuit(c : W5.t) : W16.t =
+  truncateu16 (srl_32 (((zeroextu5_32 c) * W32.of_int 3329) + W32.of_int 16) (W32.of_int 5)).
+op pcond_true5(_: W5.t) = true.
+
+lemma poly_decompress_ll : islossless Jkem1024_avx2.M._i_poly_decompress.
+ proc; inline *;wp. cfold 5; unroll for ^while;auto. 
+qed.
+
+lemma poly_decompress_corr_h (_a : W8.t Array160.t): 
+    hoare [Jkem1024_avx2.M._i_poly_decompress  :
+              arg.`2 = _a
               ==>
-             ={Glob.mem,res} /\ Glob.mem{1} = mem /\
+             lift_array256 res = decompress_poly 5 (decode5 _a) /\
+             pos_bound256_cxq res 0 256 1 ].
+proc; inline *.
+proc change 1: (sliceget16_16_256 jqx16 0); 1: by auto.
+proc change 2: (sliceget32_8_256 pd_jshufbidx 0); 1: by auto.
+proc change 3: (sliceget16_16_256 pd_mask_s 0); 1: by auto.
+proc change 4: (sliceget16_16_256 pd_shift_s 0); 1: by auto.
+proc change ^while.1 : (zeroextu128 (sliceget160_8_64 a ((10*i)*8)));1: by auto => /#.
+proc change ^while.10 : (sliceset256_16_256 rp (i*256) f);1: by auto => /#.
+proc change ^while.2: (sliceget160_8_16 a ((10*i+8)*8));1: by auto => /#.
+
+cfold 5.
+unroll for ^while.
+cfold ^i<-.
+wp -2.
+
+bdep 5 16 [_a] [a] [rp] decompress5_circuit pcond_true5. 
+
+(* BDEP pre conseq *)
++ by move => &hr />; rewrite allP /pcond_true5 /=. 
+
+(* BDEP post conseq *)
+
+(* We start with some boilerplate *)
+move => &hr [#]/= <- rr; rewrite /= !flatten1.
+move => H1; have H2 := post_lane_commute_out_aligned (to_list a{hr}) (to_list rr) W8.w2bits W8.bits2w W5.w2bits W5.bits2w W16.w2bits W16.bits2w  decompress5_circuit 8 5 16 _ _ _ _ _ _ _ _ _ _ _ _ H1;1..12:
+smt(Array160.size_to_list Array256.size_to_list W16.bits2wK BVA_Top_Bindings_W5_t.oflistP).
+
+have H3 : 
+   map decompress5_circuit (map W5.bits2w (chunk 5 (flatten (map W8.w2bits (to_list a{hr}))))) =
+   map (W16.of_int \o asint) (to_list (decompress_poly 5 (decode5 a{hr}))).
++ rewrite /decode5 /decompress_poly Array256.map_of_list Array256.of_listK;1:smt(size_map Array256.size_to_list).
+  rewrite /decode -map_comp  -(map_comp _ (decompress 5)) -(map_comp _ BS2Int.bs2int) /=.
+  apply eq_in_map => x xb. 
+  rewrite /(\o) /decompress5_circuit  -decompress_alt_decompress /decompress_alt //=.
+  have := size_nth_chunk [] (flatten (map W8.w2bits (to_list a{hr}))).
+  have := nthP witness (chunk 5 (flatten (map W8.w2bits (to_list a{hr})))) x.
+  rewrite xb /= => He;elim He; rewrite size_chunk //= => k*. 
+  have ? : size x = 5
+   by  have := size_nth_chunk witness (flatten (map W8.w2bits (to_list a{hr}))) k 5 =>/= /#.
+  rewrite qE to_uint_eq to_uint_truncateu16 /= /srl_32 /= of_uintK /=;congr;congr.
+  rewrite to_uint_shr //= /zeroextu5_32 to_uintD_small /=;1: by rewrite of_uintK /=;smt(modz_small W5.to_uint_cmp pow2_5). 
+  rewrite of_uintK /= modz_small;1:by smt( W5.to_uint_cmp pow2_5). 
+  rewrite /to_uint bits2wK 1:/# incoeffK qE /=. 
+  by smt(BS2Int.bs2int_ge0 BS2Int.bs2int_le2Xs modz_small W5.to_uint_cmp pow2_5). 
+
+split.
++ rewrite tP => i ib.
+  rewrite !mapiE 1,2:/# /= -get_to_list H2 H3 /decompress_poly.
+  rewrite (nth_map witness);1: by smt(Array256.size_to_list).
+  rewrite get_to_list /= /(\o) mapiE 1:/# /=.
+  pose c := (decompress 5 (decode5 a{hr}).[i]).
+  rewrite  /smod /= ifF;1:smt(@Zq).
+  rewrite modz_small; smt(@Zq).  
+
+rewrite /pos_bound256_cxq qE /= => k kb. 
+rewrite -get_to_list  H2 H3 /decompress_poly.
+  rewrite (nth_map witness);1: by smt(Array256.size_to_list).
+  rewrite get_to_list /= /(\o) mapiE 1:/# /=.
+  rewrite/= /smod /= ifF;1:smt(@Zq).
+  rewrite modz_small; smt(@Zq).  
+qed.
+(********** END BDEP PROOF OF DECOMPRESS **************)
+
+lemma poly_decompress_corr (_a : W8.t Array160.t): 
+    phoare [Jkem1024_avx2.M._i_poly_decompress  :
+              arg.`2 = _a
+              ==>
+             lift_array256 res = decompress_poly 5 (decode5 _a) /\
+             pos_bound256_cxq res 0 256 1 ] = 1%r
+  by conseq poly_decompress_ll (poly_decompress_corr_h _a).
+
+lemma poly_decompress_equiv  : 
+    equiv [Jkem1024_avx2.M._i_poly_decompress ~  Jkem1024.M._i_poly_decompress  :
+             a{1} = ap{2}
+              ==>
              lift_array256 res{1} = lift_array256 res{2} /\
              pos_bound256_cxq res{1} 0 256 1 /\
              pos_bound256_cxq res{2} 0 256 1 ].
-admitted.
+proc*.
+ecall{1} (poly_decompress_corr a{1}).
+ecall{2} (MLKEM_Poly.poly_decompress_corr ap{2}).
+auto => /> &1; rewrite /lift_array256 => rr1 H H0 rr2 H1 H2.
+rewrite tP in H.
+rewrite tP in H1.
+rewrite tP => i ib; rewrite H // H1 //.
+qed.
 
-equiv compressequiv_1 mem : 
- Jkem768_avx2.M._poly_compress_1 ~  Jkem768.M._i_poly_compress :
+
+(********** BEGIN BDEP PROOF OF COMPRESS  **************)
+op compress5_circuit(a : W16.t) : W5.t = 
+   if (a \ult W16.of_int 3329) then  
+   truncateu32_5 (srl_32 ((sll_32 (zeroextu32 a) (W32.of_int 5) + W32.of_int 1664) * W32.of_int 40318) (W32.of_int 27))
+   else 
+   truncateu32_5 (srl_32 ((sll_32 (zeroextu32 (W16_sub a (W16.of_int 3329))) (W32.of_int 5) + W32.of_int 1664) * W32.of_int 40318) (W32.of_int 27)).  
+
+lemma i_poly_compress_corr_ll : islossless Jkem1024_avx2.M._i_poly_compress.
+proof.
+proc; inline *.
+cfold 13.
+do 2!(unroll for ^while).
+auto.
+qed.
+
+lemma i_poly_compress_corr_h _aw  : 
+    hoare [Jkem1024_avx2.M._i_poly_compress  :
+             pos_bound256_cxq a 0 256 2 /\
+             a = _aw
+              ==>
+             res.`1 = encode5 (compress_poly 5 (lift_array256 _aw)) 
+             ].
+proof.
+proc; inline *.
+proc change 2: (sliceget16_16_256 jqx16 0); 1: by auto.
+proc change ^while.1: (sliceget256_16_256 rp0 (i0*256));1: by auto => /#.
+proc change ^while.9: (sliceset256_16_256 rp0 (i0*256) r);1: by auto => /#.
+proc change 6: (sliceget16_16_256 jvx16 0); 1: by auto.
+proc change 12: (sliceget32_8_256 pc_shufbidx_s 0); 1: by auto.
+proc change ^while{2}.1: (sliceget256_16_256 a (2*i*256));1: by auto => /#.
+proc change ^while{2}.2: (sliceget256_16_256 a ((2*i+1)*256));1: by auto => /#.
+proc change ^while{2}.18 : (sliceset160_8_128 rp  (20*i*8) t0);1: by auto => /#.
+proc change ^while{2}.19 : (sliceset160_8_32 rp  ((20*i+16)*8) (truncateu32 t1));1: by auto => /#.
+
+cfold 13.
+do 2!(unroll for ^while).
+cfold ^i0<-.
+wp -3.
+bdep 16 5 [_aw] [a] [rp] compress5_circuit pcond_reduced. 
+
+(* BDEP pre conseq *)
++ move => &hr />; rewrite flatten1 /= pre_lane_commute_in_aligned 1:/# //=.
+  rewrite allP /pos_bound256_cxq /= => Hb. 
+  rewrite /pcond_reduced /= /tolist /= => x.
+  rewrite  mkseqP => He;elim He => /= i [ib?]; rewrite ultE /=.
+  have := Hb i; rewrite ib /= qE /=.
+  rewrite /to_sint /smod /=.
+  smt(W16.to_uint_cmp).
+
+(* BDEP post conseq *)
+
+(* We start with some boilerplate *)
+move => &hr [#]/= H0 <- rr; rewrite /= !flatten1.
+move => H1.
+
+apply (inj_eq Array160.to_list Array160.to_list_inj).
+apply (flatten_map_eq _ _ W8.w2bits 8 _ W8.w2bits_inj W8.size_w2bits);1:smt().
+have -> := post_lane_commute_in_aligned (to_list a{hr}) (to_list rr) W16.w2bits W16.bits2w W8.w2bits W8.bits2w W5.w2bits W5.bits2w  compress5_circuit 16 5 8 _ _ _ _ _ _ _ _ _ _ _ _ H1;1..12:
+    smt(Array160.size_to_list Array256.size_to_list W16.bits2wK BVA_Top_Bindings_W5_t.oflistP).
+
+rewrite output_pack_160_8. 
++ rewrite (EclibExtra.size_flatten' 5);1: smt(mapP BS2Int.size_int2bs).
+  by rewrite size_map size_to_list /=.
+
+congr.
+rewrite /compress5_circuit /compress_poly -map_comp -map_comp -map_comp /(\o) /=.  
+apply (eq_from_nth witness); 1: by rewrite !size_map //.
+rewrite size_map size_iota /max /= => i ib; rewrite !(nth_map witness) //=;1,2:smt(size_iota).
+rewrite nth_iota 1:/# -(BVA_Top_Bindings_W5_t.oflistP (BS2Int.int2bs 5 (map (compress 5) (lift_array256 a{hr})).[i])); 1: by rewrite BS2Int.size_int2bs /#.
+congr; rewrite -BVA_Top_Bindings_W5_t.ofintP /lift_array256;rewrite !mapiE;1,2:smt().
+
+rewrite /truncateu4 to_uint_eq.
+(* This is now the equivalence betwen specs. It's made slightly more verbose
+   because the impl circuit is only proved correct wrt compress for values
+   in the q range. *)
+rewrite ultE /=. 
+case (to_uint a{hr}.[i] < 3329) => /= *.
++ rewrite -compress_impl5 //=;1: by rewrite /bpos16 qE /= /to_sint /smod /=;smt(W16.to_uint_cmp).     
+  by rewrite /srl_32 /sll_32 /(`<<`) /(`>>`) !of_uintK /= /#. 
+have := H0;rewrite /pos_bound256_cxq qE /= => H00.
+
+have ? : 0 <= to_sint ((W16_sub a{hr}.[i] (W16.of_int 3329))) < 3329.
++  rewrite /bpos16 to_sintB_small /=;1: by rewrite  /(to_sint (W16.of_int 3329)) /= /smod /=;smt(size_map size_iota). 
+   by rewrite  /(to_sint (W16.of_int 3329)) /= /smod /=; smt(size_map size_iota W16.to_uint_cmp).
+
+have ? : to_sint ((W16_sub a{hr}.[i] (W16.of_int 3329))) = to_sint a{hr}.[i] -  3329.
++  rewrite to_sintB_small /=;1: by rewrite  /(to_sint (W16.of_int 3329))   /= /smod /=;smt(size_map size_iota). 
+   by rewrite  /(to_sint (W16.of_int 3329))  /= /smod /=; smt(size_map size_iota W16.to_uint_cmp).
+
+have -> : (incoeff (to_sint a{hr}.[i])) = (incoeff (to_sint (W16_sub a{hr}.[i] (W16.of_int 3329)))) by  rewrite -eq_incoeff;  smt().  
+
+rewrite -compress_impl5 //=;1:by smt().
+by rewrite /srl_32 /sll_32 /(`<<`) /(`>>`) !of_uintK /= /#. 
+qed.
+
+(********** END BDEP PROOF OF COMPRESS **************)
+
+lemma i_poly_compress_corr _aw  : 
+    phoare [Jkem1024_avx2.M._i_poly_compress  :
+             pos_bound256_cxq a 0 256 2 /\
+             a = _aw
+              ==>
+             res.`1 = encode5 (compress_poly 5 (lift_array256 _aw)) 
+             ] = 1%r
+ by conseq i_poly_compress_corr_ll (i_poly_compress_corr_h _aw).
+
+equiv compressequiv_1 : 
+ Jkem1024_avx2.M._i_poly_compress ~  Jkem1024.M._i_poly_compress :
      pos_bound256_cxq a{1} 0 256 2 /\
      pos_bound256_cxq a{2} 0 256 2 /\
-    lift_array256 a{1} = lift_array256 a{2} /\ 
-    ={Glob.mem} /\ Glob.mem{1} = mem   
+    lift_array256 a{1} = lift_array256 a{2} 
     ==> 
-    ={Glob.mem} /\  Glob.mem{1} = mem /\
     res.`1{1} = res.`1{2}.
-admitted.
+proc*.
+ecall {1} (i_poly_compress_corr a{1}).
+ecall {2} (MLKEM_Poly.i_poly_compress_corr a{2}).
+auto => /> /#.
+qed.
 
-equiv compressequiv mem _p : 
- Jkem768_avx2.M._poly_compress ~  Jkem768.M._poly_compress :
-     pos_bound256_cxq a{1} 0 256 2 /\
-     pos_bound256_cxq a{2} 0 256 2 /\
-    lift_array256 a{1} = lift_array256 a{2} /\ 
-    ={Glob.mem,rp} /\ Glob.mem{1} = mem /\   valid_ptr _p 128 /\ _p = to_uint rp{1}
-    ==> 
-    ={Glob.mem} /\  touches mem Glob.mem{1} _p 128.
-admitted.
+(********** BEGIN BDEP PROOF OF FROMBYTES **************)
+
+from JazzEC require import WArray384.
+
+op frombytes_circuit(c : W12.t) : W16.t = 
+  zeroextu16 c.
+
+
+lemma polyvec_frombytes_ll : islossless Jkem1024_avx2.M.__i_polyvec_frombytes.
+proc; inline *;wp. 
+  while (0 <= i <= 4) (4-i); last by  auto =>  /> /#.
+move => *. cfold 3. unroll for ^while;auto => /> /#.
+qed.
+
+op  perm_nttunpackv(i : int) : int =  nth (-1) 
+  [0; 8; 16; 24; 32; 40; 48; 56; 64; 72; 80; 88; 96; 104; 112; 120; 1; 9; 17; 25; 33; 41; 49; 57; 65; 73; 81; 89; 97;
+     105; 113; 121; 2; 10; 18; 26; 34; 42; 50; 58; 66; 74; 82; 90; 98; 106; 114; 122; 3; 11; 19; 27; 35; 43; 51; 59;
+     67; 75; 83; 91; 99; 107; 115; 123; 4; 12; 20; 28; 36; 44; 52; 60; 68; 76; 84; 92; 100; 108; 116; 124; 5; 13; 21;
+     29; 37; 45; 53; 61; 69; 77; 85; 93; 101; 109; 117; 125; 6; 14; 22; 30; 38; 46; 54; 62; 70; 78; 86; 94; 102; 110;
+     118; 126; 7; 15; 23; 31; 39; 47; 55; 63; 71; 79; 87; 95; 103; 111; 119; 127; 128; 136; 144; 152; 160; 168; 176;
+     184; 192; 200; 208; 216; 224; 232; 240; 248; 129; 137; 145; 153; 161; 169; 177; 185; 193; 201; 209; 217; 225; 233;
+     241; 249; 130; 138; 146; 154; 162; 170; 178; 186; 194; 202; 210; 218; 226; 234; 242; 250; 131; 139; 147; 155; 163;
+     171; 179; 187; 195; 203; 211; 219; 227; 235; 243; 251; 132; 140; 148; 156; 164; 172; 180; 188; 196; 204; 212; 220;
+     228; 236; 244; 252; 133; 141; 149; 157; 165; 173; 181; 189; 197; 205; 213; 221; 229; 237; 245; 253; 134; 142; 150;
+     158; 166; 174; 182; 190; 198; 206; 214; 222; 230; 238; 246; 254; 135; 143; 151; 159; 167; 175; 183; 191; 199; 207;
+     215; 223; 231; 239; 247; 255; 256; 264; 272; 280; 288; 296; 304; 312; 320; 328; 336; 344; 352; 360; 368; 376; 257;
+     265; 273; 281; 289; 297; 305; 313; 321; 329; 337; 345; 353; 361; 369; 377; 258; 266; 274; 282; 290; 298; 306; 314;
+     322; 330; 338; 346; 354; 362; 370; 378; 259; 267; 275; 283; 291; 299; 307; 315; 323; 331; 339; 347; 355; 363; 371;
+     379; 260; 268; 276; 284; 292; 300; 308; 316; 324; 332; 340; 348; 356; 364; 372; 380; 261; 269; 277; 285; 293; 301;
+     309; 317; 325; 333; 341; 349; 357; 365; 373; 381; 262; 270; 278; 286; 294; 302; 310; 318; 326; 334; 342; 350; 358;
+     366; 374; 382; 263; 271; 279; 287; 295; 303; 311; 319; 327; 335; 343; 351; 359; 367; 375; 383; 384; 392; 400; 408;
+     416; 424; 432; 440; 448; 456; 464; 472; 480; 488; 496; 504; 385; 393; 401; 409; 417; 425; 433; 441; 449; 457; 465;
+     473; 481; 489; 497; 505; 386; 394; 402; 410; 418; 426; 434; 442; 450; 458; 466; 474; 482; 490; 498; 506; 387; 395;
+     403; 411; 419; 427; 435; 443; 451; 459; 467; 475; 483; 491; 499; 507; 388; 396; 404; 412; 420; 428; 436; 444; 452;
+     460; 468; 476; 484; 492; 500; 508; 389; 397; 405; 413; 421; 429; 437; 445; 453; 461; 469; 477; 485; 493; 501; 509;
+     390; 398; 406; 414; 422; 430; 438; 446; 454; 462; 470; 478; 486; 494; 502; 510; 391; 399; 407; 415; 423; 431; 439;
+     447; 455; 463; 471; 479; 487; 495; 503; 511; 512; 520; 528; 536; 544; 552; 560; 568; 576; 584; 592; 600; 608; 616;
+     624; 632; 513; 521; 529; 537; 545; 553; 561; 569; 577; 585; 593; 601; 609; 617; 625; 633; 514; 522; 530; 538; 546;
+     554; 562; 570; 578; 586; 594; 602; 610; 618; 626; 634; 515; 523; 531; 539; 547; 555; 563; 571; 579; 587; 595; 603;
+     611; 619; 627; 635; 516; 524; 532; 540; 548; 556; 564; 572; 580; 588; 596; 604; 612; 620; 628; 636; 517; 525; 533;
+     541; 549; 557; 565; 573; 581; 589; 597; 605; 613; 621; 629; 637; 518; 526; 534; 542; 550; 558; 566; 574; 582; 590;
+     598; 606; 614; 622; 630; 638; 519; 527; 535; 543; 551; 559; 567; 575; 583; 591; 599; 607; 615; 623; 631; 639; 640;
+     648; 656; 664; 672; 680; 688; 696; 704; 712; 720; 728; 736; 744; 752; 760; 641; 649; 657; 665; 673; 681; 689; 697;
+     705; 713; 721; 729; 737; 745; 753; 761; 642; 650; 658; 666; 674; 682; 690; 698; 706; 714; 722; 730; 738; 746; 754;
+     762; 643; 651; 659; 667; 675; 683; 691; 699; 707; 715; 723; 731; 739; 747; 755; 763; 644; 652; 660; 668; 676; 684;
+     692; 700; 708; 716; 724; 732; 740; 748; 756; 764; 645; 653; 661; 669; 677; 685; 693; 701; 709; 717; 725; 733; 741;
+     749; 757; 765; 646; 654; 662; 670; 678; 686; 694; 702; 710; 718; 726; 734; 742; 750; 758; 766; 647; 655; 663; 671;
+     679; 687; 695; 703; 711; 719; 727; 735; 743; 751; 759; 767; 768; 776; 784; 792; 800; 808; 816; 824; 832; 840; 848;
+     856; 864; 872; 880; 888; 769; 777; 785; 793; 801; 809; 817; 825; 833; 841; 849; 857; 865; 873; 881; 889; 770; 778;
+     786; 794; 802; 810; 818; 826; 834; 842; 850; 858; 866; 874; 882; 890; 771; 779; 787; 795; 803; 811; 819; 827; 835;
+     843; 851; 859; 867; 875; 883; 891; 772; 780; 788; 796; 804; 812; 820; 828; 836; 844; 852; 860; 868; 876; 884; 892;
+     773; 781; 789; 797; 805; 813; 821; 829; 837; 845; 853; 861; 869; 877; 885; 893; 774; 782; 790; 798; 806; 814; 822;
+     830; 838; 846; 854; 862; 870; 878; 886; 894; 775; 783; 791; 799; 807; 815; 823; 831; 839; 847; 855; 863; 871; 879;
+     887; 895; 896; 904; 912; 920; 928; 936; 944; 952; 960; 968; 976; 984; 992; 1000; 1008; 1016; 897; 905; 913; 921;
+     929; 937; 945; 953; 961; 969; 977; 985; 993; 1001; 1009; 1017; 898; 906; 914; 922; 930; 938; 946; 954; 962; 970;
+     978; 986; 994; 1002; 1010; 1018; 899; 907; 915; 923; 931; 939; 947; 955; 963; 971; 979; 987; 995; 1003; 1011;
+     1019; 900; 908; 916; 924; 932; 940; 948; 956; 964; 972; 980; 988; 996; 1004; 1012; 1020; 901; 909; 917; 925; 933;
+     941; 949; 957; 965; 973; 981; 989; 997; 1005; 1013; 1021; 902; 910; 918; 926; 934; 942; 950; 958; 966; 974; 982;
+     990; 998; 1006; 1014; 1022; 903; 911; 919; 927; 935; 943; 951; 959; 967; 975; 983; 991; 999; 1007; 1015; 1023] i. 
+
+op  perm_nttpackv(i : int) =  nth (-1) 
+  [0; 16; 32; 48; 64; 80; 96; 112; 1; 17; 33; 49; 65; 81; 97; 113; 2; 18; 34; 50; 66; 82; 98; 114; 3; 19; 35; 51;
+        67; 83; 99; 115; 4; 20; 36; 52; 68; 84; 100; 116; 5; 21; 37; 53; 69; 85; 101; 117; 6; 22; 38; 54; 70; 86; 102;
+        118; 7; 23; 39; 55; 71; 87; 103; 119; 8; 24; 40; 56; 72; 88; 104; 120; 9; 25; 41; 57; 73; 89; 105; 121; 10; 26;
+        42; 58; 74; 90; 106; 122; 11; 27; 43; 59; 75; 91; 107; 123; 12; 28; 44; 60; 76; 92; 108; 124; 13; 29; 45; 61;
+        77; 93; 109; 125; 14; 30; 46; 62; 78; 94; 110; 126; 15; 31; 47; 63; 79; 95; 111; 127; 128; 144; 160; 176; 192;
+        208; 224; 240; 129; 145; 161; 177; 193; 209; 225; 241; 130; 146; 162; 178; 194; 210; 226; 242; 131; 147; 163;
+        179; 195; 211; 227; 243; 132; 148; 164; 180; 196; 212; 228; 244; 133; 149; 165; 181; 197; 213; 229; 245; 134;
+        150; 166; 182; 198; 214; 230; 246; 135; 151; 167; 183; 199; 215; 231; 247; 136; 152; 168; 184; 200; 216; 232;
+        248; 137; 153; 169; 185; 201; 217; 233; 249; 138; 154; 170; 186; 202; 218; 234; 250; 139; 155; 171; 187; 203;
+        219; 235; 251; 140; 156; 172; 188; 204; 220; 236; 252; 141; 157; 173; 189; 205; 221; 237; 253; 142; 158; 174;
+        190; 206; 222; 238; 254; 143; 159; 175; 191; 207; 223; 239; 255; 256; 272; 288; 304; 320; 336; 352; 368; 257;
+        273; 289; 305; 321; 337; 353; 369; 258; 274; 290; 306; 322; 338; 354; 370; 259; 275; 291; 307; 323; 339; 355;
+        371; 260; 276; 292; 308; 324; 340; 356; 372; 261; 277; 293; 309; 325; 341; 357; 373; 262; 278; 294; 310; 326;
+        342; 358; 374; 263; 279; 295; 311; 327; 343; 359; 375; 264; 280; 296; 312; 328; 344; 360; 376; 265; 281; 297;
+        313; 329; 345; 361; 377; 266; 282; 298; 314; 330; 346; 362; 378; 267; 283; 299; 315; 331; 347; 363; 379; 268;
+        284; 300; 316; 332; 348; 364; 380; 269; 285; 301; 317; 333; 349; 365; 381; 270; 286; 302; 318; 334; 350; 366;
+        382; 271; 287; 303; 319; 335; 351; 367; 383; 384; 400; 416; 432; 448; 464; 480; 496; 385; 401; 417; 433; 449;
+        465; 481; 497; 386; 402; 418; 434; 450; 466; 482; 498; 387; 403; 419; 435; 451; 467; 483; 499; 388; 404; 420;
+        436; 452; 468; 484; 500; 389; 405; 421; 437; 453; 469; 485; 501; 390; 406; 422; 438; 454; 470; 486; 502; 391;
+        407; 423; 439; 455; 471; 487; 503; 392; 408; 424; 440; 456; 472; 488; 504; 393; 409; 425; 441; 457; 473; 489;
+        505; 394; 410; 426; 442; 458; 474; 490; 506; 395; 411; 427; 443; 459; 475; 491; 507; 396; 412; 428; 444; 460;
+        476; 492; 508; 397; 413; 429; 445; 461; 477; 493; 509; 398; 414; 430; 446; 462; 478; 494; 510; 399; 415; 431;
+        447; 463; 479; 495; 511; 512; 528; 544; 560; 576; 592; 608; 624; 513; 529; 545; 561; 577; 593; 609; 625; 514;
+        530; 546; 562; 578; 594; 610; 626; 515; 531; 547; 563; 579; 595; 611; 627; 516; 532; 548; 564; 580; 596; 612;
+        628; 517; 533; 549; 565; 581; 597; 613; 629; 518; 534; 550; 566; 582; 598; 614; 630; 519; 535; 551; 567; 583;
+        599; 615; 631; 520; 536; 552; 568; 584; 600; 616; 632; 521; 537; 553; 569; 585; 601; 617; 633; 522; 538; 554;
+        570; 586; 602; 618; 634; 523; 539; 555; 571; 587; 603; 619; 635; 524; 540; 556; 572; 588; 604; 620; 636; 525;
+        541; 557; 573; 589; 605; 621; 637; 526; 542; 558; 574; 590; 606; 622; 638; 527; 543; 559; 575; 591; 607; 623;
+        639; 640; 656; 672; 688; 704; 720; 736; 752; 641; 657; 673; 689; 705; 721; 737; 753; 642; 658; 674; 690; 706;
+        722; 738; 754; 643; 659; 675; 691; 707; 723; 739; 755; 644; 660; 676; 692; 708; 724; 740; 756; 645; 661; 677;
+        693; 709; 725; 741; 757; 646; 662; 678; 694; 710; 726; 742; 758; 647; 663; 679; 695; 711; 727; 743; 759; 648;
+        664; 680; 696; 712; 728; 744; 760; 649; 665; 681; 697; 713; 729; 745; 761; 650; 666; 682; 698; 714; 730; 746;
+        762; 651; 667; 683; 699; 715; 731; 747; 763; 652; 668; 684; 700; 716; 732; 748; 764; 653; 669; 685; 701; 717;
+        733; 749; 765; 654; 670; 686; 702; 718; 734; 750; 766; 655; 671; 687; 703; 719; 735; 751; 767; 768; 784; 800;
+        816; 832; 848; 864; 880; 769; 785; 801; 817; 833; 849; 865; 881; 770; 786; 802; 818; 834; 850; 866; 882; 771;
+        787; 803; 819; 835; 851; 867; 883; 772; 788; 804; 820; 836; 852; 868; 884; 773; 789; 805; 821; 837; 853; 869;
+        885; 774; 790; 806; 822; 838; 854; 870; 886; 775; 791; 807; 823; 839; 855; 871; 887; 776; 792; 808; 824; 840;
+        856; 872; 888; 777; 793; 809; 825; 841; 857; 873; 889; 778; 794; 810; 826; 842; 858; 874; 890; 779; 795; 811;
+        827; 843; 859; 875; 891; 780; 796; 812; 828; 844; 860; 876; 892; 781; 797; 813; 829; 845; 861; 877; 893; 782;
+        798; 814; 830; 846; 862; 878; 894; 783; 799; 815; 831; 847; 863; 879; 895; 896; 912; 928; 944; 960; 976; 992;
+        1008; 897; 913; 929; 945; 961; 977; 993; 1009; 898; 914; 930; 946; 962; 978; 994; 1010; 899; 915; 931; 947;
+        963; 979; 995; 1011; 900; 916; 932; 948; 964; 980; 996; 1012; 901; 917; 933; 949; 965; 981; 997; 1013; 902;
+        918; 934; 950; 966; 982; 998; 1014; 903; 919; 935; 951; 967; 983; 999; 1015; 904; 920; 936; 952; 968; 984;
+        1000; 1016; 905; 921; 937; 953; 969; 985; 1001; 1017; 906; 922; 938; 954; 970; 986; 1002; 1018; 907; 923; 939;
+        955; 971; 987; 1003; 1019; 908; 924; 940; 956; 972; 988; 1004; 1020; 909; 925; 941; 957; 973; 989; 1005; 1021;
+        910; 926; 942; 958; 974; 990; 1006; 1022; 911; 927; 943; 959; 975; 991; 1007; 1023] i. 
+
+lemma perm_nttunpackv_rng i :
+  0 <= i < 1024 => 0<= perm_nttunpackv i <1024.
+proof.
+  have : all (fun i => 0 <= perm_nttunpackv i < 1024) (iota_ 0 1024).
+  + by rewrite /perm_nttunpackv  -iotaredE /=.
+  move => H Hi; rewrite allP in H; move : (H i _);by smt(mem_iota). 
+qed.
+
+lemma perm_nttpackv_rng i :
+  0 <= i < 1024 => 0<= perm_nttpackv i <1024.
+proof.
+  have : all (fun i => 0 <= perm_nttpackv i < 1024) (iota_ 0 1024).
+  + by rewrite /perm_nttpackv  -iotaredE /=.
+  move => H Hi; rewrite allP in H; move : (H i _);by smt(mem_iota). 
+qed. 
+
+
+lemma post_lane_commute_out_aligned_perm ['a 'b 'c]
+    (lic : 'a list) 
+    (lo : 'c list) 
+    (tobitsic : 'a -> bool list)
+    (ofbitsic : bool list -> 'a)
+    (tobitsi : 'b -> bool list)
+    (ofbitsi : bool list -> 'b)
+    (tobitso : 'c -> bool list)
+    (ofbitso : bool list -> 'c)
+    (f : 'b -> 'c)
+    (nic ni no  : int) 
+    (perm : int -> int)
+    (permi : int -> int):
+  0 < nic =>  0 < ni => 0 < no => 
+  ni %| nic*size lic =>
+  size lo = (nic*size lic) %/ ni =>
+  (forall x, size (tobitsic x) = nic) =>
+  (forall x, ofbitsic (tobitsic x) = x) =>
+  (forall x, size (tobitsi x) = ni) =>
+  (forall x, ofbitsi (tobitsi x) = x) =>
+  (forall x, size x = ni => tobitsi (ofbitsi x) = x) =>
+  (forall x, size (tobitso x) = no) =>
+  (forall x, ofbitso (tobitso x) = x) =>
+  (forall ii, 0 <= ii < size lo => 0 <= perm ii < size lo) =>
+  (forall ii, 0 <= ii < size lo => permi (perm ii) = ii) =>
+map f (map ofbitsi (chunk ni (flatten (map tobitsic lic)))) =
+mkseq (fun (i1 : int) => nth witness
+(map ofbitso (chunk no (flatten (map tobitso lo)))) (permi i1)) 
+   (size (map ofbitso (chunk no (flatten (map tobitso lo))))) => 
+   lo =
+   mkseq (fun (i1 : int) => nth witness 
+      (map f (map ofbitsi (chunk ni (flatten (map tobitsic lic)))))
+         (perm i1)) (size ((map f (map ofbitsi (chunk ni (flatten (map tobitsic lic))))))).
+move => ??????????????; rewrite  !map_chunk_flatten_id 1..3:/#.
+move => H.
+apply (eq_from_nth witness).
++ rewrite size_mkseq. 
+  rewrite !size_map size_iota (EclibExtra.size_flatten' nic);1:smt(mapP).
+  rewrite size_map; smt(size_ge0).   
+move => i ib.
+rewrite nth_mkseq /=.
++ rewrite !size_map size_iota (EclibExtra.size_flatten' nic);1:smt(mapP).
+  rewrite size_map; smt(size_ge0).   
+rewrite H.
+rewrite nth_mkseq /=;1,2:smt().
+qed.
+
+lemma nttpermsK i :
+ 0 <= i < 1024 => 
+   perm_nttpackv (perm_nttunpackv i) = i.
+proof.
+move => Hi.
+have : all (fun i => perm_nttpackv (perm_nttunpackv i) = i) (iota_ 0 1024); 
+  last by rewrite allP /= => H; rewrite H; smt(mem_iota).
+rewrite  /perm_nttunpackv /perm_nttpackv /nttpackv /nttunpackv.
+rewrite /nttpack /nttunpack /subarray256 -iotaredE /=;do split;smt().
+qed. 
+
+lemma nttpermsKi i :
+ 0 <= i < 1024 => 
+   perm_nttunpackv (perm_nttpackv i) = i.
+proof.
+move => Hi.
+have : all (fun i => perm_nttunpackv (perm_nttpackv i) = i) (iota_ 0 1024); 
+  last by rewrite allP /= => H; rewrite H; smt(mem_iota).
+rewrite  /perm_nttunpackv /perm_nttpackv /nttpackv /nttunpackv.
+rewrite /nttpack /nttunpack /subarray256 -iotaredE /=;do split;smt().
+qed. 
+
+lemma polyvec_frombytes_corr_h (_aw : W8.t Array1536.t): 
+    hoare [Jkem1024_avx2.M.__i_polyvec_frombytes  :
+             a = _aw
+              ==>
+             lift_array1024 res = nttunpackv (map incoeff (decode12_vec _aw))  /\
+             pos_bound1024_cxq res 0 1024  2].
+proc; inline *.
+proc change ^while.1: (init_256_16 (fun (i_0 : int) => r.[256 * i + i_0])); 1: by auto.
+proc change ^while.2: (init_384_8 (fun (i_0 : int) => a.[384 * i + i_0])  ); 1: by auto.
+proc change ^while.3: (sliceget16_16_256 maskx16 0); 1: by auto.
+proc change ^while.^while.1 : (sliceget384_8_256 ap (192*i0*8)); 1: by auto => /> /#.
+proc change ^while.^while.2 : (sliceget384_8_256 ap ((192*i0+32)*8)); 1: by auto => /> /#.
+proc change ^while.^while.3 : (sliceget384_8_256 ap ((192*i0+64)*8)); 1: by auto => /> /#.
+proc change ^while.^while.4 : (sliceget384_8_256 ap ((192*i0+96)*8)); 1: by auto => /> /#.
+proc change ^while.^while.5 : (sliceget384_8_256 ap ((192*i0+128)*8)); 1: by auto => /> /#.
+proc change ^while.^while.6 : (sliceget384_8_256 ap ((192*i0+160)*8)); 1: by auto => /> /#.
+proc change ^while.^while.101 : (sliceset256_16_256 rp (8*i0 *256) t6);1: by auto => /> /#.
+proc change ^while.^while.102 : (sliceset256_16_256 rp ((8*i0+1) *256) t7);1: by auto => /> /#.
+proc change ^while.^while.103 : (sliceset256_16_256 rp ((8*i0+2) *256) t8);1: by auto => /> /#.
+proc change ^while.^while.104 : (sliceset256_16_256 rp ((8*i0+3) *256) t9);1: by auto => /> /#.
+proc change ^while.^while.105 : (sliceset256_16_256 rp ((8*i0+4) *256) t4);1: by auto => /> /#.
+proc change ^while.^while.106 : (sliceset256_16_256 rp ((8*i0+5) *256) t10);1: by auto => /> /#.
+proc change ^while.^while.107 : (sliceset256_16_256 rp ((8*i0+6) *256) t11);1: by auto => /> /#.
+proc change ^while.^while.108 : (sliceset256_16_256 rp ((8*i0+7) *256) tt);1: by auto => /> /#.
+proc change ^while.7: (init_1024_16 (fun (i_0 : int) => if 256 * i <= i_0 < 256 * i + 256 then aux.[i_0 - 256 * i] else r.[i_0])); 1: by auto.
+
+unroll for ^while.
+do 4!(unroll for ^while).
+cfold ^i0<-.
+wp -2. 
+
+bdep 12 16 [_aw] [a] [r] frombytes_circuit pcond_true12 perm_nttpackv. 
+
+(* BDEP pre conseq *)
++ by move => &hr />; rewrite allP /pcond_true12 /=. 
+
+(* BDEP post conseq *)
+
+(* We start with some boilerplate *)
+move => &hr [#]/= <- rr; rewrite /= !flatten1.
+
+move => H1; have H2 := post_lane_commute_out_aligned_perm (to_list a{hr}) (to_list rr) W8.w2bits W8.bits2w W12.w2bits W12.bits2w W16.w2bits W16.bits2w  frombytes_circuit 8 12 16 perm_nttunpackv perm_nttpackv _ _ _ _ _ _ _ _ _ _ _ _ _ _ _;1..12:
+smt(Array1536.size_to_list Array1024.size_to_list W16.bits2wK BVA_Top_Bindings_W12_t.oflistP).
++ smt(perm_nttunpackv_rng Array1024.size_to_list).
++ move => ?; rewrite Array1024.size_to_list => ?;smt(nttpermsK). 
+
+  have /=? := decode_range_vec 0 (to_list a{hr}) 12 _ _;1,2:smt(Array1536.size_to_list).
+
++ by smt().
+
+have H3 : 
+  map frombytes_circuit (map W12.bits2w (chunk 12 (flatten (map W8.w2bits (to_list a{hr}))))) =
+   to_list (map W16.of_int  (decode12_vec a{hr})).
++ rewrite /decode12_vec Array1024.map_of_list Array1024.of_listK;1:by rewrite !size_map /decode size_iota size_BytesToBits size_to_list /#.
+  rewrite /decode -map_comp -(map_comp _ BS2Int.bs2int) /=.
+  apply eq_in_map => x xb.
+  rewrite /(\o) /frombytes_circuit /zeroextu16.
+  have ? : size x = 12 by smt(@BitChunking).
+  congr;rewrite /to_uint W12.bits2wK;1 :  by smt(@BitChunking).
+  done.
+
+split.
++ rewrite tP => i ib.
+  rewrite mapiE 1:/# /= initiE 1:/# /=.
+  case (0<=i<256) => *.
+  + rewrite /nttunpack initiE 1:/# /= /subarray256 initiE /=;1:smt( nttunpack_inbounds).
+    rewrite mapiE /=;1:smt( nttunpack_inbounds).
+    rewrite -(Array1024.get_to_list rr) H2 H3 /decode12.
+    rewrite nth_mkseq /=;1: by smt(Array1024.size_to_list).
+    + rewrite  mapiE;1: by smt(perm_nttunpackv_rng).
+    congr; rewrite of_sintK /=.
+     rewrite /smod /= ifF. 
+     + rewrite /decode12_vec get_of_list;1: smt(perm_nttunpackv_rng). 
+       by have /= := decode_rng (to_list a{hr}) 12 (perm_nttunpackv i) _;smt(). 
+    rewrite modz_small. 
+    + rewrite /decode12_vec get_of_list; 1: smt(perm_nttunpackv_rng).
+       by have /= := decode_rng (to_list a{hr}) 12 (perm_nttunpackv i) _;smt(). 
+    rewrite /perm_nttunpackv /nttunpackv initiE 1:/# /= /#.
+
+  case (256<=i<512) => *.
+  + rewrite /nttunpack initiE 1:/# /= /subarray256 initiE /=;1:smt( nttunpack_inbounds).
+    rewrite mapiE /=;1:smt( nttunpack_inbounds).
+    rewrite -(Array1024.get_to_list rr) H2 H3 /decode12.
+    rewrite nth_mkseq /=;1: by smt(Array1024.size_to_list).
+    + rewrite  mapiE;1: by smt(perm_nttunpackv_rng).
+    congr; rewrite of_sintK /=.
+     rewrite /smod /= ifF. 
+     + rewrite /decode12_vec get_of_list;1: smt(perm_nttunpackv_rng). 
+       by have /= := decode_rng (to_list a{hr}) 12 (perm_nttunpackv i) _;smt(). 
+    rewrite modz_small. 
+    + rewrite /decode12_vec get_of_list; 1: smt(perm_nttunpackv_rng).
+       by have /= := decode_rng (to_list a{hr}) 12 (perm_nttunpackv i) _;smt(). 
+    rewrite /perm_nttunpackv /nttunpackv initiE 1:/# /= /#.
+
+  case (512<=i<768) => *.
+  + rewrite /nttunpack initiE 1:/# /= /subarray256 initiE /=;1:smt( nttunpack_inbounds).
+    rewrite mapiE /=;1:smt( nttunpack_inbounds).
+    rewrite -(Array1024.get_to_list rr) H2 H3 /decode12.
+    rewrite nth_mkseq /=;1: by smt(Array1024.size_to_list).
+    + rewrite  mapiE;1: by smt(perm_nttunpackv_rng).
+    congr; rewrite of_sintK /=.
+     rewrite /smod /= ifF. 
+     + rewrite /decode12_vec get_of_list;1: smt(perm_nttunpackv_rng). 
+       by have /= := decode_rng (to_list a{hr}) 12 (perm_nttunpackv i) _;smt(). 
+    rewrite modz_small. 
+    + rewrite /decode12_vec get_of_list; 1: smt(perm_nttunpackv_rng).
+       by have /= := decode_rng (to_list a{hr}) 12 (perm_nttunpackv i) _;smt(). 
+    rewrite /perm_nttunpackv /nttunpackv initiE 1:/# /= /#.
+
+  + rewrite /nttunpack initiE 1:/# /= /subarray256 initiE /=;1:smt( nttunpack_inbounds).
+    rewrite mapiE /=;1:smt( nttunpack_inbounds).
+    rewrite -(Array1024.get_to_list rr) H2 H3 /decode12.
+    rewrite nth_mkseq /=;1: by smt(Array1024.size_to_list).
+    + rewrite  mapiE;1: by smt(perm_nttunpackv_rng).
+    congr; rewrite of_sintK /=.
+     rewrite /smod /= ifF. 
+     + rewrite /decode12_vec get_of_list;1: smt(perm_nttunpackv_rng). 
+       by have /= := decode_rng (to_list a{hr}) 12 (perm_nttunpackv i) _;smt(). 
+    rewrite modz_small. 
+    + rewrite /decode12_vec get_of_list; 1: smt(perm_nttunpackv_rng).
+       by have /= := decode_rng (to_list a{hr}) 12 (perm_nttunpackv i) _;smt(). 
+    rewrite /perm_nttunpackv /nttunpackv initiE 1:/# /= /#.
+
+  rewrite /pos_bound1024_cxq qE /= => k kb. 
+  have /=? := decode_range_vec witness (to_list a{hr}) 12 _ _;1..2:smt(Array1536.size_to_list).
+  rewrite -get_to_list  H2 H3 /decode12_vec.
+  rewrite nth_mkseq /=;1: by rewrite size_map size_iota /#. 
+  rewrite get_of_list;1:smt(perm_nttunpackv_rng). 
+  rewrite (nth_map witness);1:smt(perm_nttunpackv_rng). 
+rewrite of_sintK /= /smod /= ifF;1:smt(@Zq perm_nttunpackv_rng).
+  rewrite modz_small;1,2:  smt(perm_nttunpackv_rng).  
+   
+qed.
+
+(********** END BDEP PROOF OF FROMBYTES **************)
+
+lemma polyvec_frombytes_corr (_aw : W8.t Array1536.t): 
+    phoare [Jkem1024_avx2.M.__i_polyvec_frombytes  :
+             a = _aw
+              ==>
+             lift_array1024 res = nttunpackv (map incoeff (decode12_vec _aw))  /\
+             pos_bound1024_cxq res 0 1024  2] = 1%r
+  by conseq polyvec_frombytes_ll (polyvec_frombytes_corr_h _aw).
 
 lemma polyvec_frombytes_equiv :
-    equiv [Jkem768_avx2.M.__polyvec_frombytes ~Jkem768.M.__polyvec_frombytes :
-             valid_ptr (W64.to_uint ap{1}) (3*384) /\
-             ={Glob.mem,ap} ==>
-             lift_array768 res{1} = nttunpackv (lift_array768 res{2}) /\
-             pos_bound768_cxq res{1} 0 768 2 /\
-             pos_bound768_cxq res{2} 0 768 2 ].
-admitted.
-
-lemma polyvec_tobytes_equiv :
-    forall (_p : int),
-    equiv [Jkem768_avx2.M.__polyvec_tobytes ~Jkem768.M.__polyvec_tobytes :
-             _p = to_uint rp{1} /\
-             valid_ptr (W64.to_uint rp{1}) (3*384) /\
-             pos_bound768_cxq a{1} 0 768 2 /\
-             pos_bound768_cxq a{2} 0 768 2 /\
-             lift_array768 a{1} = nttunpackv (lift_array768 a{2}) /\ ={rp,Glob.mem} ==> ={Glob.mem} ].
-admitted.
+    equiv [Jkem1024_avx2.M.__i_polyvec_frombytes ~Jkem1024.M.__i_polyvec_frombytes :
+             a{1}=ap{2} ==>
+             lift_array1024 res{1} = nttunpackv (lift_array1024 res{2}) /\
+             pos_bound1024_cxq res{1} 0 1024 2 /\
+             pos_bound1024_cxq res{2} 0 1024 2 ].
+proc*.
+ecall{1} (polyvec_frombytes_corr a{1}).
+ecall{2} (MLKEM_PolyVec.polyvec_frombytes_corr ap{2}).
+auto => /> &2 rr1 -> ? rr2 -> ? //.
+qed.
 
 
 lemma subequiv_noperm  (ab bb : int):
     0 <= ab && ab <= 6 =>
     0 <= bb && bb <= 3 =>
-    equiv [Jkem768_avx2.M._poly_sub ~Jkem768.M._poly_sub :
+    equiv [Jkem1024_avx2.M._poly_sub ~Jkem1024.M._poly_sub :
       lift_array256 ap{1} = lift_array256 ( ap{2}) /\
       lift_array256 bp{1} = lift_array256 ( bp{2}) /\
       signed_bound_cxq ap{2} 0 256 ab /\ 
@@ -126,9 +1637,8 @@ lemma subequiv_noperm  (ab bb : int):
               ].
 move => boundab boundbb; proc => /=.
 exists* ap{2}, bp{2}. elim* => _ap2 _bp2.
-while {2} (#pre /\ 0<= to_uint i{2} <= 256 /\ forall k, 0<=k<to_uint i{2} => rp{2}.[k] = _ap2.[k] -_bp2.[k]) (256 - to_uint i{2}); 
- 1: by move => &1 ?; auto => /> => &2 ?????????; rewrite ultE /=  !to_uintD_small 1:/# ;
-  smt(Array256.set_neqiE Array256.set_eqiE).
+while {2} (#pre /\ 0<= i{2} <= 256 /\ forall k, 0<=k<i{2} => rp{2}.[k] = _ap2.[k] -_bp2.[k]) (256 -  i{2}); 
+ 1: by move => &1 ?; auto => />;smt(Array256.set_neqiE Array256.set_eqiE).
 
 exists* ap{1}, bp{1}. elim* => _ap1 _bp1.
 while {1} (#pre /\ 0<= i{1} <= 16 /\ forall k, 0<=k<16*i{1} => rp{1}.[k] = _ap1.[k] -_bp1.[k]) (16 - i{1}); last first.
@@ -136,7 +1646,7 @@ while {1} (#pre /\ 0<= i{1} <= 16 /\ forall k, 0<=k<16*i{1} => rp{1}.[k] = _ap1.
   move => &1 &2 H H0 H1 H2 H3 H4; split; 1: smt(). 
   move => i1 res1; split; 1: smt().
   move => ??? res1v; split; 1: smt().
-  move => i2 res2; rewrite ultE /=; split; 1: smt().
+  move => i2 res2; split; 1: smt().
   move => ??? res2v.
   do split; first last.
   + do 2!( move : H3 H4;rewrite /signed_bound_cxq => H3 H4 k kb; rewrite res1v // 1:/#; 
@@ -200,7 +1710,7 @@ move : HHH; move : (W16.to_uint_cmp x); move :  (W16.to_uint_cmp y) => /=; smt()
 qed.
 
 equiv frommontequiv : 
- Jkem768_avx2.M._poly_frommont ~  Jkem768.M._poly_frommont :
+ Jkem1024_avx2.M._poly_frommont ~  Jkem1024.M._poly_frommont :
     lift_array256 arg{1} = nttunpack (lift_array256 arg{2}) ==> 
     lift_array256 res{1} = nttunpack (lift_array256 res{2}) /\
     signed_bound_cxq res{1} 0 256 2 /\ 
@@ -269,7 +1779,7 @@ do split.
 qed.
 
 equiv reduceequiv : 
- Jkem768_avx2.M.__poly_reduce ~  Jkem768.M.__poly_reduce :
+ Jkem1024_avx2.M.__poly_reduce ~  Jkem1024.M.__poly_reduce :
     lift_array256 arg{1} = nttunpack (lift_array256 arg{2}) ==> 
     lift_array256 res{1} = nttunpack (lift_array256 res{2}) /\
     pos_bound256_cxq res{1} 0 256 2 /\ 
@@ -299,7 +1809,7 @@ smt(Array256.mapiE nttunpack_bnd Array256.allP).
 qed.
 
 equiv reduceequiv_noperm : 
- Jkem768_avx2.M.__poly_reduce ~  Jkem768.M.__poly_reduce :
+ Jkem1024_avx2.M.__poly_reduce ~  Jkem1024.M.__poly_reduce :
     lift_array256 arg{1} = lift_array256 arg{2} ==> 
     lift_array256 res{1} = lift_array256 res{2} /\
     pos_bound256_cxq res{1} 0 256 2 /\ 
@@ -332,7 +1842,7 @@ import Zq.
 require import NTT_AVX_j.
 
 equiv basemulequiv : 
- Jkem768_avx2.M._poly_basemul ~Jkem768.M._poly_basemul :
+ Jkem1024_avx2.M._poly_basemul ~Jkem1024.M._poly_basemul :
     lift_array256 ap{1} = nttunpack (lift_array256 ap{2}) /\
     lift_array256 bp{1} = nttunpack (lift_array256 bp{2}) /\
     signed_bound_cxq ap{1} 0 256 2 /\  
@@ -342,7 +1852,7 @@ equiv basemulequiv :
                               ==> 
     lift_array256 res{1} = nttunpack (lift_array256 res{2}) /\
     signed_bound_cxq res{1} 0 256 1 /\ 
-    signed_bound_cxq res{2} 0 256 3.
+    signed_bound_cxq res{2} 0 256 2.
 proof.
 proc*; simplify.
 ecall{2} (poly_basemul_correct (lift_array256 ap{2}) (lift_array256 bp{2})).
@@ -372,7 +1882,7 @@ lemma addequiv  (ab1 bb1 ab2 bb2 : int):
     0 <= ab2 && ab2 <= 6 =>
     0 <= bb1 && bb1 <= 3 =>
     0 <= bb2 && bb2 <= 3 =>
-    equiv [Jkem768_avx2.M._poly_add2 ~Jkem768.M._poly_add2 :
+    equiv [Jkem1024_avx2.M._poly_add2 ~Jkem1024.M._poly_add2 :
       lift_array256 rp{1} = lift_array256 (nttunpack rp{2}) /\
       lift_array256 bp{1} = lift_array256 (nttunpack bp{2}) /\
       signed_bound_cxq rp{2} 0 256 ab2 /\ 
@@ -423,7 +1933,7 @@ qed.
 lemma addequiv_noperm  (ab bb : int):
     0 <= ab && ab <= 6 =>
     0 <= bb && bb <= 3 =>
-    equiv [Jkem768_avx2.M._poly_add2 ~Jkem768.M._poly_add2 :
+    equiv [Jkem1024_avx2.M._poly_add2 ~Jkem1024.M._poly_add2 :
       lift_array256 rp{1} = lift_array256 ( rp{2}) /\
       lift_array256 bp{1} = lift_array256 ( bp{2}) /\
       signed_bound_cxq rp{2} 0 256 ab /\ 
@@ -462,51 +1972,736 @@ rewrite !mapiE //=.
 rewrite H7 // H9 /#.
 qed.
 
+
+
+(********** BEGIN BDEP PROOF OF FROMMSG **************)
+
+op decompress1_circuit(c : bool) : W16.t = 
+  truncateu16 (srl_32 (((if c then W32.one else W32.zero) * W32.of_int 3329) + W32.one) (W32.of_int 1)).
+
+op pcond_true (w: bool) =  true. 
+
+lemma poly_frommsg_ll : islossless Jkem1024_avx2.M._i_poly_frommsg 
+ by proc; inline *;wp;while (0 <= i <= 32) (32-i);  by  auto =>  /> /#.
+
+lemma poly_frommsg_corr_h (_m : W8.t Array32.t): 
+    hoare [Jkem1024_avx2.M._i_poly_frommsg :
+             ap =  _m 
+              ==>
+             lift_array256 res = decompress_poly 1 (decode1 _m) /\
+             pos_bound256_cxq res 0 256 1 ].
+proc; inline *.
+proc change 1: (sliceget16_16_256 hqx16_p1 0);1: by auto.
+proc change 2: (VPBROADCAST_2u128 (sliceget4_32_128 pfm_shift_s 0));1: by auto.
+proc change 3: (VPBROADCAST_2u128 (sliceget16_8_128 pfm_idx_s 0));1: by auto.
+proc change 4: (sliceget32_8_256 ap 0);1: by auto.
+proc change ^while.23 : (sliceset256_16_256 rp (2*i*256) g0); 1: by auto => /#. 
+proc change ^while.24 : (sliceset256_16_256 rp ((2*i+1)*256) g1); 1: by auto => /#. 
+proc change ^while.25 : (sliceset256_16_256 rp ((2*i+8)*256) g2); 1: by auto => /#. 
+proc change ^while.26 : (sliceset256_16_256 rp ((2*i+9)*256) g3); 1: by auto => /#. 
+
+
+unroll for ^while.
+wp -1.
+
+bdep 1 16 [_m] [ap] [rp] decompress1_circuit pcond_true. 
+
+(* BDEP pre conseq *)
++ by move => &hr />; rewrite allP /pcond_true /=. 
+
+(* BDEP post conseq *)
+
+(* We start with some boilerplate *)
+move => &hr [#]/= <- rr; rewrite /= !flatten1.
+move => H1; have H2 := post_lane_commute_out_aligned (to_list ap{hr}) (to_list rr) W8.w2bits W8.bits2w bool2bits bits2bool W16.w2bits W16.bits2w  decompress1_circuit 8 1 16 _ _ _ _ _ _ _ _ _ _ _ _ H1;1..12:
+smt(Array32.size_to_list Array256.size_to_list W16.bits2wK BVA_Top_Pervasive_bool.oflistP).
+
+have H3 : 
+   map decompress1_circuit (map bits2bool (chunk 1 (flatten (map W8.w2bits (to_list ap{hr}))))) =
+   map (W16.of_int \o asint) (to_list (decompress_poly 1 (decode1 ap{hr}))).
++ rewrite /decode1 /decompress_poly Array256.map_of_list Array256.of_listK;1:smt(size_map Array256.size_to_list).
+  rewrite /decode -map_comp  -(map_comp _ (decompress 1)) -(map_comp _ BS2Int.bs2int) /=.
+  apply eq_in_map => x xb.
+  rewrite /(\o) /decompress1_circuit /bits2bool -decompress_alt_decompress /decompress_alt //=.
+  have := size_nth_chunk [] (flatten (map W8.w2bits (to_list ap{hr}))).
+  have := nthP witness (chunk 1 (flatten (map W8.w2bits (to_list ap{hr})))) x.
+  rewrite xb /= => He;elim He; rewrite size_chunk //= => k*. 
+  have ? : size x = 1 
+   by  have := size_nth_chunk witness (flatten (map W8.w2bits (to_list ap{hr}))) k 1 =>/= /#.
+  rewrite qE to_uint_eq to_uint_truncateu16 /= /srl_32 /= of_uintK /=;congr;congr.
+  rewrite to_uint_shr //=.
+  case (x = [true]).
+  + move => -> /=;rewrite bs2int_cons /= BS2Int.bs2int_nil /= /b2i /=;smt(@Zq).
+  case (x = [false]); last by smt(@List).
+  by  move => -> /=;rewrite bs2int_cons /= BS2Int.bs2int_nil /= /b2i /=;smt(@Zq).
+
+split.
++ rewrite tP => i ib.
+  rewrite !mapiE 1,2:/# /= -get_to_list H2 H3 /decompress_poly.
+  rewrite (nth_map witness);1: by smt(Array256.size_to_list).
+  rewrite get_to_list /= /(\o) mapiE 1:/# /=.
+  pose c := (decompress 1 (decode1 ap{hr}).[i]).
+  rewrite /smod /= ifF;1:smt(@Zq).
+  rewrite modz_small; smt(@Zq).  
+
+rewrite /pos_bound256_cxq qE /= => k kb. 
+rewrite -get_to_list  H2 H3 /decompress_poly.
+  rewrite (nth_map witness);1: by smt(Array256.size_to_list).
+  rewrite get_to_list /= /(\o) mapiE 1:/# /=.
+  rewrite  /smod /= ifF;1:smt(@Zq).
+  rewrite modz_small; smt(@Zq).  
+qed.
+
+(********** END BDEP PROOF OF FROMMSG **************)
+
+
+lemma poly_frommsg_corr (_m : W8.t Array32.t): 
+    phoare [Jkem1024_avx2.M._i_poly_frommsg :
+             ap =  _m 
+              ==>
+             lift_array256 res = decompress_poly 1 (decode1 _m) /\
+             pos_bound256_cxq res 0 256 1 ] = 1%r
+  by conseq poly_frommsg_ll (poly_frommsg_corr_h _m).
+
 equiv frommsgequiv_noperm  : 
- Jkem768_avx2.M._poly_frommsg_1 ~  Jkem768.M._i_poly_frommsg :
+ Jkem1024_avx2.M._i_poly_frommsg ~  Jkem1024.M._i_poly_frommsg :
     ={ap} ==> 
     lift_array256 res{1} = lift_array256 res{2} /\
     pos_bound256_cxq res{1} 0 256 1 /\ 
     pos_bound256_cxq res{2} 0 256 1.
-admitted.
+proc*.
+ecall {1} (poly_frommsg_corr ap{1}).
+ecall {2} (MLKEM_Poly.poly_frommsg_corr ap{1}).
+by auto => /> /#.
+qed.
 
 lemma compress_poly_rng i xs :
   1 <= i < 12 =>
   all (fun (x : int) => 0 <= x < 2^i) (compress_poly i xs).
 rewrite /compress_poly /map allP => Hi j Hj. rewrite !initiE //=. rewrite compress_rng //. qed.
 
+
+lemma poly_tomsg_ll : islossless Jkem1024_avx2.M._i_poly_tomsg.
+proc.
+cfold 7.
+inline *.
+do 2!(unroll for ^while).
+auto.
+qed.
+
+(********** BEGIN BDEP PROOF OF TOMSG **************)
+
+
+op compress1_circuit(a : W16.t) : bool = 
+   if (a \ult W16.of_int 3329) then  
+   (srl_32 ((sll_32 (zeroextu32 a) (W32.of_int 1) + W32.of_int 1665) * W32.of_int 80635) (W32.of_int 28)).[0]
+   else 
+   (srl_32 ((sll_32 (zeroextu32 (W16_sub a (W16.of_int 3329))) (W32.of_int 1) + W32.of_int 1665) * W32.of_int 80635) (W32.of_int 28)).[0].  
+
+op pcond_reduced (w: W16.t) =   w \ult W16.of_int (2*3329). 
+
+lemma poly_tomsg_corr_h _aw : 
+    hoare [Jkem1024_avx2.M._i_poly_tomsg :
+             pos_bound256_cxq a 0 256 2 /\ 
+              a = _aw
+              ==>
+             res.`1 = encode1 (compress_poly 1 (lift_array256 _aw))  ].
+proof.
+proc; inline *.
+proc change 3 : (sliceget16_16_256 jqx16 0);1: by auto.
+proc change ^while.1: (sliceget256_16_256 rp0 (i0*256));1: by auto => /#.
+proc change ^while.9: (sliceset256_16_256 rp0 (i0*256) r);1: by auto => /#.
+proc change 8: (sliceget16_16_256 px16 0); 1: by auto.
+proc change 10: (sliceget16_16_256 px16 0); 1: by auto.
+proc change ^while{2}.1: (sliceget256_16_256 a (2*i*256));1: by auto => /#.
+proc change ^while{2}.2: (sliceget256_16_256 a ((2*i+1)*256));1: by auto => /#.
+proc change ^while{2}.14 : (sliceset32_8_32 rp  (i*32) c);1: by auto => /#.
+
+
+cfold 11.
+unroll for ^while.
+cfold ^i0<-.
+unroll for ^while.
+wp -3. 
+
+bdep 16 1 [_aw] [a] [rp] compress1_circuit pcond_reduced. 
+
+(* BDEP pre conseq *)
++ move => &hr />; rewrite flatten1 /= pre_lane_commute_in_aligned 1:/# //=.
+  rewrite allP /pos_bound256_cxq /= => Hb. 
+  rewrite /pcond_reduced /= /tolist /= => x.
+  rewrite  mkseqP => He;elim He => /= i [ib?]; rewrite ultE /=.
+  have := Hb i; rewrite ib /= qE /=.
+  rewrite /to_sint /smod /=.
+  smt(W16.to_uint_cmp).
+
+(* BDEP post conseq *)
+
+(* We start with some boilerplate *)
+move => &hr [#]/= H0 <- rr; rewrite /= !flatten1.
+move => H1.
+
+apply (inj_eq Array32.to_list Array32.to_list_inj).
+apply (flatten_map_eq _ _ W8.w2bits 8 _ W8.w2bits_inj W8.size_w2bits);1:smt().
+have -> := post_lane_commute_in_aligned (to_list a{hr}) (to_list rr) W16.w2bits W16.bits2w W8.w2bits W8.bits2w bool2bits bits2bool  compress1_circuit 16 1 8 _ _ _ _ _ _ _ _ _ _ _ _ H1;1..12:
+    smt(Array32.size_to_list Array256.size_to_list W16.bits2wK BVA_Top_Pervasive_bool.oflistP).
+
+rewrite output_pack_32_8. 
++ rewrite (EclibExtra.size_flatten' 1);1: smt(mapP BS2Int.size_int2bs).
+  by rewrite size_map size_to_list /=.
+
+congr.
+rewrite /compress1_circuit /compress_poly -map_comp -map_comp -map_comp /(\o) /=.  
+apply (eq_from_nth witness); 1: by rewrite !size_map //.
+rewrite size_map size_iota /max /= => i ib; rewrite !(nth_map witness) //=;1,2:smt(size_iota).
+rewrite nth_iota 1:/# -(BVA_Top_Pervasive_bool.oflistP (BS2Int.int2bs 1 (map (compress 1) (lift_array256 a{hr})).[i]));1: by rewrite BS2Int.size_int2bs /#.
+congr; rewrite -BVA_Top_Pervasive_bool.ofintP /lift_array256;rewrite !mapiE;1,2:smt().
+
+rewrite /i2b !get_to_uint /=.
+
+(* This is now the equivalence betwen specs. It's made slightly more verbose
+   because the impl circuit is only proved correct wrt compress for values
+   in the q range. *)
+rewrite ultE /=. 
+case (to_uint a{hr}.[i] < 3329) => /= *.
++ rewrite -compress_impl_small //=;1: by rewrite /bpos16 qE /= /to_sint /smod /=;smt(W16.to_uint_cmp).  
+  congr;congr;rewrite modz_mod;congr;congr.
+  by rewrite /srl_32 /sll_32 /(`<<`) /(`>>`).
+
+have := H0;rewrite /pos_bound256_cxq qE /= => H00.
+
+have ? : 0 <= to_sint ((W16_sub a{hr}.[i] (W16.of_int 3329))) < 3329.
++  rewrite /bpos16 to_sintB_small /=;1: by rewrite  /(to_sint (W16.of_int 3329)) /= /smod /=;smt(size_map size_iota). 
+   by rewrite  /(to_sint (W16.of_int 3329)) /= /smod /=; smt(size_map size_iota W16.to_uint_cmp).
+
+have ? : to_sint ((W16_sub a{hr}.[i] (W16.of_int 3329))) = to_sint a{hr}.[i] -  3329.
++  rewrite to_sintB_small /=;1: by rewrite  /(to_sint (W16.of_int 3329)) /= /smod /=;smt(size_map size_iota). 
+   by rewrite  /(to_sint (W16.of_int 3329))  /= /smod /=; smt(size_map size_iota W16.to_uint_cmp).
+
+have -> : (incoeff (to_sint a{hr}.[i])) = (incoeff (to_sint (W16_sub a{hr}.[i] (W16.of_int 3329)))) by  rewrite -eq_incoeff;  smt().  
+
+rewrite -compress_impl_small //=;1:by smt().
+by rewrite modz_mod /srl_32 /sll_32 /(`<<`) /(`>>`).
+qed.
+
+(********** END BDEP PROOF OF TOMSG **************)
+
+
+lemma poly_tomsg_corr _aw : 
+    phoare [Jkem1024_avx2.M._i_poly_tomsg :
+             pos_bound256_cxq a 0 256 2 /\ 
+              a = _aw
+              ==>
+             res.`1 = encode1 (compress_poly 1 (lift_array256 _aw))  ] = 1%r
+  by conseq poly_tomsg_ll (poly_tomsg_corr_h _aw).
+
 equiv tomsgequiv_noperm  : 
- Jkem768_avx2.M._poly_tomsg_1 ~  Jkem768.M._i_poly_tomsg :
+ Jkem1024_avx2.M._i_poly_tomsg ~  Jkem1024.M._i_poly_tomsg :
     lift_array256 a{1} = lift_array256 a{2} /\
     pos_bound256_cxq a{1} 0 256 2 /\ 
     pos_bound256_cxq a{2} 0 256 2 ==>
     res{1}.`1 = res{2}.`1.
-admitted.
+proc *.
+ecall {1} (poly_tomsg_corr a{1}).
+ecall {2} (MLKEM_Poly.poly_tomsg_corr a{2}).
+auto => /#. 
+qed.
+
+(********** BEGIN BDEP PROOF OF TOBYTES **************)
+
+op tobytes_circuit(a : W16.t) : W12.t = 
+   if (a \ult W16.of_int 3329) then truncateu12 a else truncateu12 (W16_sub a (W16.of_int 3329)).  
+
+lemma polyvec_tobytes_ll : islossless Jkem1024_avx2.M.__i_polyvec_tobytes.
+proc.
+inline *. 
+do 9!(unroll for ^while); auto. 
+qed.
+
+lemma post_lane_commute_in_aligned_perm ['a 'b 'c]
+    (li : 'a list) 
+    (loc : 'b list) 
+    (tobitsi : 'a -> bool list)
+    (ofbitsi : bool list -> 'a)
+    (tobitsoc : 'b -> bool list)
+    (ofbitsoc : bool list -> 'b)
+    (tobitso : 'c -> bool list)
+    (ofbitso : bool list -> 'c)
+    (f : 'a -> 'c)
+    (ni no noc  : int) 
+    (perm : int -> int)
+    (permi : int -> int):
+  0 < ni =>  0 < no => 0 < noc => 
+  no %| noc*size loc =>
+  size li = (noc*size loc) %/ no =>
+  (forall x, size (tobitsi x) = ni) =>
+  (forall x, ofbitsi (tobitsi x) = x) =>
+  (forall x, size (tobitso x) = no) =>
+  (forall x, ofbitso (tobitso x) = x) =>
+  (forall x, size x = no => tobitso (ofbitso x) = x) =>
+  (forall x, size (tobitsoc x) = noc) =>
+  (forall x, ofbitsoc (tobitsoc x) = x) =>
+  (forall ii, 0 <= ii < size li => 0 <= permi ii < size li) =>
+  (forall ii, 0 <= ii < size li => perm (permi ii) = ii) =>
+map f (map ofbitsi (chunk ni (flatten (map tobitsi  li)))) =
+mkseq (fun i => nth witness
+     (map ofbitso (chunk no (flatten (map tobitsoc loc)))) (perm i)) 
+      (size (map ofbitso (chunk no (flatten (map tobitsoc loc))))) => 
+   flatten (map tobitsoc loc) =
+   flatten (map tobitso (map f (mkseq (fun i => nth witness li (permi i)) (size li)))).
+move => 14?.
+rewrite map_chunk_flatten_id 1..3:/#.
+move => H.
+rewrite map_mkseq /(\o) /=.
+have -> : (mkseq (fun (x : int) => f (nth witness li (permi x))) (size li)) =
+   (mkseq (fun (x : int) =>  (nth witness (map f li) (permi x))) (size li)).
++ apply eq_in_mkseq => i ib /=.
+  by rewrite (nth_map witness) 1:/#.
+rewrite H.
+have -> : (mkseq
+        (fun (x : int) =>
+           nth witness
+             (mkseq (fun (i : int) => nth witness (map ofbitso (chunk no (flatten (map tobitsoc loc)))) (perm i))
+                (size (map ofbitso (chunk no (flatten (map tobitsoc loc)))))) (
+             permi x)) (size li)) =
+   map ofbitso (mkseq
+        (fun (x : int) =>
+           nth witness
+             (mkseq (fun (i : int) => nth witness (chunk no (flatten (map tobitsoc loc))) (perm i))
+                (size (map ofbitso (chunk no (flatten (map tobitsoc loc)))))) (
+             permi x)) (size li)).
+have -> := map_mkseq ofbitso
+     (fun (x : int) =>
+        nth witness
+          (mkseq (fun (i : int) => nth witness (chunk no (flatten (map tobitsoc loc))) (perm i))
+             (size (map ofbitso (chunk no (flatten (map tobitsoc loc)))))) (
+          permi x)) (size li).
++ apply eq_in_mkseq => i ib /=.
+  rewrite /(\o) /= !(nth_mkseq) /=;1,2: by 
+  rewrite size_map size_chunk 1:/#  (EclibExtra.size_flatten' noc);smt(mapP size_map).
+  by rewrite (nth_map witness);1: by
+   rewrite size_chunk 1:/# (EclibExtra.size_flatten' noc);smt(mapP size_map).
+
+rewrite -map_comp /(\o) /=.
+
+have -> : (mkseq
+        (fun (x : int) =>
+           nth witness
+             (mkseq (fun (i : int) => nth witness (chunk no (flatten (map tobitsoc loc))) (perm i))
+                (size (map ofbitso (chunk no (flatten (map tobitsoc loc)))))) (
+             permi x)) (size li))
+ = (chunk no (flatten (map tobitsoc loc))) .
++ apply (eq_from_nth witness).
+  + rewrite size_mkseq size_chunk 1:/# (EclibExtra.size_flatten' noc);1: smt(mapP).
+    rewrite size_map;smt(size_ge0).
+  move => i; rewrite size_mkseq /max => ib.
+  rewrite nth_mkseq 1:/# /= nth_mkseq /=.  
+  + rewrite size_map size_chunk 1:/# (EclibExtra.size_flatten' noc);1: smt(mapP).
+    rewrite size_map;smt(size_ge0).
+  by smt().
+have /= [-> x] := eq_in_map (fun (x : bool list) => tobitso (ofbitso x)) idfun (chunk no (flatten (map tobitsoc loc))).
+have := in_chunk_size no (flatten (map tobitsoc loc)) x _;smt().
+
+rewrite map_id chunkK 1:/#; last by done.
+rewrite (EclibExtra.size_flatten' noc); smt(size_map mapP).
+qed.
+
+lemma output_pack_1536_8(l : bool list) :
+ size l = 1024*12 =>
+ flatten
+  (map W8.w2bits
+     (to_list (Array1536.of_list W8.zero (BitsToBytes l)))) = l.
+move => *.
+rewrite of_listK; 1: by rewrite size_BitsToBytes /#.
+have ? : size (flatten (map W8.w2bits (BitsToBytes l))) = size l.
++ rewrite (EclibExtra.size_flatten' 8);1: smt(mapP W8.size_w2bits).
+  by rewrite size_map size_BitsToBytes /#.
+
+apply (eq_from_nth witness); 1: smt().
+move => i ib.
+rewrite (nth_flatten _ 8);1: by rewrite allP => *; smt( mapP W8.size_w2bits).
+rewrite (nth_map witness);1: smt(size_BitsToBytes).
+rewrite /BitsToBytes (nth_map []);1:by smt(size_chunk).
+rewrite bits2wK;1: smt(size_nth_chunk).
+rewrite -(nth_flatten _ 8);1: by rewrite allP => * /=;smt(in_chunk_size). 
+by rewrite chunkK /#.
+qed.
+
+lemma nttpackv_alt (a : W16.t Array1024.t) i :
+ 0 <= i < 1024 =>
+  a.[perm_nttpackv i] = (nttpackv a).[i].
+proof.
+move => ?;have : all (fun i => a.[perm_nttpackv i] = (nttpackv a).[i]) (iota_ 0 1024);
+  last by rewrite allP => H; move : (H i);smt(mem_iota).
+by rewrite /nttpackv /subarray256 /nttpack /perm_nttpackv -iotaredE /=.
+qed. 
+
+abbrev mask12 = VPBROADCAST_16u16(W16.of_int 4095).
+
+module AuxToBytes = {
+proc __i_polyvec_tobytes(r : W8.t Array1536.t, a : W16.t Array1024.t) : W8.t Array1536.t = {
+  var i,rp,a0,i0,t0,t1,t2,t3,t4,t5,t6,t7,tt,ttt,a1,b,t00,r00,t10,r1,a2,b0,t01,r01,t11,r10,a3,b1,t02,r02,t12,r11,a4,b2,t03,t13,a5,b3,t04,t14,a6,b4,t05,t15,a7,b5,r03,r12,a8,b6,r04,r13,a9,b7,r05,r14,a10,b8,r06,r15,a11,b9,r07,r16,a12,b10,r08,r17,aux,aux_0;
+  i <- 0;                                                                                                                       
+  while (i < 4) {                                                                                                              
+    rp <- Array384.init (fun (i_0 : int) => r.[384 * i + i_0]);                                                                 
+    a0 <- Array256.init (fun (i_0 : int) => a.[256 * i + i_0]);  
+    a0 <@ Jkem1024_avx2.M._poly_csubq(a0);                                                           
+    i0 <- 0;                                                                                                                    
+    while (i0 < 2) {                                                                                                           
+      t0 <- get256 (WArray512.init16 (fun (i_0 : int) => a0.[i_0])) (8 * i0);                                                   
+      t1 <- get256 (WArray512.init16 (fun (i_0 : int) => a0.[i_0])) (8 * i0 + 1);                                               
+      t2 <- get256 (WArray512.init16 (fun (i_0 : int) => a0.[i_0])) (8 * i0 + 2);                                               
+      t3 <- get256 (WArray512.init16 (fun (i_0 : int) => a0.[i_0])) (8 * i0 + 3);                                               
+      t4 <- get256 (WArray512.init16 (fun (i_0 : int) => a0.[i_0])) (8 * i0 + 4);                                               
+      t5 <- get256 (WArray512.init16 (fun (i_0 : int) => a0.[i_0])) (8 * i0 + 5);                                               
+      t6 <- get256 (WArray512.init16 (fun (i_0 : int) => a0.[i_0])) (8 * i0 + 6);                                               
+      t7 <- get256 (WArray512.init16 (fun (i_0 : int) => a0.[i_0])) (8 * i0 + 7);                                               
+      t0 <- t0 `&` mask12;                                                                                                      
+      t1 <- t1 `&` mask12;                                                                                                      
+      t2 <- t2 `&` mask12;                                                                                                      
+      t3 <- t3 `&` mask12;                                                                                                      
+      t4 <- t4 `&` mask12;                                                                                                      
+      t5 <- t5 `&` mask12;                                                                                                      
+      t6 <- t6 `&` mask12;                                                                                                      
+      t7 <- t7 `&` mask12;                                                                                                      
+      tt <- VPSLL_16u16 t1 (W128.of_int 12);                                                                                    
+      tt <- tt `|` t0;                                                                                                          
+      t0 <- VPSRL_16u16 t1 (W128.of_int 4);                                                                                     
+      t1 <- VPSLL_16u16 t2 (W128.of_int 8);                                                                                     
+      t0 <- t0 `|` t1;                                                                                                          
+      t1 <- VPSRL_16u16 t2 (W128.of_int 8);                                                                                     
+      t2 <- VPSLL_16u16 t3 (W128.of_int 4);                                                                                     
+      t1 <- t1 `|` t2;                                                                                                          
+      t2 <- VPSLL_16u16 t5 (W128.of_int 12);                                                                                    
+      t2 <- t2 `|` t4;                                                                                                          
+      t3 <- VPSRL_16u16 t5 (W128.of_int 4);                                                                                     
+      t4 <- VPSLL_16u16 t6 (W128.of_int 8);                                                                                     
+      t3 <- t3 `|` t4;                                                                                                         
+      t4 <- VPSRL_16u16 t6 (W128.of_int 8);                                                                                     
+      t5 <- VPSLL_16u16 t7 (W128.of_int 4);                                                                                     
+      t4 <- t4 `|` t5;                                                                                                          
+      a1 <- tt;                                                                                                                 
+      b <- t0;                                                                                                                  
+      t00 <- VPSLL_8u32 b (W128.of_int 16);                                                                                     
+      r00 <- VPBLENDW_256 a1 t00 (W8.of_int 170);                                                                               
+      t10 <- VPSRL_8u32 a1 (W128.of_int 16);                                                                                    
+      r1 <- VPBLENDW_256 t10 b (W8.of_int 170);                                                                                 
+      (ttt, t0) <- (r00, r1);                                                                                                   
+      a2 <- t1;                                                                                                                 
+      b0 <- t2;                                                                                                                 
+      t01 <- VPSLL_8u32 b0 (W128.of_int 16);                                                                                    
+      r01 <- VPBLENDW_256 a2 t01 (W8.of_int 170);                                                                               
+      t11 <- VPSRL_8u32 a2 (W128.of_int 16);                                                                                    
+      r10 <- VPBLENDW_256 t11 b0 (W8.of_int 170);                                                                               
+      (tt, t2) <- (r01, r10);                                                                                                   
+      a3 <- t3;                                                                                                                 
+      b1 <- t4;                                                                                                                
+      t02 <- VPSLL_8u32 b1 (W128.of_int 16);                                                                                    
+      r02 <- VPBLENDW_256 a3 t02 (W8.of_int 170);                                                                               
+      t12 <- VPSRL_8u32 a3 (W128.of_int 16);                                                                                    
+      r11 <- VPBLENDW_256 t12 b1 (W8.of_int 170);                                                                               
+      (t1, t4) <- (r02, r11);                                                                                                   
+      a4 <- ttt;                                                                                                               
+      b2 <- tt;                                                                                                                 
+      t03 <- VMOVSLDUP_256 b2;                                                                                                  
+      t03 <- VPBLENDD_256 a4 t03 (W8.of_int 170);                                                                               
+      a4 <- VPSRL_4u64 a4 (W128.of_int 32);                                                                                     
+      t13 <- VPBLENDD_256 a4 b2 (W8.of_int 170);                                                                                
+      (t3, tt) <- (t03, t13);                                                                                                   
+      a5 <- t1;                                                                                                                 
+      b3 <- t0;                                                                                                                 
+      t04 <- VMOVSLDUP_256 b3;                                                                                                  
+      t04 <- VPBLENDD_256 a5 t04 (W8.of_int 170);                                                                               
+      a5 <- VPSRL_4u64 a5 (W128.of_int 32);                                                                                     
+      t14 <- VPBLENDD_256 a5 b3 (W8.of_int 170);                                                                                
+      (ttt, t0) <- (t04, t14);                                                                                                  
+      a6 <- t2;                                                                                                                 
+      b4 <- t4;                                                                                                                 
+      t05 <- VMOVSLDUP_256 b4;                                                                                                  
+      t05 <- VPBLENDD_256 a6 t05 (W8.of_int 170);                                                                               
+      a6 <- VPSRL_4u64 a6 (W128.of_int 32);                                                                                     
+      t15 <- VPBLENDD_256 a6 b4 (W8.of_int 170);                                                                                
+      (t1, t4) <- (t05, t15);                                                                                                   
+      a7 <- t3;                                                                                                                 
+      b5 <- ttt;                                                                                                                
+      r03 <- VPUNPCKL_4u64 a7 b5;                                                                                               
+      r12 <- VPUNPCKH_4u64 a7 b5;                                                                                               
+      (t2, ttt) <- (r03, r12);                                                                                                  
+      a8 <- t1;                                                                                                                 
+      b6 <- tt;                                                                                                                 
+      r04 <- VPUNPCKL_4u64 a8 b6;                                                                                               
+      r13 <- VPUNPCKH_4u64 a8 b6;                                                                                               
+      (t3, tt) <- (r04, r13);                                                                                                   
+      a9 <- t0;                                                                                                                 
+      b7 <- t4;                                                                                                                 
+      r05 <- VPUNPCKL_4u64 a9 b7;                                                                                               
+      r14 <- VPUNPCKH_4u64 a9 b7;                                                                                               
+      (t1, t4) <- (r05, r14);                                                                                                   
+      a10 <- t2;                                                                                                                
+      b8 <- t3;                                                                                                                 
+      r06 <- VPERM2I128 a10 b8 (W8.of_int 32);                                                                                  
+      r15 <- VPERM2I128 a10 b8 (W8.of_int 49);                                                                                  
+      (t0, t3) <- (r06, r15);                                                                                                   
+      a11 <- t1;                                                                                                                
+      b9 <- ttt;                                                                                                                
+      r07 <- VPERM2I128 a11 b9 (W8.of_int 32) ;                                                                                 
+      r16 <- VPERM2I128 a11 b9 (W8.of_int 49) ;                                                                                 
+      (t2, ttt) <- (r07, r16);                                                                                                  
+      a12 <- tt;                                                                                                                
+      b10 <- t4;                                                                                                                
+      r08 <- VPERM2I128 a12 b10 (W8.of_int 32);                                                                                 
+      r17 <- VPERM2I128 a12 b10 (W8.of_int 49);                                                                                 
+      (t1, t4) <- (r08, r17);                                                                                                   
+      rp <-                                                                                                                    
+        Array384.init                                                                                                          
+          (WArray384.get8                                                                                            
+             (WArray384.set256_direct (WArray384.init8 (fun (i_0 : int) => rp.[i_0])) (192 * i0) t0));      
+      rp <-                                                                                                                    
+        Array384.init                                                                                                          
+          (WArray384.get8                                                                                            
+             (WArray384.set256_direct (WArray384.init8 (fun (i_0 : int) => rp.[i_0])) (192 * i0 + 32) t2)); 
+      rp <-                                                                                                                    
+        Array384.init                                                                                                          
+          (WArray384.get8                                                                                            
+             (WArray384.set256_direct (WArray384.init8 (fun (i_0 : int) => rp.[i_0])) (192 * i0 + 64) t1)); 
+      rp <-                                                                                                                    
+        Array384.init                                                                                                          
+          (WArray384.get8                                                                                            
+             (WArray384.set256_direct (WArray384.init8 (fun (i_0 : int) => rp.[i_0])) (192 * i0 + 96) t3)); 
+      rp <-                                                                                                                    
+        Array384.init                                                                                                          
+          (WArray384.get8                                                                                            
+             (WArray384.set256_direct (WArray384.init8 (fun (i_0 : int) => rp.[i_0])) (                    
+                192 * i0 + 128) ttt));                                                                                          
+      rp <-                                                                                                                    
+        Array384.init                                                                                                          
+          (WArray384.get8                                                                                            
+             (WArray384.set256_direct (WArray384.init8 (fun (i_0 : int) => rp.[i_0])) (192 * i0 + 160) t4));
+      i0 <- i0 + 1;                                                                                                             
+    }                                                                                                                          
+    (aux, aux_0) <- (rp, a0);                                                                                                   
+    r <- Array1536.init (fun (i_0 : int) => if 384 * i <= i_0 < 384 * i + 384 then aux.[i_0 - 384 * i] else r.[i_0]);           
+    a <- Array1024.init (fun (i_0 : int) => if 256 * i <= i_0 < 256 * i + 256 then aux_0.[i_0 - 256 * i] else a.[i_0]);         
+    i <- i + 1;                                                                                                                 
+  }
+  return r;
+ }       
+}.
+
+lemma auxtobytes_corr_h (_aw : W16.t Array1024.t):
+    hoare[AuxToBytes.__i_polyvec_tobytes :
+             pos_bound1024_cxq a 0 1024 2 /\ a = _aw ==> 
+    res = encode12_vec (map asint (lift_array1024 (nttpackv _aw)))]. 
+proc;inline *.
+proc change ^while.1: (init_384_8 (fun i_0 => r.[384 * i + i_0]));1: by auto.
+proc change ^while.2: (init_256_16 (fun i_0 => a.[256 * i + i_0]));1: by auto.
+(* FIXME: CHECK qx16 initialization inside while *)
+proc change ^while.4: (sliceget16_16_256 jqx16 0); 1: by auto.
+proc change ^while.^while.1: (sliceget256_16_256 rp0 (i1*256)); 1: by auto => /#.
+proc change ^while.^while.9 : (sliceset256_16_256 rp0 (i1*256) r0); 1: by auto => /> /#.
+proc change ^while.^while{2}.1 : (sliceget256_16_256 a0 (8*i0*256));1: by auto => /#.
+proc change ^while.^while{2}.2 : (sliceget256_16_256 a0 ((8*i0+1)*256));1: by auto => /#.
+proc change ^while.^while{2}.3 : (sliceget256_16_256 a0 ((8*i0+2)*256));1: by auto => /#.
+proc change ^while.^while{2}.4 : (sliceget256_16_256 a0 ((8*i0+3)*256));1: by auto => /#.
+proc change ^while.^while{2}.5 : (sliceget256_16_256 a0 ((8*i0+4)*256));1: by auto => /#.
+proc change ^while.^while{2}.6 : (sliceget256_16_256 a0 ((8*i0+5)*256));1: by auto => /#.
+proc change ^while.^while{2}.7 : (sliceget256_16_256 a0 ((8*i0+6)*256));1: by auto => /#.
+proc change ^while.^while{2}.8 : (sliceget256_16_256 a0 ((8*i0+7)*256));1: by auto => /#.
+proc change ^while.^while{2}.105 : (sliceset384_8_256 rp (192*i0*8) t0);1: by auto => /#.
+proc change ^while.^while{2}.106 : (sliceset384_8_256 rp ((192*i0+32)*8) t2);1: by auto => /#.
+proc change ^while.^while{2}.107 : (sliceset384_8_256 rp ((192*i0+64)*8) t1);1: by auto => /#.
+proc change ^while.^while{2}.108 : (sliceset384_8_256 rp ((192*i0+96)*8) t3);1: by auto => /#.
+proc change ^while.^while{2}.109 : (sliceset384_8_256 rp ((192*i0+128)*8) ttt);1: by auto => /#.
+proc change ^while.^while{2}.110 : (sliceset384_8_256 rp ((192*i0+160)*8) t4);1: by auto => /#.
+proc change ^while.11: (init_1536_8 (fun (i_0 : int) => if 384 * i <= i_0 < 384 * i + 384 then aux.[i_0 - 384 * i] else r.[i_0])  ); 1: by auto.
+proc change ^while.12: (init_1024_16  (fun (i_0 : int) => if 256 * i <= i_0 < 256 * i + 256 then aux_0.[i_0 - 256 * i] else a.[i_0]));1: by auto. 
+
+unroll for ^while.
+do 8!(unroll for ^while).
+cfold ^i<-.
+cfold ^i0<-.
+cfold ^i1<-.
+wp -4.
+
+bdep 16 12 [_aw] [a] [r] tobytes_circuit pcond_reduced perm_nttunpackv. 
+
+(* BDEP pre conseq *)
++ move => &hr />; rewrite flatten1 /= pre_lane_commute_in_aligned 1:/# //=.
+  rewrite allP /pos_bound124_cxq /= => Hb. 
+  rewrite /pcond_reduced /= /tolist /= => x.
+  rewrite  mkseqP => He;elim He => /= i [ib?]; rewrite ultE /=.
+  have := Hb i; rewrite ib /= qE /=.
+  rewrite /to_sint /smod /=.
+  smt(W16.to_uint_cmp).
+
+(* BDEP post conseq *)
+
+(* We start with some boilerplate *)
+move => &hr [#]/= H0 <- rr; rewrite /= !flatten1.
+move => H1.
+apply (inj_eq Array1536.to_list Array1536.to_list_inj).
+apply (flatten_map_eq _ _ W8.w2bits 8 _ W8.w2bits_inj W8.size_w2bits);1:smt().
+have -> := post_lane_commute_in_aligned_perm (to_list a{hr}) (to_list rr) W16.w2bits W16.bits2w W8.w2bits W8.bits2w W12.w2bits W12.bits2w  tobytes_circuit 16 12 8 perm_nttunpackv perm_nttpackv _ _ _ _ _ _ _ _ _ _ _ _ _ _ _;1..12:
+smt(Array1536.size_to_list Array1024.size_to_list W16.bits2wK BVA_Top_Bindings_W12_t.oflistP).
++ smt(perm_nttpackv_rng Array1024.size_to_list).
++ move => ?; rewrite Array1024.size_to_list => ?;smt(nttpermsKi). 
++ by smt().
+
+rewrite output_pack_1536_8. 
++ rewrite (EclibExtra.size_flatten' 12);1: smt(mapP BS2Int.size_int2bs).
+  by rewrite size_map size_to_list /=.
+
+congr.
+rewrite /tobytes_circuit -map_comp -map_comp -map_comp /(\o) /=.
+apply (eq_from_nth witness);1: by  rewrite !size_map //;smt(size_iota).
+rewrite size_map !size_iota /max /= => i; rewrite size_to_list /= => ib; rewrite !(nth_map witness) //=;1,2:smt(size_iota).
+rewrite nth_iota 1:/# -(BVA_Top_Bindings_W12_t.oflistP (BS2Int.int2bs 12 (map asint (lift_array1024 (nttpackv a{hr}))).[i])); 1: by rewrite BS2Int.size_int2bs /#.
+congr; rewrite -BVA_Top_Bindings_W12_t.ofintP /lift_array256;rewrite !mapiE 1,2:/#.
+
+(* This is now the equivalence betwen specs.*)
+rewrite ultE /=; have HH := nttpackv_alt a{hr} i ib.
+have HG := perm_nttpackv_rng i ib.
+rewrite HH.
+
+case (to_uint (nttpackv a{hr}).[i] < 3329) => /= *.
++ rewrite  /truncateu12;congr. 
+  rewrite incoeffK qE /to_sint /= /smod /= ifF 1:/#  modz_small;smt(W16.to_uint_cmp). 
+
+have := H0;rewrite /pos_bound1024_cxq qE /= => H00.
+
+have ? : 0 <= to_sint ((W16_sub (nttpackv a{hr}).[i] (W16.of_int 3329))) < 3329.
++  rewrite /bpos16 to_sintB_small /=;1: by rewrite  /(to_sint (W16.of_int 3329))  /= /smod /=;smt(size_map size_iota). 
+   rewrite  /(to_sint (W16.of_int 3329)) /= /smod /=;   smt(size_map size_iota W16.to_uint_cmp).
+
+have ? : to_sint ((W16_sub (nttpackv a{hr}).[i] (W16.of_int 3329))) = to_sint (nttpackv a{hr}).[i] -  3329.
++  rewrite to_sintB_small /=;1: by rewrite  /(to_sint (W16.of_int 3329))  /= /smod /=;smt(size_map size_iota). 
+   by rewrite  /(to_sint (W16.of_int 3329))  /= /smod /=; smt(size_map size_iota W16.to_uint_cmp).
+
+have -> : (incoeff (to_sint (nttpackv a{hr}).[i])) = (incoeff (to_sint (W16_sub (nttpackv a{hr}).[i] (W16.of_int 3329)))) by  rewrite -eq_incoeff; smt(). 
+
++ rewrite  /truncateu12;congr. 
+  rewrite incoeffK qE modz_small;smt(W16.to_uint_cmp). 
+ 
+qed.
+
+lemma auxtobytes_ll : islossless AuxToBytes.__i_polyvec_tobytes.
+proc.
+inline *. 
+do 9!(unroll for ^while); auto. 
+qed.
+
+lemma auxtobytes_corr (_aw : W16.t Array1024.t):
+    phoare[ AuxToBytes.__i_polyvec_tobytes :
+             pos_bound1024_cxq a 0 1024 2 /\ a = _aw ==> 
+    res = encode12_vec (map asint (lift_array1024 (nttpackv _aw)))] = 1%r
+  by conseq auxtobytes_ll (auxtobytes_corr_h _aw).
+
+
+lemma polyvec_tobytes_corr (_aw : W16.t Array1024.t):
+    phoare[ Jkem1024_avx2.M.__i_polyvec_tobytes :
+             pos_bound1024_cxq a 0 1024 2 /\ a = _aw ==> 
+    res = encode12_vec (map asint (lift_array1024 (nttpackv _aw)))] = 1%r.
+proof.
+bypr => &m [??].
+have <- : Pr[AuxToBytes.__i_polyvec_tobytes(r{m}, _aw) @ &m : res = encode12_vec (map asint (lift_array1024 (nttpackv _aw)))] = 1%r
+ by byphoare (auxtobytes_corr _aw)  =>/=; 1:smt().
+byequiv (: ={arg} /\ a{1} = _aw /\
+             pos_bound1024_cxq a{1} 0 1024 2 ==> ={res}) => //.
+proc => /=. 
+inline M._i_poly_tobytes.
+while (={r, a,i} /\ 0 <= i{1} <= 4 /\
+   pos_bound1024_cxq a{1} 0 1024 2); last by auto => /> /#.
+seq 3 3 : (#pre /\ ={rp,a0} /\
+   pos_bound256_cxq a0{1} 0 256 1).
++ ecall {1} (poly_csubq_avx2_corr a0{1}).
+  ecall {2} (poly_csubq_avx2_corr a0{2}).
+  auto => /> &1; rewrite /pos_bound1024_cxq /pos_bound256_cxq /lift_array256 /= qE /= => ????;split; 1: by smt(Array256.initiE).
+  move => ? rr1.
+  rewrite !tP;move =>  Hrr11 Hrr12 rr2.
+  rewrite !tP;move =>  Hrr21 Hrr22.
+  move => ii iib. 
+  have := Hrr11 ii iib; rewrite !mapiE 1,2:/# /=. 
+  have := Hrr12 ii iib.  
+  have := Hrr21 ii iib; rewrite !mapiE 1,2:/# /=. 
+  have := Hrr22 ii iib.  
+  rewrite /to_sint /smod /=. 
+  move => Hrr11i Hrr12i Hrr21i Hrr22i.
+  have Hn1 : !(32768 <= to_uint rr2.[ii]) by smt(W16.to_uint_cmp pow2_16).
+  have Hn2 : !(32768 <= to_uint rr1.[ii]) by smt(W16.to_uint_cmp pow2_16).
+  have Hn3 : !(32768 <= to_uint _aw.[ii]) by smt(W16.to_uint_cmp pow2_16).
+  move : Hrr11i Hrr12i Hrr21i Hrr22i; rewrite Hn1 Hn2 /=.
+  move => Hrr11i Hrr12i Hrr21i Hrr22i.
+  move : Hrr12i; rewrite -Hrr22i -eq_incoeff.  
+  by rewrite !modz_small ?qE /= 1,2:/# to_uint_eq /#.
+
+wp;while (#pre /\ ={i0} /\ 0<=i0{1}<=2); last first.
++ auto => /> &2 ?????i0r????;split;1:smt().
+  rewrite /pos_bound1024_cxq => k kb; rewrite initiE 1:/# /= /#.
+
+wp -1 -1; conseq (: _ ==> ={rp}); 1: by smt().
+
+inline *;sim; auto => /> &1 &2 ???;rewrite /pos_bound256_cxq qE /= => Hb ???.
+
+have Hpos : forall jj kk ii, 0 <= jj < 8 => 0 <= kk < 16 => 0 <= ii < 16 => (get256 (WArray512.init16 ("_.[_]" a0{1})) (8 * i0{1} + jj) \bits16 kk).[ii] = a0{1}.[kk + 16*jj + i0{1}*128].[ii] by
+  move => jj kk ii jjb kkb iib; rewrite get256E /pack32_t /(\bits16) initiE 1:/# /= initiE 1:/# /= initiE 1:/# /= initiE 1:/# /= /(\bits8) initiE 1:/# /= /#.
+
+have bits : forall kk ii, 0 <= kk < 256 => 12 <= ii < 16 => !a0{1}.[kk].[ii].
++ move => kk ii kkb iib; have := Hb kk kkb;rewrite /to_sint /smod /= => Hn.
+  have Hn1 : !32768 <= to_uint a0{1}.[kk] by smt(W16.to_uint_cmp pow2_16).
+  move : Hn; rewrite Hn1 /= get_to_uint . 
+  have ? : 4096 <= 2^ii;last by smt().
+  have ? : 4096 = 2^12 by auto.
+  smt(@StdOrder.IntOrder). 
+
+have bitsC : forall  ii, 0 <= ii < 16 => (W16.of_int 4095).[ii] <=> 0<=ii<12.
++ move => ii iib.
+  have : all (fun i => (W16.of_int 4095).[i] <=> 0 <= i < 12) (iota_ 0 16); 
+  last by rewrite allP => H; move : (H ii _);smt(mem_iota).
+  by rewrite -iotaredE /= !get_to_uint /=.
+
+
+do split; rewrite /VPBROADCAST_16u16 /= -(W16u16.unpack16K (WArray512.get256 _ _)) -(W16u16.unpack16K (W16u16.pack16 _)) !andb16u16E;congr;rewrite packP => k kb;rewrite map2iE 1:/# /= andE wordP => ii iib;rewrite map2iE 1:/# /= get_of_list 1:/# /= (nth_map witness)  /=;1,3,5,7,9,11,13,15:smt(size_iota); rewrite unpack16E initiE 1:/# /=;1..7: by rewrite Hpos /#.
+      have /= -> := Hpos 0;smt().
+qed.
+
+
+lemma polyvec_tobytes_equiv :
+    equiv [Jkem1024_avx2.M.__i_polyvec_tobytes ~Jkem1024.M.__i_polyvec_tobytes :
+             pos_bound1024_cxq a{1} 0 1024 2 /\
+             pos_bound1024_cxq a{2} 0 1024 2 /\
+             lift_array1024 a{1} = nttunpackv (lift_array1024 a{2}) ==> ={res} ].
+proof.
+proc*.
+ecall{1} (polyvec_tobytes_corr a{1}).
+ecall{2} (MLKEM_PolyVec.polyvec_tobytes_corr a{2}).
+by auto => /> &1 &2 ??; rewrite -nttpackv_lift => ->; rewrite  unpackvK.
+qed.
+
 
 lemma polyvec_add2_equiv  (ab bb : int):
     0 <= ab && ab <= 6 =>
     0 <= bb && bb <= 3 =>
-  forall (_a _b : coeff Array768.t),
-    equiv [Jkem768_avx2.M.__polyvec_add2 ~Jkem768.M.__polyvec_add2 :
-      _a = lift_array768 r{2} /\
-      _b = lift_array768 b{2} /\ signed_bound768_cxq r{2} 0 768 ab /\ signed_bound768_cxq b{2} 0 768 bb /\
-      _a = nttpackv (lift_array768 r{1}) /\
-      _b = nttpackv (lift_array768 b{1}) /\ signed_bound768_cxq r{1} 0 768 ab /\ signed_bound768_cxq b{1} 0 768 bb
-           ==> lift_array768 res{1} = nttunpackv (lift_array768  res{2}) /\
-               signed_bound768_cxq res{1} 0 768 (ab + bb) /\
-               signed_bound768_cxq res{2} 0 768 (ab + bb) 
+  forall (_a _b : coeff Array1024.t),
+    equiv [Jkem1024_avx2.M.__polyvec_add2 ~Jkem1024.M.__polyvec_add2 :
+      _a = lift_array1024 r{2} /\
+      _b = lift_array1024 b{2} /\ signed_bound1024_cxq r{2} 0 1024 ab /\ signed_bound1024_cxq b{2} 0 1024 bb /\
+      _a = nttpackv (lift_array1024 r{1}) /\
+      _b = nttpackv (lift_array1024 b{1}) /\ signed_bound1024_cxq r{1} 0 1024 ab /\ signed_bound1024_cxq b{1} 0 1024 bb
+           ==> lift_array1024 res{1} = nttunpackv (lift_array1024  res{2}) /\
+               signed_bound1024_cxq res{1} 0 1024 (ab + bb) /\
+               signed_bound1024_cxq res{2} 0 1024 (ab + bb) 
               ].
 proof. 
 move => abb bbb _a _b;proc* => /=.
 transitivity {1} {r0 <@ MLKEM_PolyVec_avx2_prevec.Mprevec.polyvec_add2(r,b); }
        (={r,b} ==> ={r0})
-       (_a = lift_array768 r{2} /\
-  _b = lift_array768 b{2} /\
-  signed_bound768_cxq r{2} 0 768 ab /\
-  signed_bound768_cxq b{2} 0 768 bb /\
-  _a = nttpackv (lift_array768 r{1}) /\
-  _b = nttpackv (lift_array768 b{1}) /\ signed_bound768_cxq r{1} 0 768 ab /\ signed_bound768_cxq b{1} 0 768 bb   ==> 
-      lift_array768 r0{1} = nttunpackv (lift_array768 r0{2}) /\ signed_bound768_cxq r0{1} 0 768 (ab + bb) /\ signed_bound768_cxq r0{2} 0 768 (ab + bb)); 1,2: by smt().
+       (_a = lift_array1024 r{2} /\
+  _b = lift_array1024 b{2} /\
+  signed_bound1024_cxq r{2} 0 1024 ab /\
+  signed_bound1024_cxq b{2} 0 1024 bb /\
+  _a = nttpackv (lift_array1024 r{1}) /\
+  _b = nttpackv (lift_array1024 b{1}) /\ signed_bound1024_cxq r{1} 0 1024 ab /\ signed_bound1024_cxq b{1} 0 1024 bb   ==> 
+      lift_array1024 r0{1} = nttunpackv (lift_array1024 r0{2}) /\ signed_bound1024_cxq r0{1} 0 1024 (ab + bb) /\ signed_bound1024_cxq r0{2} 0 1024 (ab + bb)); 1,2: by smt().
   + symmetry. call prevec_eq_polyvec_add2 => //.
 have corr1 := (polvec_add_corr (nttunpackv _a) (nttunpackv _b) ab bb abb bbb). call {1} corr1.
 have corr2 := (polyvec_add_corr _a _b ab bb abb bbb); call {2} corr2.
@@ -515,10 +2710,10 @@ auto => />.
 move => &1 &2 ????->->??rr?rval; do split; 1,2: by rewrite packvK.  
 move => ??rr0?r0val.
 rewrite tP => k kb.
-rewrite /(lift_array768 rr0) mapiE //= r0val // !packvK.
-have  -> : lift_array768 rr = 
-   Array768.init (fun k => (nttpackv (lift_array768 r{1})).[k] + (nttpackv (lift_array768 b{1})).[k])
- by rewrite tP => kk kkb; rewrite initiE //= /(lift_array768 rr) mapiE //= /#.
+rewrite /(lift_array1024 rr0) mapiE //= r0val // !packvK.
+have  -> : lift_array1024 rr = 
+   Array1024.init (fun k => (nttpackv (lift_array1024 r{1})).[k] + (nttpackv (lift_array1024 b{1})).[k])
+ by rewrite tP => kk kkb; rewrite initiE //= /(lift_array1024 rr) mapiE //= /#.
 rewrite /nttunpackv /nttpackv initiE //=.
 case (0<=k<256).
 + move => *.
@@ -549,14 +2744,35 @@ case (256<=k<512).
   rewrite initiE //=;1: smt(nttpack_bnd nttunpack_bnd Array256.allP).
   move : nttpack_idxK; rewrite allP; smt(mem_iota).  
 
+case (512<=k<768).
 + move => *.
   rewrite /subarray256 /nttunpack initiE //=;1: smt(nttunpack_bnd Array256.allP).
-  pose a := nttunpack_idx.[k - 512].
+  pose a := nttunpack_idx.[k-512].
+  do 3!(rewrite  /nttpack initiE //=;1: smt(nttpack_bnd nttunpack_bnd Array256.allP)).
+  rewrite ifF; 1: smt(nttunpack_bnd Array256.allP). 
+  rewrite ifF; 1: smt(nttunpack_bnd Array256.allP). 
+  rewrite ifT; 1: smt(nttunpack_bnd Array256.allP). 
+  do 2!(rewrite  /nttpack initiE //=;1: smt(nttpack_bnd nttunpack_bnd Array256.allP)).
+  pose b := nttpack_idx.[a].
+  rewrite initiE //=;1: smt(nttpack_bnd nttunpack_bnd Array256.allP).
+  rewrite ifF; 1: smt(nttunpack_bnd Array256.allP). 
+  rewrite ifF; 1: smt(nttunpack_bnd Array256.allP). 
+  rewrite ifT; 1: smt(nttunpack_bnd Array256.allP). 
+  rewrite initiE //=;1: smt(nttpack_bnd nttunpack_bnd Array256.allP).
+  rewrite -/b.
+  rewrite initiE //=;1: smt(nttpack_bnd nttunpack_bnd Array256.allP).
+  move : nttpack_idxK; rewrite allP; smt(mem_iota).  
+
++ move => *.
+  rewrite /subarray256 /nttunpack initiE //=;1: smt(nttunpack_bnd Array256.allP).
+  pose a := nttunpack_idx.[k - 768].
   do 4!(rewrite initiE //=; 1:smt(nttunpack_bnd Array256.allP)).
+  rewrite ifF;1: smt(nttunpack_bnd Array256.allP).
   rewrite ifF;1: smt(nttunpack_bnd Array256.allP).
   rewrite ifF;1: smt(nttunpack_bnd Array256.allP).
   do 2!(rewrite /nttpack initiE //=;1: smt(nttpack_bnd nttunpack_bnd Array256.allP)).
   pose b := nttpack_idx.[a].
+  rewrite ifF;1: smt(nttunpack_bnd Array256.allP).
   rewrite ifF;1: smt(nttunpack_bnd Array256.allP).
   rewrite ifF;1: smt(nttunpack_bnd Array256.allP).
   do 2!(rewrite initiE //=;1: smt(nttpack_bnd nttunpack_bnd Array256.allP)).
@@ -567,50 +2783,50 @@ qed.
 lemma polyvec_add2_equiv_noperm  (ab bb : int):
     0 <= ab && ab <= 6 =>
     0 <= bb && bb <= 3 =>
-  forall (_a _b : coeff Array768.t),
-    equiv [Jkem768_avx2.M.__polyvec_add2 ~Jkem768.M.__polyvec_add2 :
-      _a = lift_array768 r{2} /\
-      _b = lift_array768 b{2} /\ signed_bound768_cxq r{2} 0 768 ab /\ signed_bound768_cxq b{2} 0 768 bb /\
-      _a = lift_array768 r{1} /\
-      _b = lift_array768 b{1} /\ signed_bound768_cxq r{1} 0 768 ab /\ signed_bound768_cxq b{1} 0 768 bb
-           ==> lift_array768 res{1} = lift_array768  res{2} /\
-               signed_bound768_cxq res{1} 0 768 (ab + bb) /\
-               signed_bound768_cxq res{2} 0 768 (ab + bb) 
+  forall (_a _b : coeff Array1024.t),
+    equiv [Jkem1024_avx2.M.__polyvec_add2 ~Jkem1024.M.__polyvec_add2 :
+      _a = lift_array1024 r{2} /\
+      _b = lift_array1024 b{2} /\ signed_bound1024_cxq r{2} 0 1024 ab /\ signed_bound1024_cxq b{2} 0 1024 bb /\
+      _a = lift_array1024 r{1} /\
+      _b = lift_array1024 b{1} /\ signed_bound1024_cxq r{1} 0 1024 ab /\ signed_bound1024_cxq b{1} 0 1024 bb
+           ==> lift_array1024 res{1} = lift_array1024  res{2} /\
+               signed_bound1024_cxq res{1} 0 1024 (ab + bb) /\
+               signed_bound1024_cxq res{2} 0 1024 (ab + bb) 
               ].
 proof. 
 move => abb bbb _a _b;proc* => /=.
 transitivity {1} {r0 <@ MLKEM_PolyVec_avx2_prevec.Mprevec.polyvec_add2(r,b); }
        (={r,b} ==> ={r0})
-       (_a = lift_array768 r{2} /\
-  _b = lift_array768 b{2} /\
-  signed_bound768_cxq r{2} 0 768 ab /\
-  signed_bound768_cxq b{2} 0 768 bb /\
-  _a =  (lift_array768 r{1}) /\
-  _b =  (lift_array768 b{1}) /\ signed_bound768_cxq r{1} 0 768 ab /\ signed_bound768_cxq b{1} 0 768 bb   ==> 
-      lift_array768 r0{1} = (lift_array768 r0{2}) /\ signed_bound768_cxq r0{1} 0 768 (ab + bb) /\ signed_bound768_cxq r0{2} 0 768 (ab + bb)); 1,2: by smt().
+       (_a = lift_array1024 r{2} /\
+  _b = lift_array1024 b{2} /\
+  signed_bound1024_cxq r{2} 0 1024 ab /\
+  signed_bound1024_cxq b{2} 0 1024 bb /\
+  _a =  (lift_array1024 r{1}) /\
+  _b =  (lift_array1024 b{1}) /\ signed_bound1024_cxq r{1} 0 1024 ab /\ signed_bound1024_cxq b{1} 0 1024 bb   ==> 
+      lift_array1024 r0{1} = (lift_array1024 r0{2}) /\ signed_bound1024_cxq r0{1} 0 1024 (ab + bb) /\ signed_bound1024_cxq r0{2} 0 1024 (ab + bb)); 1,2: by smt().
   + symmetry. call prevec_eq_polyvec_add2 => //.
 have corr1 := (polvec_add_corr ( _a) ( _b) ab bb abb bbb). call {1} corr1.
 have corr2 := (polyvec_add_corr _a _b ab bb abb bbb); call {2} corr2.
 
 auto => />.  
 move => &1 &2 ????????rr? H rval? H0. 
-move : H H0; rewrite /lift_array768 !tP => ? ? k kb. 
-rewrite !mapiE;smt(Array768.mapiE).
+move : H H0; rewrite /lift_array1024 !tP => ? ? k kb. 
+rewrite !mapiE;smt(Array1024.mapiE).
 qed.
 
 lemma polyvec_reduce_equiv _a :
-    equiv [Jkem768_avx2.M.__polyvec_reduce ~Jkem768.M.__polyvec_reduce :
-       _a  = lift_array768 r{2} /\  _a  = nttpackv (lift_array768 r{1})  ==>
-       (forall k, 0 <= k < 768 => bpos16 res{1}.[k] (2*q)) /\
-       (forall k, 0 <= k < 768 => bpos16 res{2}.[k] (2*q)) /\
-              lift_array768 res{1} = nttunpackv (lift_array768 res{2}) ].
+    equiv [Jkem1024_avx2.M.__polyvec_reduce ~Jkem1024.M.__polyvec_reduce :
+       _a  = lift_array1024 r{2} /\  _a  = nttpackv (lift_array1024 r{1})  ==>
+       (forall k, 0 <= k < 1024 => bpos16 res{1}.[k] (2*q)) /\
+       (forall k, 0 <= k < 1024 => bpos16 res{2}.[k] (2*q)) /\
+              lift_array1024 res{1} = nttunpackv (lift_array1024 res{2}) ].
 proc*. 
 transitivity {1} {r0 <@ MLKEM_PolyVec_avx2_prevec.Mprevec.polyvec_reduce(r); }
        (={r} ==> ={r0})
-       (_a = lift_array768 r{2} /\ _a = nttpackv (lift_array768 r{1})   ==> 
-      (forall (k : int), 0 <= k && k < 768 => bpos16 r0{1}.[k] (2 * q)) /\
-  (forall (k : int), 0 <= k && k < 768 => bpos16 r0{2}.[k] (2 * q)) /\
-  lift_array768 r0{1} = nttunpackv (lift_array768  r0{2})); 1,2: by smt().
+       (_a = lift_array1024 r{2} /\ _a = nttpackv (lift_array1024 r{1})   ==> 
+      (forall (k : int), 0 <= k && k < 1024 => bpos16 r0{1}.[k] (2 * q)) /\
+  (forall (k : int), 0 <= k && k < 1024 => bpos16 r0{2}.[k] (2 * q)) /\
+  lift_array1024 r0{1} = nttunpackv (lift_array1024  r0{2})); 1,2: by smt().
   + symmetry. call prevec_eq_polyvec_reduce => //.
 have corr1 := (polvec_reduce_corr (nttunpackv _a)). call {1} corr1.
 have corr2 := (polyvec_reduce_corr _a); call {2} corr2.
@@ -623,18 +2839,18 @@ qed.
 
 
 lemma polyvec_reduce_equiv_noperm _a :
-    equiv [Jkem768_avx2.M.__polyvec_reduce ~Jkem768.M.__polyvec_reduce :
-       _a  = lift_array768 r{2} /\  _a  = lift_array768 r{1}  ==>
-       (forall k, 0 <= k < 768 => bpos16 res{1}.[k] (2*q)) /\
-       (forall k, 0 <= k < 768 => bpos16 res{2}.[k] (2*q)) /\
-              lift_array768 res{1} =  lift_array768 res{2} ].
+    equiv [Jkem1024_avx2.M.__polyvec_reduce ~Jkem1024.M.__polyvec_reduce :
+       _a  = lift_array1024 r{2} /\  _a  = lift_array1024 r{1}  ==>
+       (forall k, 0 <= k < 1024 => bpos16 res{1}.[k] (2*q)) /\
+       (forall k, 0 <= k < 1024 => bpos16 res{2}.[k] (2*q)) /\
+              lift_array1024 res{1} =  lift_array1024 res{2} ].
 proc*. 
 transitivity {1} {r0 <@ MLKEM_PolyVec_avx2_prevec.Mprevec.polyvec_reduce(r); }
        (={r} ==> ={r0})
-       (_a = lift_array768 r{2} /\ _a = (lift_array768 r{1})   ==> 
-      (forall (k : int), 0 <= k && k < 768 => bpos16 r0{1}.[k] (2 * q)) /\
-  (forall (k : int), 0 <= k && k < 768 => bpos16 r0{2}.[k] (2 * q)) /\
-  lift_array768 r0{1} =  (lift_array768  r0{2})); 1,2: by smt().
+       (_a = lift_array1024 r{2} /\ _a = (lift_array1024 r{1})   ==> 
+      (forall (k : int), 0 <= k && k < 1024 => bpos16 r0{1}.[k] (2 * q)) /\
+  (forall (k : int), 0 <= k && k < 1024 => bpos16 r0{2}.[k] (2 * q)) /\
+  lift_array1024 r0{1} =  (lift_array1024  r0{2})); 1,2: by smt().
   + symmetry. call prevec_eq_polyvec_reduce => //.
 have corr1 := (polvec_reduce_corr ( _a)). call {1} corr1.
 have corr2 := (polyvec_reduce_corr _a); call {2} corr2.
@@ -643,13 +2859,13 @@ auto => /> /#.
 qed.
 
 equiv pointwiseequiv : 
- Jkem768_avx2.M.__polyvec_pointwise_acc ~  Jkem768.M.__polyvec_pointwise_acc :
-    lift_array768 arg{1}.`2 = nttunpackv (lift_array768 arg{2}.`1) /\
-    lift_array768 arg{1}.`3 = nttunpackv (lift_array768 arg{2}.`2) /\
-    signed_bound768_cxq arg{1}.`2 0 768 2 /\
-    signed_bound768_cxq arg{1}.`3 0 768 2 /\
-    signed_bound768_cxq arg{2}.`1 0 768 2 /\
-    signed_bound768_cxq arg{2}.`2 0 768 2
+ Jkem1024_avx2.M.__polyvec_pointwise_acc ~  Jkem1024.M.__polyvec_pointwise_acc :
+    lift_array1024 arg{1}.`2 = nttunpackv (lift_array1024 arg{2}.`1) /\
+    lift_array1024 arg{1}.`3 = nttunpackv (lift_array1024 arg{2}.`2) /\
+    signed_bound1024_cxq arg{1}.`2 0 1024 2 /\
+    signed_bound1024_cxq arg{1}.`3 0 1024 2 /\
+    signed_bound1024_cxq arg{2}.`1 0 1024 2 /\
+    signed_bound1024_cxq arg{2}.`2 0 1024 2
     ==> 
     lift_array256 res{1} = nttunpack (lift_array256 res{2}) /\
     signed_bound_cxq res{1} 0 256 4 /\ 
@@ -659,7 +2875,7 @@ proc => /=.
 seq 2 3 :(#pre /\ 
          lift_array256 r{1} = nttunpack (lift_array256 r{2}) /\
          signed_bound_cxq r{1} 0 256 1 /\
-         signed_bound_cxq r{2} 0 256 3).
+         signed_bound_cxq r{2} 0 256 2).
 ecall (basemulequiv). auto => />.
 move => &1 &2 H H0 H1 H2 H3 H4. do split. 
 + move : H; rewrite /nttunpackv -lift256_nttunpack /lift_array256 !tP => H k kb.
@@ -667,27 +2883,27 @@ move => &1 &2 H H0 H1 H2 H3 H4. do split.
   rewrite /nttunpack !mapiE //= 1:/# !initiE//=.
   pose a := nttunpack_idx.[k].
   rewrite !initiE//=; 1,2: smt(nttunpack_bnd Array256.allP). 
-  rewrite /lift_array768;smt(Array768.mapiE nttunpack_bnd Array256.allP).
+  rewrite /lift_array1024;smt(Array1024.mapiE nttunpack_bnd Array256.allP).
 + move : H0; rewrite /nttunpackv -lift256_nttunpack /lift_array256 !tP => H0 k kb.
   move : (H0 k _); 1: smt(). rewrite !initiE//= 1:/# kb /=.
   rewrite /nttunpack !mapiE //= 1:/# !initiE//=.
   pose a := nttunpack_idx.[k].
   rewrite !initiE//=; 1,2: smt(nttunpack_bnd Array256.allP). 
-  rewrite /lift_array768;smt(Array768.mapiE nttunpack_bnd Array256.allP).
-+ move : H1; rewrite /signed_bound768_cxq /signed_bound_cxq /nttunpackv => H1 k kb.
+  rewrite /lift_array1024;smt(Array1024.mapiE nttunpack_bnd Array256.allP).
++ move : H1; rewrite /signed_bound1024_cxq /signed_bound_cxq /nttunpackv => H1 k kb.
   move : (H1 k _); 1: smt(). rewrite !initiE//=.
-move : H2; rewrite /signed_bound768_cxq /signed_bound_cxq /nttunpackv => H2 k kb.
+move : H2; rewrite /signed_bound1024_cxq /signed_bound_cxq /nttunpackv => H2 k kb.
 move : (H2 k _); 1: smt(). rewrite !initiE//=.
-+ move : H3; rewrite /signed_bound768_cxq /signed_bound_cxq /nttunpackv => H3 k kb.
++ move : H3; rewrite /signed_bound1024_cxq /signed_bound_cxq /nttunpackv => H3 k kb.
   move : (H3 k _); 1: smt(). rewrite !initiE//=.
-move : H4; rewrite /signed_bound768_cxq /signed_bound_cxq /nttunpackv => H4 k kb.
+move : H4; rewrite /signed_bound1024_cxq /signed_bound_cxq /nttunpackv => H4 k kb.
 move : (H4 k _); 1: smt(). rewrite !initiE//=.
 
 unroll for {1} 2; unroll for {2} 2.
 seq 1 1 :(#pre /\ 
          lift_array256 t{1} = nttunpack (lift_array256 t{2}) /\
          signed_bound_cxq t{1} 0 256 1 /\
-         signed_bound_cxq t{2} 0 256 3).
+         signed_bound_cxq t{2} 0 256 2).
 ecall (basemulequiv). auto => />.
 move => &1 &2 H H0 H1 H2 H3 H4 H5 H6 H7. do split. 
 + move : H; rewrite /nttunpackv -lift256_nttunpack /lift_array256 !tP => H k kb.
@@ -695,27 +2911,27 @@ move => &1 &2 H H0 H1 H2 H3 H4 H5 H6 H7. do split.
   rewrite ifF 1:/# /nttunpack !mapiE //= 1:/# ifT 1:/# !initiE//=. 
   pose a := nttunpack_idx.[k].
   rewrite !initiE//=; 1,2: smt(nttunpack_bnd Array256.allP). 
-  rewrite /lift_array768;smt(Array768.mapiE nttunpack_bnd Array256.allP).
+  rewrite /lift_array1024;smt(Array1024.mapiE nttunpack_bnd Array256.allP).
 + move : H0; rewrite /nttunpackv -lift256_nttunpack /lift_array256 !tP => H0 k kb.
   move : (H0 (256+k) _); 1: smt(). rewrite !initiE//= 1:/# /=.
   rewrite ifF 1:/# /nttunpack !mapiE //= 1:/# ifT 1:/# !initiE//=. 
   pose a := nttunpack_idx.[k].
   rewrite !initiE//=; 1,2: smt(nttunpack_bnd Array256.allP). 
-  rewrite /lift_array768;smt(Array768.mapiE nttunpack_bnd Array256.allP).
-+ move : H1; rewrite /signed_bound768_cxq /signed_bound_cxq /nttunpackv => H1 k kb.
+  rewrite /lift_array1024;smt(Array1024.mapiE nttunpack_bnd Array256.allP).
++ move : H1; rewrite /signed_bound1024_cxq /signed_bound_cxq /nttunpackv => H1 k kb.
   move : (H1 k _); 1: smt(). rewrite !initiE//=;1: smt().
-move : H2; rewrite /signed_bound768_cxq /signed_bound_cxq /nttunpackv => H2 k kb.
+move : H2; rewrite /signed_bound1024_cxq /signed_bound_cxq /nttunpackv => H2 k kb.
 move : (H2 k _); 1: smt(). rewrite !initiE//=;1: smt().
-+ move : H3; rewrite /signed_bound768_cxq /signed_bound_cxq /nttunpackv => H3 k kb.
++ move : H3; rewrite /signed_bound1024_cxq /signed_bound_cxq /nttunpackv => H3 k kb.
   move : (H3 k _); 1: smt(). rewrite !initiE//=;1: smt().
-move : H4; rewrite /signed_bound768_cxq /signed_bound_cxq /nttunpackv => H4 k kb.
+move : H4; rewrite /signed_bound1024_cxq /signed_bound_cxq /nttunpackv => H4 k kb.
 move : (H4 k _); 1: smt(). rewrite !initiE//=;1:smt().
 
 seq 1 1 :(#{/~r{2}}{~r{1}}{~t{2}}{~t{1}}pre /\ 
          lift_array256 r{1} = nttunpack (lift_array256 r{2}) /\
          signed_bound_cxq r{1} 0 256 2 /\
-         signed_bound_cxq r{2} 0 256 6).
-have Hcall:= addequiv 1 1 3 3 _ _ => //.
+         signed_bound_cxq r{2} 0 256 4).
+have Hcall:= addequiv 1 1 2 2 _ _ => //.
 call Hcall.
 auto => />.
 move => &1 &2 H H0 H1 H2 H3 H4 H5 H6 H7 H8 H9 H10. do split. 
@@ -727,36 +2943,77 @@ rewrite -lift256_nttunpack;1: assumption.
 seq 1 1 :(#pre /\ 
          lift_array256 t{1} = nttunpack (lift_array256 t{2}) /\
          signed_bound_cxq t{1} 0 256 1 /\
-         signed_bound_cxq t{2} 0 256 3).
+         signed_bound_cxq t{2} 0 256 2).
 ecall (basemulequiv). auto => />.
 move => &1 &2 H H0 H1 H2 H3 H4 H5 H6 H7. do split. 
 + move : H; rewrite /nttunpackv -lift256_nttunpack /lift_array256 !tP => H k kb.
   move : (H (512+k) _); 1: smt(). rewrite !initiE//= 1:/# /=.
-  rewrite ifF 1:/# /nttunpack !mapiE //= 1:/# ifF 1:/# !initiE//=. 
+  rewrite ifF 1:/# /= ifF 1:/# ifT 1:/# /nttunpack !mapiE //= 1:/#  !initiE//=. 
   pose a := nttunpack_idx.[k].
   rewrite !initiE//=; 1,2: smt(nttunpack_bnd Array256.allP). 
-  rewrite /lift_array768;smt(Array768.mapiE nttunpack_bnd Array256.allP).
+  rewrite /lift_array1024;smt(Array1024.mapiE nttunpack_bnd Array256.allP).
 + move : H0; rewrite /nttunpackv -lift256_nttunpack /lift_array256 !tP => H0 k kb.
   move : (H0 (512+k) _); 1: smt(). rewrite !initiE//= 1:/# /=.
-  rewrite ifF 1:/# /nttunpack !mapiE //= 1:/# ifF 1:/# !initiE//=. 
+  rewrite ifF 1:/# /= ifF 1:/# ifT 1:/# /nttunpack !mapiE //= 1:/#  !initiE//=. 
   pose a := nttunpack_idx.[k].
   rewrite !initiE//=; 1,2: smt(nttunpack_bnd Array256.allP). 
-  rewrite /lift_array768;smt(Array768.mapiE nttunpack_bnd Array256.allP).
-+ move : H1; rewrite /signed_bound768_cxq /signed_bound_cxq /nttunpackv => H1 k kb.
+  rewrite /lift_array1024;smt(Array1024.mapiE nttunpack_bnd Array256.allP).
++ move : H1; rewrite /signed_bound1024_cxq /signed_bound_cxq /nttunpackv => H1 k kb.
   move : (H1 k _); 1: smt(). rewrite !initiE//=;1: smt().
-move : H2; rewrite /signed_bound768_cxq /signed_bound_cxq /nttunpackv => H2 k kb.
+move : H2; rewrite /signed_bound1024_cxq /signed_bound_cxq /nttunpackv => H2 k kb.
 move : (H2 k _); 1: smt(). rewrite !initiE//=;1: smt().
-+ move : H3; rewrite /signed_bound768_cxq /signed_bound_cxq /nttunpackv => H3 k kb.
++ move : H3; rewrite /signed_bound1024_cxq /signed_bound_cxq /nttunpackv => H3 k kb.
   move : (H3 k _); 1: smt(). rewrite !initiE//=;1: smt().
-move : H4; rewrite /signed_bound768_cxq /signed_bound_cxq /nttunpackv => H4 k kb.
+move : H4; rewrite /signed_bound1024_cxq /signed_bound_cxq /nttunpackv => H4 k kb.
 move : (H4 k _); 1: smt(). rewrite !initiE//=;1: smt().
 
 
 seq 1 1 :(#{/~r{2}}{~r{1}}{~t{2}}{~t{1}}pre /\ 
          lift_array256 r{1} = nttunpack (lift_array256 r{2}) /\
          signed_bound_cxq r{1} 0 256 3 /\
-         signed_bound_cxq r{2} 0 256 9).
-have Hcall:= addequiv 2 1 6 3 _ _ => //.
+         signed_bound_cxq r{2} 0 256 6).
+have Hcall:= addequiv 2 1 4 2 _ _ => //.
+call Hcall.
+auto => />.
+move => &1 &2 ????????????. do split. 
++ rewrite lift256_nttunpack;1: assumption.
++ rewrite lift256_nttunpack;1: assumption.
+move => ?? r1 r2 ???.
+rewrite -lift256_nttunpack;1: assumption.
+
+seq 1 1 :(#pre /\ 
+         lift_array256 t{1} = nttunpack (lift_array256 t{2}) /\
+         signed_bound_cxq t{1} 0 256 1 /\
+         signed_bound_cxq t{2} 0 256 2).
+ecall (basemulequiv). auto => />.
+move => &1 &2 H H0 H1 H2 H3 H4 H5 H6 H7. do split. 
++ move : H; rewrite /nttunpackv -lift256_nttunpack /lift_array256 !tP => H k kb.
+  move : (H (768+k) _); 1: smt(). rewrite !initiE//= 1:/# /=.
+  rewrite ifF 1:/# /= ifF 1:/# ifF 1:/# /nttunpack !mapiE //= 1:/#  !initiE//=. 
+  pose a := nttunpack_idx.[k].
+  rewrite !initiE//=; 1,2: smt(nttunpack_bnd Array256.allP). 
+  rewrite /lift_array1024;smt(Array1024.mapiE nttunpack_bnd Array256.allP).
++ move : H0; rewrite /nttunpackv -lift256_nttunpack /lift_array256 !tP => H0 k kb.
+  move : (H0 (768+k) _); 1: smt(). rewrite !initiE//= 1:/# /=.
+  rewrite ifF 1:/# /= ifF 1:/# ifF 1:/# /nttunpack !mapiE //= 1:/#  !initiE//=. 
+  pose a := nttunpack_idx.[k].
+  rewrite !initiE//=; 1,2: smt(nttunpack_bnd Array256.allP). 
+  rewrite /lift_array1024;smt(Array1024.mapiE nttunpack_bnd Array256.allP).
++ move : H1; rewrite /signed_bound1024_cxq /signed_bound_cxq /nttunpackv => H1 k kb.
+  move : (H1 k _); 1: smt(). rewrite !initiE//=;1: smt().
+move : H2; rewrite /signed_bound1024_cxq /signed_bound_cxq /nttunpackv => H2 k kb.
+move : (H2 k _); 1: smt(). rewrite !initiE//=;1: smt().
++ move : H3; rewrite /signed_bound1024_cxq /signed_bound_cxq /nttunpackv => H3 k kb.
+  move : (H3 k _); 1: smt(). rewrite !initiE//=;1: smt().
+move : H4; rewrite /signed_bound1024_cxq /signed_bound_cxq /nttunpackv => H4 k kb.
+move : (H4 k _); 1: smt(). rewrite !initiE//=;1: smt().
+
+
+seq 1 1 :(#{/~r{2}}{~r{1}}{~t{2}}{~t{1}}pre /\ 
+         lift_array256 r{1} = nttunpack (lift_array256 r{2}) /\
+         signed_bound_cxq r{1} 0 256 4 /\
+         signed_bound_cxq r{2} 0 256 8).
+have Hcall:= addequiv 3 1 6 2 _ _ => //.
 call Hcall.
 auto => />.
 move => &1 &2 ????????????. do split. 
@@ -775,13 +3032,13 @@ smt().
 qed.
 
 equiv nttequiv :
-Jkem768_avx2.M.__polyvec_ntt ~Jkem768.M.__polyvec_ntt : 
-   lift_array768 arg{1} = lift_array768 arg{2} /\ 
-   signed_bound768_cxq arg{1} 0 768 2 /\ 
-   signed_bound768_cxq arg{2} 0 768 2 ==>
-   lift_array768 res{1} = nttunpackv (lift_array768 res{2}) /\ 
-   pos_bound768_cxq res{1} 0 768 2 /\ 
-   pos_bound768_cxq res{2} 0 768 2.
+Jkem1024_avx2.M.__polyvec_ntt ~Jkem1024.M.__polyvec_ntt : 
+   lift_array1024 arg{1} = lift_array1024 arg{2} /\ 
+   signed_bound1024_cxq arg{1} 0 1024 2 /\ 
+   signed_bound1024_cxq arg{2} 0 1024 2 ==>
+   lift_array1024 res{1} = nttunpackv (lift_array1024 res{2}) /\ 
+   pos_bound1024_cxq res{1} 0 1024 2 /\ 
+   pos_bound1024_cxq res{2} 0 1024 2.
 proc *. 
 ecall {2} (polyvec_ntt_corr r{2}) => /=.
 conseq />;1: smt().
@@ -791,11 +3048,11 @@ have  : lift_polyvec (nttpackv r) = lift_polyvec r2.
 + rewrite -H1 -H;congr.
   rewrite /lift_polyvec KMatrix.Vector.eq_vectorP => k kb.
   rewrite !KMatrix.Vector.offunvE //=.
-  rewrite /lift_array768 tP in HH.
+  rewrite /lift_array1024 tP in HH.
   rewrite /subarray256 /lift_array256 tP => i ib.
   move : (HH (k*256+i) _); 1: by smt().
   rewrite !mapiE //= 1,2: /# !initiE //= /#.
-rewrite /lift_polyvec /lift_array768 tP KMatrix.Vector.eq_vectorP => H3 k kb. 
+rewrite /lift_polyvec /lift_array1024 tP KMatrix.Vector.eq_vectorP => H3 k kb. 
 rewrite !mapiE //=.
 case (0<=k<256).
 + move => kbb; move : (H3 0 _) => //; rewrite !KMatrix.Vector.offunvE //=.
@@ -827,24 +3084,40 @@ case (256 <= k < 512).
   move : nttpack_idxK; rewrite allP => Hidx.
   move : (Hidx (k-256) _)=>//; smt(mem_iota).
 
-move => *; move : (H3 2 _) => //; rewrite !KMatrix.Vector.offunvE //=.
+case (512 <= k < 768).
++ move => kbb ?; move : (H3 2 _) => //; rewrite !KMatrix.Vector.offunvE //=.
+  rewrite /nttpackv /nttunpackv /= /nttpack /nttunpack initiE//=.
+  rewrite /subarray256 /lift_array256 /nttpackv tP => HHH.
+  rewrite ifF  1:/# ifF 1:/# ifT 1:/# initiE //= 1:/#.
+  pose a := nttunpack_idx.[k-512].
+  move :nttunpack_bnd nttpack_bnd; rewrite !allP => pb upb.
+  rewrite initiE //= 1: /# !mapiE //= 1: /#. 
+  move : (HHH (a) _); 1: smt(). 
+  rewrite !mapiE //= 1,2: /# initiE//= 1:/#  initiE//= 1:/# initiE//= 1:/#.
+  rewrite ifF 1: /# ifF 1:/# initiE//= 1:/# initiE//= 1:/#. 
+  rewrite ifT 1: /#. 
+  pose b := nttpack_idx.[a].
+  move : nttpack_idxK; rewrite allP => Hidx.
+  move : (Hidx (k-512) _)=>//; smt(mem_iota).
+
+move => *; move : (H3 3 _) => //; rewrite !KMatrix.Vector.offunvE //=.
 rewrite /nttpackv /nttunpackv /= /nttpack /nttunpack initiE//=.
 rewrite /subarray256 /lift_array256 /nttpackv tP => HHH.
-rewrite ifF //= ifF //= initiE //= 1:/#.
-pose a := nttunpack_idx.[k-512].
+rewrite ifF  1:/# ifF 1:/# ifF 1:/# initiE //= 1:/#.
+pose a := nttunpack_idx.[k-768].
 move :nttunpack_bnd nttpack_bnd; rewrite !allP => pb upb.
 rewrite initiE //= 1: /# !mapiE //= 1: /#. 
 move : (HHH (a) _); 1: smt(). 
 rewrite !mapiE //= 1,2: /# initiE//= 1:/#  initiE//= 1:/# initiE//= 1:/#.
-rewrite ifF 1: /# ifF 1:/# initiE//= 1:/#. 
+rewrite ifF 1: /# ifF 1:/# ifF 1:/# initiE//= 1:/#. 
 pose b := nttpack_idx.[a].
 rewrite initiE//=  1:/# . 
 move : nttpack_idxK; rewrite allP => Hidx.
-move : (Hidx (k-512) _)=>//; smt(mem_iota).
+move : (Hidx (k-768) _)=>//; smt(mem_iota).
 qed.
 
 equiv polyinvnttequiv :
-Jkem768_avx2.M._poly_invntt ~Jkem768.M._poly_invntt : 
+Jkem1024_avx2.M._poly_invntt ~Jkem1024.M._poly_invntt : 
    lift_array256 arg{1} = nttunpack (lift_array256 arg{2}) /\ 
    signed_bound_cxq arg{1} 0 256 4 /\ 
    signed_bound_cxq arg{2} 0 256 4 ==>
@@ -858,31 +3131,45 @@ ecall{1} (poly_invntt_avx2_corr rp{2}) => /=.
 auto => /> &1 &2. rewrite lift_nttpack => -> H1 H2. rewrite nttunpackK //= => r <- H3. move => r0 <- H4. 
 rewrite /scale /map /lift_array256 /R tP => /> i Hi1 Hi2. rewrite !initiE //=. rewrite Zq.ComRing.mulrC //. qed.
 
-lemma signed_bound768_cxq_small r (i j:int) :
-  i <= j => signed_bound768_cxq r 0 768 i => signed_bound768_cxq r 0 768 j.
-rewrite /signed_bound768_cxq => />Hij H k Hk1 Hk2. move :(H k). rewrite Hk1 Hk2 => />. smt(). qed.
+lemma signed_bound1024_cxq_small r (i j:int) :
+  i <= j => signed_bound1024_cxq r 0 1024 i => signed_bound1024_cxq r 0 1024 j.
+rewrite /signed_bound1024_cxq => />Hij H k Hk1 Hk2. move :(H k). rewrite Hk1 Hk2 => />. smt(). qed.
 
-lemma eq_vectorP3 :
+lemma eq_vectorP4 :
       forall (v1 v2 : PolyVec.polyvec),
-        (v1 = v2) <=> ((KMatrix.Vector."_.[_]" v1 0 = KMatrix.Vector."_.[_]" v2 0) /\ (KMatrix.Vector."_.[_]" v1 1 = KMatrix.Vector."_.[_]" v2 1) /\ (KMatrix.Vector."_.[_]" v1 2 = KMatrix.Vector."_.[_]" v2 2) ).
+        (v1 = v2) <=> ((KMatrix.Vector."_.[_]" v1 0 = KMatrix.Vector."_.[_]" v2 0) /\ (KMatrix.Vector."_.[_]" v1 1 = KMatrix.Vector."_.[_]" v2 1) /\ (KMatrix.Vector."_.[_]" v1 2 = KMatrix.Vector."_.[_]" v2 2) /\ (KMatrix.Vector."_.[_]" v1 3 = KMatrix.Vector."_.[_]" v2 3)).
 smt(KMatrix.Vector.eq_vectorP). qed.
 
 equiv invnttequiv :
-Jkem768_avx2.M.__polyvec_invntt ~Jkem768.M.__polyvec_invntt : 
-   lift_array768 arg{1} = nttunpackv (lift_array768 arg{2}) /\ 
-   signed_bound768_cxq arg{1} 0 768 4 /\ 
-   signed_bound768_cxq arg{2} 0 768 4 ==>
-   lift_array768 res{1} = lift_array768 res{2} /\ 
-   signed_bound768_cxq res{1} 0 768 1 /\ 
-   signed_bound768_cxq res{2} 0 768 1.
+Jkem1024_avx2.M.__polyvec_invntt ~Jkem1024.M.__polyvec_invntt : 
+   lift_array1024 arg{1} = nttunpackv (lift_array1024 arg{2}) /\ 
+   signed_bound1024_cxq arg{1} 0 1024 4 /\ 
+   signed_bound1024_cxq arg{2} 0 1024 4 ==>
+   lift_array1024 res{1} = lift_array1024 res{2} /\ 
+   signed_bound1024_cxq res{1} 0 1024 1 /\ 
+   signed_bound1024_cxq res{2} 0 1024 1.
 proc *.
 ecall {2} (polyvec_invntt_corr r{2}) => /=.
 conseq />;1: smt().
 ecall {1} (polyvec_invntt_avx2_corr r{2}) => /=. 
 auto => /> &1 &2 -> Hm1 Hm2. rewrite unpackvK //= => r Hr1 Hr2 s Hs1 Hs2.
-rewrite /lift_array768 /map tP => />j Hj1 Hj2. rewrite !initiE //=.
-move :Hr1. rewrite !mapvE /lift_polyvec eq_vectorP3. rewrite !KMatrix.Vector.offunvE //=. rewrite /lift_array256 /subarray256 /map !tP -!andaE. apply andaW. move => Hr10. apply andaW. move => Hr11 Hr12. 
-move :Hs1. rewrite /scale_vector /lift_polyvec eq_vectorP3. rewrite !KMatrix.Vector.offunvE //=. rewrite /scale /lift_array256 /subarray256 /map !tP -!andaE. apply andaW. move => Hs10. apply andaW. move => Hs11 Hs12.
+rewrite /lift_array1024 /map tP => />j Hj1 Hj2. rewrite !initiE //=.
+move :Hr1; rewrite !mapvE /lift_polyvec eq_vectorP4 !KMatrix.Vector.offunvE //=. 
+rewrite /lift_array256 /subarray256 /map !tP -!andaE. 
+apply andaW. 
+move => Hr10. 
+apply andaW. 
+move => Hr11. 
+apply andaW. 
+move =>  Hr12 Hr21.   
+move :Hs1;rewrite /scale_vector /lift_polyvec eq_vectorP4 !KMatrix.Vector.offunvE //=.
+rewrite /scale /lift_array256 /subarray256 /map !tP -!andaE.
+apply andaW. 
+move => Hs10. 
+apply andaW. 
+move => Hs11.
+apply andaW. 
+move =>  Hs12 Hs21.  
 case (0 <= j < 256) => Hj_0.
  + move :(Hr10 j). rewrite Hj_0 !initiE //= !initiE //= => <-.
  + move :(Hs10 j). rewrite Hj_0 !initiE //= !initiE //= => <-.
@@ -892,9 +3179,14 @@ case (256 <= j < 512). move => Hj_1.
  + move :(Hr11 (j-256)). rewrite Hj_2 !initiE //= !initiE //= => <-.
  + move :(Hs11 (j-256)). rewrite Hj_2 !initiE //= !initiE //= => <-.
  + rewrite /R Zq.ComRing.mulrC => />. 
-move => Hj_2.
+case (512 <= j < 768). move => ?Hj_2.
  + have Hj_3: 0 <= j - 512 && j - 512 < 256. smt().
  + move :(Hr12 (j-512)). rewrite Hj_3 !initiE //= !initiE //= => <-.
  + move :(Hs12 (j-512)). rewrite Hj_3 !initiE //= !initiE //= => <-.
+ + rewrite /R Zq.ComRing.mulrC => />. 
+move =>? Hj_3.
+ + have Hj_4: 0 <= j - 768 && j - 768 < 256. smt().
+ + move :(Hr21 (j-768)). rewrite Hj_4 !initiE //= !initiE //= => <-.
+ + move :(Hs21 (j-768)). rewrite Hj_4 !initiE //= !initiE //= => <-.
  + rewrite /R Zq.ComRing.mulrC => />. 
 qed.
