proof/correctness768/avx2/MLKEM_keccak_avx2.ec
@@ -12,8 +12,7 @@ from CryptoSpecs require export Keccak1600_Spec Keccakf1600_Spec.
 from CryptoSpecs require import Symmetric.
 require import MLKEMFCLib.
 
-from JazzEC require import Jkem1024_avx2 WArray200.
-from JazzEC require Jkem1024_avx2.
+from JazzEC require import Jkem768_avx2 WArray200.
 
 
 
@@ -59,7 +58,7 @@ equiv addratebit_avx2x4_eq:
 (****************************************************************************)
 
 from Keccak require import Keccakf1600_ref Keccakf1600_avx2x4.
-from JazzEC require import WArray1536.
+from JazzEC require import WArray1152.
 from JazzEC require import Array24 Array5.
 
 from Keccak require Keccak1600_array_avx2.
@@ -118,6 +117,19 @@ equiv a32__absorb_array_avx2x4_eq:
  : ={arg} ==> ={res}
  by sim.
 
+(****************************************************************************)
+from JazzEC require import Array2 WArray2. 
+
+clone Keccak1600_array_avx2.KeccakArrayAvx2 as A2avx2
+ with op aSIZE <- 2,
+      theory A <- Array2,
+      theory WA <- WArray2
+      proof aSIZE_ge0 by done.
+
+equiv a2__absorb_array_avx2_eq:
+ M.a2____pabsorb_array_avx2 ~ A2avx2.M(A2avx2.P).__pabsorb_array_avx2
+ : ={arg} ==> ={res}
+ by sim.
 (****************************************************************************)
 from JazzEC require import Array33 WArray33.  (* DS SEED SIZE *)
 
@@ -190,31 +202,30 @@ equiv aBUFLEN__dumpstate_array_avx2x4_eq:
  by sim.
 
 (****************************************************************************)
-from JazzEC require import Array1568 WArray1568.
+from JazzEC require import Array1184 WArray1184.
 
-clone Keccak1600_array_avx2.KeccakArrayAvx2 as A1568avx2
- with op aSIZE <- 1568,
-      theory A <- Array1568,
-      theory WA <- WArray1568
+clone Keccak1600_array_avx2.KeccakArrayAvx2 as A1184avx2
+ with op aSIZE <- 1184,
+      theory A <- Array1184,
+      theory WA <- WArray1184
       proof aSIZE_ge0 by done.
 
-equiv a1568__absorb_array_avx2_eq:
- Jkem1024_avx2.M.a1568____absorb_array_avx2 ~ A1568avx2.M(A1568avx2.P).__absorb_array_avx2
+equiv a1184__absorb_array_avx2_eq:
+ Jkem768_avx2.M.a1184____absorb_array_avx2 ~ A1184avx2.M(A1184avx2.P).__absorb_array_avx2
  : ={arg} ==> ={res}
  by sim.
 
 
 (****************************************************************************)
-from JazzEC require import Array1600 WArray1600.
+from JazzEC require import Array1120 WArray1120.
 
-clone Keccak1600_array_avx2.KeccakArrayAvx2 as A1600avx2
- with op aSIZE <- 1600,
-      theory A <- Array1600,
-      theory WA <- WArray1600
+clone Keccak1600_array_avx2.KeccakArrayAvx2 as A1120avx2
+ with op aSIZE <- 1120,
+      theory A <- Array1120,
+      theory WA <- WArray1120
       proof aSIZE_ge0 by done.
-
-equiv a1600__absorb_array_avx2_eq:
- Jkem1024_avx2.M.a1600____absorb_array_avx2 ~ A1600avx2.M(A1600avx2.P).__absorb_array_avx2
+equiv a1120__absorb_array_avx2_eq:
+ Jkem768_avx2.M.a1120____absorb_array_avx2 ~ A1120avx2.M(A1120avx2.P).__absorb_array_avx2
  : ={arg} ==> ={res}
  by sim.
 
@@ -226,7 +237,7 @@ from JazzEC require import Array4.
 from JazzEC require import Array8.   (* mat. indexes *)
 from JazzEC require import Array128 WArray128.
 from JazzEC require import Array1408.
-from JazzEC require import Array1536.
+from JazzEC require import Array1152.
 from JazzEC require import Array2144. (* 4*BUF_SIZE *) 
 from JazzEC require import Array7.
 
@@ -268,7 +279,7 @@ module K = {
   }
   
 
-  proc _sha3_256A_A1568(out : W8.t Array32.t, in_0 : W8.t Array1568.t) :
+  proc _sha3_256A_A1184(out : W8.t Array32.t, in_0 : W8.t Array1184.t) :
     W8.t Array32.t = {
     var st : W256.t Array7.t;
     var offset : W64.t;
@@ -278,14 +289,14 @@ module K = {
     _1 <- witness;
     st <- witness;
     st <@ Jazz_avx2.M.__state_init_avx2();
-    (st, _0) <@ A1568avx2.M(A1568avx2.P).__absorb_array_avx2(st, in_0, W64.zero, 1568, 136, 6);
+    (st, _0) <@ A1184avx2.M(A1184avx2.P).__absorb_array_avx2(st, in_0, W64.zero, 1184, 136, 6);
     offset <- W64.zero;
     (out, _1) <@ A32avx2.M(A32avx2.P).__squeeze_array_avx2(out, offset, 32, st, 136);
     
     return out;
   }
   
-  proc _shake256_A32__A1600(out : W8.t Array32.t, in_0 : W8.t Array1600.t) :
+  proc _shake256_A32__A1120(out : W8.t Array32.t, in_0 : W8.t Array1120.t) :
     W8.t Array32.t = {
     var st : W256.t t;
     var offset : W64.t;
@@ -296,11 +307,34 @@ module K = {
     st <- witness;
     st <@ Jazz_avx2.M.__state_init_avx2();
     offset <- W64.zero;
-    (st, _0) <@ A1600avx2.M(A1600avx2.P).__absorb_array_avx2(st, in_0, offset, 1600, 136, 31);
+    (st, _0) <@ A1120avx2.M(A1120avx2.P).__absorb_array_avx2(st, in_0, offset, 1120, 136, 31);
     offset <- W64.zero;
     (out, _1) <@ A32avx2.M(A32avx2.P).__squeeze_array_avx2(out, offset, 32, st, 136);
     
     return out;
+  }
+
+  proc _shake128_absorb_A32_A2(seed : W8.t Array32.t, pos : W8.t Array2.t) : W256.t Array7.t = {
+    var st : W256.t Array7.t;
+    var pst_s : W64.t Array25.t;
+    var pst : W64.t Array25.t;
+    var offset : W64.t;
+    var _0 : int;
+    var _1 : W64.t;
+    var _2 : int;
+    var _3 : W64.t;
+    
+    pst <- witness;
+    pst_s <- witness;
+    st <- witness;
+    pst <- pst_s;
+    (pst, st) <@ Jazz_avx2.M.__pstate_init_avx2(pst);
+    offset <- W64.zero;
+    (pst, _0, st, _1) <@ A32avx2.M(A32avx2.P).__pabsorb_array_avx2(pst, 0, st, seed, offset, 32, 168, 0);
+    offset <- W64.zero;
+    (pst, _2, st, _3) <@ A2avx2.M(A2avx2.P).__pabsorb_array_avx2(pst, 32, st, pos, offset, 2, 168, 31);
+    
+    return st;
   }
 
   proc _shake128_squeeze3blocks(buf : W8.t Array536.t, st : W256.t t) :
@@ -482,7 +516,7 @@ rewrite stavx2_from_st25K -(Array64.of_listK W8.zero (SHA3_512 _)).
  by rewrite size_SQUEEZE1600 /#.
 congr; rewrite tP => i Hi.
 rewrite initiE // filliE //= Hi /=.
-by congr; rewrite /SHA3_512 /c1024_r8 /KECCAK1600; congr; congr => //.
+by congr; rewrite /SHA3_512.
 qed.
 
 (* IF NEEDED...
@@ -542,7 +576,7 @@ call (: offset=W64.of_int 0 /\ lEN=64 /\ rATE8=72 /\ absorb_spec_avx2 rATE8 6 (t
   rewrite size_SQUEEZE1600 /#.
  congr; rewrite tP => i Hi.
  rewrite initiE // filliE //= Hi /=.
- congr; rewrite /SHA3_512 /c1024_r8 /KECCAK1600; congr.
+ congr; rewrite /SHA3_512 /c768_r8 /KECCAK1600; congr.
  (* etc... *).
 wp; call (: st=stavx2_st0 /\ buf=_in /\ offset=W64.of_int 0 /\ lEN=33 /\ rATE8=72 /\ tRAILB=6 ==> absorb_spec_avx2 72 6 (to_list _in) res.`1 ).
  conseq a33__absorb_array_avx2_eq (A33avx2.absorb_array_avx2_ph stavx2_st0 _in W64.zero 33 72 6) => //.
@@ -574,7 +608,7 @@ rewrite stavx2_from_st25K -(Array64.of_listK W8.zero (SHA3_512 _)).
  by rewrite size_SQUEEZE1600 /#.
 congr; rewrite tP => i Hi.
 rewrite initiE // filliE //= Hi /=.
-by congr; rewrite /SHA3_512 /c1024_r8 /KECCAK1600; congr; congr => //.
+by congr; rewrite /SHA3_512.
 qed.
 
 lemma sha3_512A_A64_ll: islossless K._sha3_512A_A64.
@@ -625,7 +659,7 @@ smt().
 qed.
 
 phoare sha3_512A_512A_A64 m hpk:
- [ Jkem1024_avx2.M._sha3_512A_A64
+ [ Jkem768_avx2.M._sha3_512A_A64
  : 
    m = Array32.init (fun i => arg.`2.[i]) /\
    hpk = Array32.init (fun i => arg.`2.[i+32])
@@ -662,96 +696,96 @@ by rewrite /to_list initiE 1:// nth_mkseq /#.
 qed.
 
 (*********************************************************************************)
-from JazzEC require import Array1568.
+from JazzEC require import Array1184.
 
 
 (*********************************************************************************)
-equiv sha3_256A_A1568_eq:
-  Jkem1024_avx2.M._sha3_256A_A1568 ~ K._sha3_256A_A1568
+equiv sha3_256A_A1184_eq:
+  Jkem768_avx2.M._sha3_256A_A1184 ~ K._sha3_256A_A1184
  : ={arg} ==> ={res}
  by sim.
 
-hoare sha3_256A_A1568_h' _in:
- K._sha3_256A_A1568
+hoare sha3_256A_A1184_h' _in:
+ K._sha3_256A_A1184
  : arg.`2 = _in 
  ==> 
-   res = SHA3_256_1568_32
-            (Array1536.init (fun i => _in.[i]),
-             Array32.init (fun i => _in.[1536+i])).
+   res = SHA3_256_1184_32
+            (Array1152.init (fun i => _in.[i]),
+             Array32.init (fun i => _in.[1152+i])).
 proof.
 proc => /=.
 ecall (A32avx2.squeeze_array_avx2_h out offset 32 st 136).
-wp; ecall (A1568avx2.absorb_array_avx2_h st in_0 W64.zero 1568 136 6).
+wp; ecall (A1184avx2.absorb_array_avx2_h st in_0 W64.zero 1184 136 6).
 wp; call state_init_avx2_h.
 auto =>  /> &m.
 move=> [st ?] /= => -> _.
 move=> [_out ?] /= -> _.
-rewrite /SHA3_256_1568_32 stavx2_from_st25K /= tP => i Hi.
+rewrite /SHA3_256_1184_32 stavx2_from_st25K /= tP => i Hi.
 rewrite initiE // filliE //= Hi /=.
 rewrite /SHA3_256 /c512_r8 /KECCAK1600; congr; congr; congr => //.
-rewrite (:1568=1536+32) 1:// /sub mkseq_add 1..2://; congr.
+rewrite (:1184=1152+32) 1:// /sub mkseq_add 1..2://; congr.
  by apply eq_in_mkseq => k Hk /=; rewrite initiE /#.
 by apply eq_in_mkseq => k Hk /=; rewrite initiE /#.
 qed.
 
-lemma sha3_256A_A1568_ll: islossless K._sha3_256A_A1568.
+lemma sha3_256A_A1184_ll: islossless K._sha3_256A_A1184.
 proof.
 proc.
 call A32avx2.squeeze_array_avx2_ll.
-wp; call A1568avx2.absorb_array_avx2_ll.
+wp; call A1184avx2.absorb_array_avx2_ll.
 call state_init_avx2_ll.
 by auto => />.
 qed.
 
-phoare sha3_256A_A1568_ph' _in:
- [ K._sha3_256A_A1568
+phoare sha3_256A_A1184_ph' _in:
+ [ K._sha3_256A_A1184
  : arg.`2 = _in 
  ==> 
-   res = SHA3_256_1568_32
-            (Array1536.init (fun i => _in.[i]),
-             Array32.init (fun i => _in.[1536+i]))
+   res = SHA3_256_1184_32
+            (Array1152.init (fun i => _in.[i]),
+             Array32.init (fun i => _in.[1152+i]))
  ] = 1%r.
-proof. by conseq sha3_256A_A1568_ll (sha3_256A_A1568_h' _in). qed.
+proof. by conseq sha3_256A_A1184_ll (sha3_256A_A1184_h' _in). qed.
 
-phoare sha3_256A_M1568_ph (inp : W8.t Array1568.t):
- [ Jkem1024_avx2.M._sha3_256A_A1568
+phoare sha3_256A_M1184_ph (inp : W8.t Array1184.t):
+ [ Jkem768_avx2.M._sha3_256A_A1184
  : arg.`2 = inp 
  ==> 
-   res = SHA3_256_1568_32
-            (Array1536.init (fun i => inp.[i]),
-             Array32.init (fun i => inp.[1536+i]))
+   res = SHA3_256_1184_32
+            (Array1152.init (fun i => inp.[i]),
+             Array32.init (fun i => inp.[1152+i]))
  ] = 1%r.
 proof.
-by conseq sha3_256A_A1568_eq (sha3_256A_A1568_ph' inp) => /> /#.
+by conseq sha3_256A_A1184_eq (sha3_256A_A1184_ph' inp) => /> /#.
 qed.
 
 (*********************************************************************************)
 
 
-from JazzEC require import Array1408 Array160.
+from JazzEC require import Array960 Array128.
 
 
 (*********************************************************************************)
-equiv shake256_A32__A1600_eq:
-  Jkem1024_avx2.M._shake256_A32__A1600 ~ K._shake256_A32__A1600
+equiv shake256_A32__A1120_eq:
+  Jkem768_avx2.M._shake256_A32__A1120 ~ K._shake256_A32__A1120
  : ={arg, Glob.mem} ==> ={res, Glob.mem}
  by sim.
 
-hoare shake256_A32__A1600_h' _in:
- K._shake256_A32__A1600
+hoare shake256_A32__A1120_h' _in:
+ K._shake256_A32__A1120
  : arg.`2=_in
  ==>
-   res = SHAKE_256_1600_32
+   res = SHAKE_256_1120_32
            (init (fun (k : int) => _in.[k]))%Array32
-           ((init (fun (k : int) => _in.[32 + k]))%Array1408,
-            (init (fun (k : int) => _in.[1408 + 32 + k]))%Array160).
+           ((init (fun (k : int) => _in.[32 + k]))%Array960,
+            (init (fun (k : int) => _in.[960 + 32 + k]))%Array128).
 proof.
 proc => /=.
 ecall (A32avx2.squeeze_array_avx2_h out offset 32 st 136).
-wp; ecall (A1600avx2.absorb_array_avx2_h st in_0 offset 1600 136 31).
+wp; ecall (A1120avx2.absorb_array_avx2_h st in_0 offset 1120 136 31).
 wp; call state_init_avx2_h.
 auto => |> &m [st ?] /= -> _ [out st2] /= -> Hst2.
-rewrite stavx2_from_st25K /SHAKE_256_1600_32 -(Array32.of_listK W8.zero (SHAKE256 _ _)).
+rewrite stavx2_from_st25K /SHAKE_256_1120_32 -(Array32.of_listK W8.zero (SHAKE256 _ _)).
  by rewrite size_SHAKE256 /#.
 rewrite tP => i Hi.
 rewrite filliE 1:// /= Hi /= get_of_list 1://.
@@ -759,49 +793,49 @@ rewrite of_listK.
  by rewrite size_SHAKE256 /#.
 rewrite /SHAKE256 /KECCAK1600; congr; congr; 1:smt().
 congr; 1..2:smt().
-rewrite (:1600=32+1408+160) 1:// /sub !mkseq_add 1..4:/#; congr.
+rewrite (:1120=32+960+128) 1:// /sub !mkseq_add 1..4:/#; congr.
  congr.
   by apply eq_in_mkseq => k Hk /=; rewrite initiE.
  by apply eq_in_mkseq => k Hk /=; rewrite initiE /#.
 by apply eq_in_mkseq => k Hk /=; rewrite initiE /#.
 qed.
 
-lemma shake256_A32__A1600_ll: islossless K._shake256_A32__A1600.
+lemma shake256_A32__A1120_ll: islossless K._shake256_A32__A1120.
 proof.
 proc.
 call A32avx2.squeeze_array_avx2_ll.
-wp; call A1600avx2.absorb_array_avx2_ll.
+wp; call A1120avx2.absorb_array_avx2_ll.
 wp; call state_init_avx2_ll.
 by auto.
 qed.
 
-phoare shake256_A32__A1600_ph' _in:
- [ K._shake256_A32__A1600
+phoare shake256_A32__A1120_ph' _in:
+ [ K._shake256_A32__A1120
  : arg.`2=_in
  ==>
-   res = SHAKE_256_1600_32
+   res = SHAKE_256_1120_32
            (init (fun (k : int) => _in.[k]))%Array32
-           ((init (fun (k : int) => _in.[32 + k]))%Array1408,
-            (init (fun (k : int) => _in.[1408 + 32 + k]))%Array160)
+           ((init (fun (k : int) => _in.[32 + k]))%Array960,
+            (init (fun (k : int) => _in.[960 + 32 + k]))%Array128)
  ] = 1%r.
 proof.
-by conseq shake256_A32__A1600_ll (shake256_A32__A1600_h' _in).
+by conseq shake256_A32__A1120_ll (shake256_A32__A1120_h' _in).
 qed.
 
-phoare shake256_A32_A1600_ph (_in : W8.t Array1600.t):
- [ Jkem1024_avx2.M._shake256_A32__A1600
+phoare shake256_A32_A1120_ph (_in : W8.t Array1120.t):
+ [ Jkem768_avx2.M._shake256_A32__A1120
  : arg.`2=_in
- ==> res = SHAKE_256_1600_32 
+ ==> res = SHAKE_256_1120_32 
                (init (fun (k : int) => _in.[k]))%Array32
-               ((init (fun (k : int) => _in.[32 + k]))%Array1408,
-                (init (fun (k : int) => _in.[1408 + 32 + k]))%Array160)
+               ((init (fun (k : int) => _in.[32 + k]))%Array960,
+                (init (fun (k : int) => _in.[960 + 32 + k]))%Array128)
  ] = 1%r.
 proof.
-by conseq shake256_A32__A1600_eq (shake256_A32__A1600_ph' _in) => /> /#.
+by conseq shake256_A32__A1120_eq (shake256_A32__A1120_ph' _in) => /> /#.
 qed.
 
 (*********************************************************************************)
-(* 
+
 equiv shake128_absorb_A32_A2_eq:
   M._shake128_absorb_A32_A2 ~ K._shake128_absorb_A32_A2
  : ={arg} ==> ={res}
@@ -839,12 +873,11 @@ phoare shake128_absorb_A32_A2_ph' _rho _rc:
 proof.
 by conseq shake128_absorb_A32_A2_ll (shake128_absorb_A32_A2_h' _rho _rc).
 qed.
-*)
 op stmatch_avx2 st stavx2 =
  stavx2 = stavx2_from_st25 st.
-(* 
+
 phoare shake128_absorb_A32_A2_ph _rho _rc:
- [ Jkem1024_avx2.M._shake128_absorb_A32_A2
+ [ Jkem768_avx2.M._shake128_absorb_A32_A2
    : seed = _rho /\ pos = _rc
      ==>
      stmatch_avx2 (SHAKE128_ABSORB (to_list _rho ++ to_list _rc)) res
@@ -852,9 +885,7 @@ phoare shake128_absorb_A32_A2_ph _rho _rc:
 proof.
 by conseq shake128_absorb_A32_A2_eq (shake128_absorb_A32_A2_ph' _rho _rc) => /> /#.
 qed.
-*)
 (*********************************************************************************)
-(* 
 equiv shake128_squeeze3blocks_eq:
   M._shake128_squeeze3blocks ~ K._shake128_squeeze3blocks
  : ={arg} ==> ={res}
@@ -937,7 +968,7 @@ phoare shake128_squeeze3blocks_ph _buf _st:
 proof.
 by conseq shake128_squeeze3blocks_eq (shake128_squeeze3blocks_ph' _buf _st) => /> /#.
 qed.
-*)
+
 (*********************************************************************************)
 equiv shake128_next_state_eq:
   M._shake128_next_state ~ K._shake128_next_state
@@ -994,7 +1025,7 @@ by conseq shake128_next_state_ll (shake128_next_state_h' _buf).
 qed.
 
 phoare shake128_next_state_ph _buf:
- [ Jkem1024_avx2.M._shake128_next_state
+ [ Jkem768_avx2.M._shake128_next_state
  : buf = _buf
    ==>
    let st = bytes2state (sub _buf (2*168) 200) in
@@ -1077,7 +1108,7 @@ qed.
 
 phoare shake256x4_A128__A32_A1_ph _seed _nonces :
  [ 
-   Jkem1024_avx2.M._shake256x4_A128__A32_A1
+   Jkem768_avx2.M._shake256x4_A128__A32_A1
  : seed = _seed /\ nonces = _nonces 
  ==>
     res.`1 = Array128.of_list W8.zero (SHAKE256 (to_list _seed ++ [_nonces.[0]]) 128)
@@ -1158,7 +1189,7 @@ by conseq shake128x4_absorb_A32_A2_ll (shake128x4_absorb_A32_A2_h' _rho _rc).
 qed.
 
 phoare shake128x4_absorb_A32_A2_ph _rho _rc:
- [ Jkem1024_avx2.M._shake128x4_absorb_A32_A2
+ [ Jkem768_avx2.M._shake128x4_absorb_A32_A2
  : seed = _rho /\ pos = _rc
  ==>
     match_state4x
@@ -1337,7 +1368,7 @@ by conseq shake128x4_squeeze3blocks_ll (shake128x4_squeeze3blocks_h' _st0 _st1 _
 qed.
 
 phoare shake128x4_squeeze3blocks_ph _st0 _st1 _st2 _st3:
- [ Jkem1024_avx2.M._shake128x4_squeeze3blocks
+ [ Jkem768_avx2.M._shake128x4_squeeze3blocks
  : match_state4x _st0 _st1 _st2 _st3 st
  ==>
       sub res.`2 (0*536) (3*168) = SHAKE128_SQUEEZE (3*168) _st0
